@prefix sdmx-measure: <http://purl.org/linked-data/sdmx/2009/measure#> .
@prefix ex-geo: <http://example.org/geo#> .
@prefix foaf:  <http://xmlns.com/foaf/0.1/> .
@prefix interval: <http://reference.data.gov.uk/def/intervals/> .
@prefix sdmx-attribute: <http://purl.org/linked-data/sdmx/2009/attribute#> .
@prefix void:  <http://rdfs.org/ns/void#> .
@prefix sdmx-concept: <http://purl.org/linked-data/sdmx/2009/concept#> .
@prefix qb:    <http://purl.org/linked-data/cube#> .
@prefix org:   <http://www.w3.org/ns/org#> .
@prefix sdmx-code: <http://purl.org/linked-data/sdmx/2009/code#> .
@prefix vcard: <http://www.w3.org/2006/vcard/ns#> .
@prefix dcterms: <http://dublincore.org/documents/dcmi-terms/> .
@prefix rdfs:  <http://www.w3.org/2000/01/rdf-schema#> .
@prefix eg:    <http://example.org/ns#> .
@prefix dct:   <http://purl.org/dc/terms/> .
@prefix owl:   <http://www.w3.org/2002/07/owl#> .
@prefix xsd:   <http://www.w3.org/2001/XMLSchema#> .
@prefix rdf:   <http://www.w3.org/1999/02/22-rdf-syntax-ns#> .
@prefix scovo: <http://purl.org/NET/scovo#> .
@prefix sdmx-metadata: <http://purl.org/linked-data/sdmx/2009/metadata#> .
@prefix admingeo: <http://data.ordnancesurvey.co.uk/ontology/admingeo/> .
@prefix sdmx:  <http://purl.org/linked-data/sdmx#> .
@prefix skos:  <http://www.w3.org/2004/02/skos/core#> .
@prefix sdmx-dimension: <http://purl.org/linked-data/sdmx/2009/dimension#> .
@prefix sdmx-subject: <http://purl.org/linked-data/sdmx/2009/subject#> .

sdmx-code:decimals-8  a    skos:Concept , sdmx:Concept , sdmx-code:Decimals ;
        skos:inScheme      sdmx-code:decimals ;
        skos:notation      "8" ;
        skos:prefLabel     "Eight"@en ;
        skos:topConceptOf  sdmx-code:decimals .

sdmx-metadata:comparGeo
        a                 sdmx:MetadataProperty , rdf:Property ;
        rdfs:comment      "Extent to which statistics are comparable between geographical areas."@en ;
        rdfs:isDefinedBy  <http://sdmx.org/wp-content/uploads/2009/01/01_sdmx_cog_annex_1_cdc_2009.pdf> ;
        rdfs:label        "Comparability - geographical"@en ;
        qb:concept        sdmx-concept:comparGeo .

sdmx-dimension:civilStatus
        a                 qb:DimensionProperty , rdf:Property ;
        rdfs:comment      "Legal, conjugal status of each individual in relation to the marriage laws or customs of the country."@en ;
        rdfs:isDefinedBy  <http://sdmx.org/wp-content/uploads/2009/01/01_sdmx_cog_annex_1_cdc_2009.pdf> ;
        rdfs:label        "Civil Status"@en ;
        rdfs:range        rdfs:Resource ;
        qb:concept        sdmx-concept:civilStatus .

sdmx-concept:origDataId
        a                 sdmx:Concept , skos:Concept ;
        rdfs:comment      "The data identifier as found in the originating database."@en ;
        rdfs:isDefinedBy  <http://sdmx.org/wp-content/uploads/2009/01/01_sdmx_cog_annex_1_cdc_2009.pdf> ;
        rdfs:label        "Original Data Identifier"@en ;
        skos:inScheme     sdmx-concept:cog ;
        skos:notation     "urn:sdmx:org.sdmx.infomodel.conceptscheme.Concept=SDMX:CROSS_DOMAIN_CONCEPTS[1.0].ORIG_DATA_ID" .

sdmx-attribute:recording
        a                 qb:AttributeProperty , rdf:Property ;
        rdfs:comment      "Processes and standards employed in calculating statistical aggregates."@en ;
        rdfs:isDefinedBy  <http://sdmx.org/wp-content/uploads/2009/01/01_sdmx_cog_annex_1_cdc_2009.pdf> ;
        rdfs:label        "Recording Basis"@en ;
        qb:concept        sdmx-concept:recording .

sdmx:ConceptScheme  a    rdfs:Class , owl:Class ;
        rdfs:label       "Concept scheme"@en ;
        rdfs:subClassOf  skos:ConceptScheme .

sdmx-concept:userNeeds
        a                 sdmx:Concept , skos:Concept ;
        rdfs:comment      "Description of users and their respective needs with respect to the statistical data."@en ;
        rdfs:isDefinedBy  <http://sdmx.org/wp-content/uploads/2009/01/01_sdmx_cog_annex_1_cdc_2009.pdf> ;
        rdfs:label        "Relevance - user needs"@en ;
        skos:broader      sdmx-concept:relevance ;
        skos:inScheme     sdmx-concept:cog ;
        skos:notation     "urn:sdmx:org.sdmx.infomodel.conceptscheme.Concept=SDMX:CROSS_DOMAIN_CONCEPTS[1.0].USER_NEEDS" .

sdmx-concept:revPractice
        a                 sdmx:Concept , skos:Concept ;
        rdfs:comment      "Information on the data revision practice."@en ;
        rdfs:isDefinedBy  <http://sdmx.org/wp-content/uploads/2009/01/01_sdmx_cog_annex_1_cdc_2009.pdf> ;
        rdfs:label        "Data Revision - practice"@en ;
        skos:broader      sdmx-concept:dataRev ;
        skos:inScheme     sdmx-concept:cog ;
        skos:notation     "urn:sdmx:org.sdmx.infomodel.conceptscheme.Concept=SDMX:CROSS_DOMAIN_CONCEPTS[1.0].REV_PRACTICE" .

sdmx-code:Currency  a    rdfs:Class , owl:Class ;
        rdfs:comment     "This code list provides code values for currencies."@en ;
        rdfs:label       "code list for Currency (CURRENCY) - codelist class"@en ;
        rdfs:seeAlso     sdmx-code:currency ;
        rdfs:subClassOf  skos:Concept .

sdmx-code:unitMult-9  a    skos:Concept , sdmx:Concept , sdmx-code:UnitMult ;
        skos:inScheme      sdmx-code:unitMult ;
        skos:notation      "9" ;
        skos:prefLabel     "Billions"@en ;
        skos:topConceptOf  sdmx-code:unitMult .

sdmx-concept:qualityAssmnt
        a                 sdmx:Concept , skos:Concept ;
        rdfs:comment      "Overall assessment of data quality, based on standard quality criteria."@en ;
        rdfs:isDefinedBy  <http://sdmx.org/wp-content/uploads/2009/01/01_sdmx_cog_annex_1_cdc_2009.pdf> ;
        rdfs:label        "Quality Management - assessment"@en ;
        skos:broader      sdmx-concept:qualityMgmnt ;
        skos:inScheme     sdmx-concept:cog ;
        skos:notation     "urn:sdmx:org.sdmx.infomodel.conceptscheme.Concept=SDMX:CROSS_DOMAIN_CONCEPTS[1.0].QUALITY_ASSMNT" .

sdmx-attribute:profMeth
        a                 qb:AttributeProperty , rdf:Property ;
        rdfs:comment      "Describes the elements providing assurances that the choices of sources and statistical techniques as well as decisions about dissemination are informed solely by statistical considerations."@en ;
        rdfs:isDefinedBy  <http://sdmx.org/wp-content/uploads/2009/01/01_sdmx_cog_annex_1_cdc_2009.pdf> ;
        rdfs:label        "Professionalism - methodology"@en ;
        qb:concept        sdmx-concept:profMeth .

sdmx-code:Decimals  a    rdfs:Class , owl:Class ;
        rdfs:comment     "It provides a list of values showing the number of decimal digits used in the data."@en ;
        rdfs:label       "Code list for Decimals (DECIMALS) - codelist class"@en ;
        rdfs:seeAlso     sdmx-code:decimals ;
        rdfs:subClassOf  skos:Concept .

eg:o63  a                  qb:Observation ;
        eg:lifeExpectancy  81.7 ;
        eg:refArea         ex-geo:monmouthshire_00pp ;
        qb:dataSet         eg:dataset-le3 .

sdmx-attribute:contactName
        a                 qb:AttributeProperty , rdf:Property ;
        rdfs:comment      "The name of the contact points for the data or metadata."@en ;
        rdfs:isDefinedBy  <http://sdmx.org/wp-content/uploads/2009/01/01_sdmx_cog_annex_1_cdc_2009.pdf> ;
        rdfs:label        "Contact name"@en ;
        qb:concept        sdmx-concept:contactName .

sdmx-attribute:dataValidation
        a                 qb:AttributeProperty , rdf:Property ;
        rdfs:comment      "Process of monitoring the results of data compilation and ensuring the quality of the statistical results."@en ;
        rdfs:isDefinedBy  <http://sdmx.org/wp-content/uploads/2009/01/01_sdmx_cog_annex_1_cdc_2009.pdf> ;
        rdfs:label        "Data Validation"@en ;
        qb:concept        sdmx-concept:dataValidation .

sdmx-metadata:userSat
        a                 sdmx:MetadataProperty , rdf:Property ;
        rdfs:comment      "Measure to determine user satisfaction."@en ;
        rdfs:isDefinedBy  <http://sdmx.org/wp-content/uploads/2009/01/01_sdmx_cog_annex_1_cdc_2009.pdf> ;
        rdfs:label        "Relevance - user satisifaction"@en ;
        qb:concept        sdmx-concept:userSat .

eg:o31  a                  qb:Observation ;
        eg:lifeExpectancy  77.1 ;
        eg:refArea         ex-geo:newport_00pr ;
        qb:dataSet         eg:dataset-le3 .

sdmx-concept:contact  a   sdmx:Concept , skos:Concept ;
        rdfs:comment      "Individual or organisational contact points for the data or metadata, including information on how to reach the contact points."@en ;
        rdfs:isDefinedBy  <http://sdmx.org/wp-content/uploads/2009/01/01_sdmx_cog_annex_1_cdc_2009.pdf> ;
        rdfs:label        "Contact"@en ;
        skos:inScheme     sdmx-concept:cog ;
        skos:notation     "urn:sdmx:org.sdmx.infomodel.conceptscheme.Concept=SDMX:CROSS_DOMAIN_CONCEPTS[1.0].CONTACT" .

sdmx:identityProperty
        a                   rdf:Property , owl:ObjectProperty ;
        rdfs:comment        "identifies the Concept that plays the role of an identifier which is taken from a known scheme of identifiers"@en ;
        rdfs:label          "identity property"@en ;
        rdfs:range          sdmx:DimensionOrAttributeProperty ;
        rdfs:subPropertyOf  sdmx:component .

sdmx-code:Area  a        rdfs:Class , owl:Class ;
        rdfs:comment     ": This code list provides code values for geographical areas, defined as areas included within the borders of a country, region, group of countries, etc."@en ;
        rdfs:label       "Code list for providing values to concepts such as 'Reference area' and/or 'Counterpart area' - codelist class"@en ;
        rdfs:seeAlso     sdmx-code:area ;
        rdfs:subClassOf  skos:Concept .

sdmx-attribute:adjustCoded
        a                 qb:AttributeProperty , rdf:Property ;
        rdfs:comment      "Type of adjustment used, represented by a code."@en ;
        rdfs:isDefinedBy  <http://sdmx.org/wp-content/uploads/2009/01/01_sdmx_cog_annex_1_cdc_2009.pdf> ;
        rdfs:label        "Adjustment - coded"@en ;
        qb:concept        sdmx-concept:adjustCoded .

sdmx-metadata:statPop
        a                 sdmx:MetadataProperty , rdf:Property ;
        rdfs:comment      "The total membership or population or \"universe\" of a defined class of people, objects or events."@en ;
        rdfs:isDefinedBy  <http://sdmx.org/wp-content/uploads/2009/01/01_sdmx_cog_annex_1_cdc_2009.pdf> ;
        rdfs:label        "Statistical Population"@en ;
        qb:concept        sdmx-concept:statPop .

sdmx-concept:statUnit
        a                 sdmx:Concept , skos:Concept ;
        rdfs:comment      "Entity for which information is sought and for which statistics are ultimately compiled."@en ;
        rdfs:isDefinedBy  <http://sdmx.org/wp-content/uploads/2009/01/01_sdmx_cog_annex_1_cdc_2009.pdf> ;
        rdfs:label        "Statistical Unit"@en ;
        skos:inScheme     sdmx-concept:cog ;
        skos:notation     "urn:sdmx:org.sdmx.infomodel.conceptscheme.Concept=SDMX:CROSS_DOMAIN_CONCEPTS[1.0].STAT_UNIT" .

sdmx-concept:revPolicy
        a                 sdmx:Concept , skos:Concept ;
        rdfs:comment      "Policy aimed at ensuring the transparency of disseminated data, whereby preliminary data are compiled that are later revised."@en ;
        rdfs:isDefinedBy  <http://sdmx.org/wp-content/uploads/2009/01/01_sdmx_cog_annex_1_cdc_2009.pdf> ;
        rdfs:label        "Data Revision - policy"@en ;
        skos:broader      sdmx-concept:dataRev ;
        skos:inScheme     sdmx-concept:cog ;
        skos:notation     "urn:sdmx:org.sdmx.infomodel.conceptscheme.Concept=SDMX:CROSS_DOMAIN_CONCEPTS[1.0].REV_POLICY" .

sdmx-metadata:statUnit
        a                 sdmx:MetadataProperty , rdf:Property ;
        rdfs:comment      "Entity for which information is sought and for which statistics are ultimately compiled."@en ;
        rdfs:isDefinedBy  <http://sdmx.org/wp-content/uploads/2009/01/01_sdmx_cog_annex_1_cdc_2009.pdf> ;
        rdfs:label        "Statistical Unit"@en ;
        qb:concept        sdmx-concept:statUnit .

sdmx-attribute:profCond
        a                 qb:AttributeProperty , rdf:Property ;
        rdfs:comment      "Provision for assuring the qualifications of staff and allowing staff to perform their functions without intervention motivated by non-statistical objectives."@en ;
        rdfs:isDefinedBy  <http://sdmx.org/wp-content/uploads/2009/01/01_sdmx_cog_annex_1_cdc_2009.pdf> ;
        rdfs:label        "Professionalism - code of conduct"@en ;
        qb:concept        sdmx-concept:profCond .

sdmx-concept:newsRel  a   sdmx:Concept , skos:Concept ;
        rdfs:comment      "Regular or ad-hoc press releases linked to the data."@en ;
        rdfs:isDefinedBy  <http://sdmx.org/wp-content/uploads/2009/01/01_sdmx_cog_annex_1_cdc_2009.pdf> ;
        rdfs:label        "Dissemination Format - news release"@en ;
        skos:broader      sdmx-concept:dissFormat ;
        skos:inScheme     sdmx-concept:cog ;
        skos:notation     "urn:sdmx:org.sdmx.infomodel.conceptscheme.Concept=SDMX:CROSS_DOMAIN_CONCEPTS[1.0].NEWS_REL" .

sdmx-code:timeFormat-708
        a                  skos:Concept , sdmx:Concept , sdmx-code:TimeFormat ;
        skos:definition    "(for quarterly series)\nfrom year/quarter to year/quarter"@en ;
        skos:inScheme      sdmx-code:timeFormat ;
        skos:notation      "708" ;
        skos:prefLabel     "CCYYQCCYYQ"@en ;
        skos:topConceptOf  sdmx-code:timeFormat .

sdmx:DataSet  a              rdfs:Class , owl:Class ;
        rdfs:label           "Data set"@en ;
        rdfs:subClassOf      sdmx:Attachable , sdmx:DataSetOrFlow , sdmx:ReportEntry , sdmx:Structured ;
        owl:equivalentClass  scovo:Dataset .

sdmx-metadata:instManShar
        a                 sdmx:MetadataProperty , rdf:Property ;
        rdfs:comment      "Arrangements or procedures for data sharing and coordination between data producing agencies."@en ;
        rdfs:isDefinedBy  <http://sdmx.org/wp-content/uploads/2009/01/01_sdmx_cog_annex_1_cdc_2009.pdf> ;
        rdfs:label        "Institutional Mandate - data sharing"@en ;
        qb:concept        sdmx-concept:instManShar .

sdmx-code:decimals-3  a    skos:Concept , sdmx:Concept , sdmx-code:Decimals ;
        skos:inScheme      sdmx-code:decimals ;
        skos:notation      "3" ;
        skos:prefLabel     "Three"@en ;
        skos:topConceptOf  sdmx-code:decimals .

sdmx-metadata:obsPreBreak
        a                 sdmx:MetadataProperty , rdf:Property ;
        rdfs:comment      "The observation, at a time series break period, that was calculated using the old methodology."@en ;
        rdfs:isDefinedBy  <http://sdmx.org/wp-content/uploads/2009/01/01_sdmx_cog_annex_1_cdc_2009.pdf> ;
        rdfs:label        "Observation Pre-break Value"@en ;
        qb:concept        sdmx-concept:obsPreBreak .

sdmx:MeasureTypeProperty
        a                 rdfs:Class , owl:Class ;
        rdfs:label        "Measure type property"@en ;
        rdfs:subClassOf   sdmx:ConceptRoleProperty , sdmx:DimensionProperty ;
        owl:disjointWith  sdmx:MeasureProperty , sdmx:AttributeProperty .

sdmx:dataSet  a                 rdf:Property , owl:ObjectProperty ;
        rdfs:domain             sdmx:Observation ;
        rdfs:label              "data set"@en ;
        rdfs:range              sdmx:DataSet ;
        owl:equivalentProperty  scovo:dataset .

sdmx-concept:comparDomains
        a                 sdmx:Concept , skos:Concept ;
        rdfs:comment      "Extent to which statistics are comparable between different statistical domains."@en ;
        rdfs:isDefinedBy  <http://sdmx.org/wp-content/uploads/2009/01/01_sdmx_cog_annex_1_cdc_2009.pdf> ;
        rdfs:label        "Comparability - between domains"@en ;
        skos:broader      sdmx-concept:comparability ;
        skos:inScheme     sdmx-concept:cog ;
        skos:notation     "urn:sdmx:org.sdmx.infomodel.conceptscheme.Concept=SDMX:CROSS_DOMAIN_CONCEPTS[1.0].COMPAR_DOMAINS" .

sdmx-attribute:timeFormat
        a                 qb:AttributeProperty , rdf:Property , qb:CodedProperty ;
        rdfs:comment      "Technical format in which time is represented for the measured phenomenon."@en ;
        rdfs:isDefinedBy  <http://sdmx.org/wp-content/uploads/2009/01/01_sdmx_cog_annex_1_cdc_2009.pdf> ;
        rdfs:label        "Time Format"@en ;
        rdfs:range        sdmx-code:TimeFormat ;
        qb:codeList       sdmx-code:timeFormat ;
        qb:concept        sdmx-concept:timeFormat .

sdmx:observation  a  rdf:Property , owl:ObjectProperty ;
        rdfs:domain  sdmx:Slice ;
        rdfs:label   "observation"@en ;
        rdfs:range   sdmx:Observation .

sdmx-concept:adjustDetail
        a                 sdmx:Concept , skos:Concept ;
        rdfs:comment      "Textual description of the type of adjustment used."@en ;
        rdfs:isDefinedBy  <http://sdmx.org/wp-content/uploads/2009/01/01_sdmx_cog_annex_1_cdc_2009.pdf> ;
        rdfs:label        "Adjustment - detail"@en ;
        skos:broader      sdmx-concept:adjustment ;
        skos:inScheme     sdmx-concept:cog ;
        skos:notation     "urn:sdmx:org.sdmx.infomodel.conceptscheme.Concept=SDMX:CROSS_DOMAIN_CONCEPTS[1.0].ADJUST_DETAIL" .

eg:o44  a                  qb:Observation ;
        eg:lifeExpectancy  79.4 ;
        eg:refArea         ex-geo:merthyr_tdfil_00ph ;
        qb:dataSet         eg:dataset-le3 .

sdmx-code:unitMult-4  a    skos:Concept , sdmx:Concept , sdmx-code:UnitMult ;
        skos:inScheme      sdmx-code:unitMult ;
        skos:notation      "4" ;
        skos:prefLabel     "Tens of thousands"@en ;
        skos:topConceptOf  sdmx-code:unitMult .

eg:o12  a                  qb:Observation ;
        eg:lifeExpectancy  78.7 ;
        eg:refArea         ex-geo:cardiff_00pt ;
        qb:dataSet         eg:dataset-le3 .

sdmx:Section  a          rdfs:Class , owl:Class ;
        rdfs:label       "Section"@en ;
        rdfs:subClassOf  sdmx:Attachable , sdmx:Slice .

sdmx:PrimaryMeasureProperty
        a                 rdfs:Class , owl:Class ;
        rdfs:label        "Primary measure property"@en ;
        rdfs:subClassOf   sdmx:ConceptRoleProperty , sdmx:MeasureProperty ;
        owl:disjointWith  sdmx:DimensionProperty , sdmx:AttributeProperty .

sdmx-attribute:revStudy
        a                 qb:AttributeProperty , rdf:Property ;
        rdfs:comment      "Information about data revision studies and analyses."@en ;
        rdfs:isDefinedBy  <http://sdmx.org/wp-content/uploads/2009/01/01_sdmx_cog_annex_1_cdc_2009.pdf> ;
        rdfs:label        "Data Revision - studies"@en ;
        qb:concept        sdmx-concept:revStudy .

sdmx-attribute:profStatCom
        a                 qb:AttributeProperty , rdf:Property ;
        rdfs:comment      "Describes the elements providing assurances that the statistical entity is entitled to comment on erroneous interpretation and misuse of statistics."@en ;
        rdfs:isDefinedBy  <http://sdmx.org/wp-content/uploads/2009/01/01_sdmx_cog_annex_1_cdc_2009.pdf> ;
        rdfs:label        "Professionalism - statistical commentary"@en ;
        qb:concept        sdmx-concept:profStatCom .

sdmx-metadata:dataUpdate
        a                 sdmx:MetadataProperty , rdf:Property ;
        rdfs:comment      "The date on which the data element was inserted or modified in the database."@en ;
        rdfs:isDefinedBy  <http://sdmx.org/wp-content/uploads/2009/01/01_sdmx_cog_annex_1_cdc_2009.pdf> ;
        rdfs:label        "Data Update"@en ;
        qb:concept        sdmx-concept:dataUpdate .

sdmx-attribute:qualityAssure
        a                 qb:AttributeProperty , rdf:Property ;
        rdfs:comment      "Guidelines focusing on quality in general and dealing with quality of statistical programmes, including measures for ensuring the efficient use of resources."@en ;
        rdfs:isDefinedBy  <http://sdmx.org/wp-content/uploads/2009/01/01_sdmx_cog_annex_1_cdc_2009.pdf> ;
        rdfs:label        "Quality Management - assurance"@en ;
        qb:concept        sdmx-concept:qualityAssure .

sdmx-attribute:profImp
        a                 qb:AttributeProperty , rdf:Property ;
        rdfs:comment      "Description of the elements providing assurances that statistics are produced on an impartial basis."@en ;
        rdfs:isDefinedBy  <http://sdmx.org/wp-content/uploads/2009/01/01_sdmx_cog_annex_1_cdc_2009.pdf> ;
        rdfs:label        "Professionalism - impartiality"@en ;
        qb:concept        sdmx-concept:profImp .

sdmx-code:timeFormat-602
        a                  skos:Concept , sdmx:Concept , sdmx-code:TimeFormat ;
        skos:definition    "(for annual series)\nyear"@en ;
        skos:inScheme      sdmx-code:timeFormat ;
        skos:notation      "602" ;
        skos:prefLabel     "CCYY"@en ;
        skos:topConceptOf  sdmx-code:timeFormat .

sdmx:reportComponent  a     rdf:Property , owl:ObjectProperty ;
        rdfs:comment        "designates a component of a report, may be a data set, data flow or nested report"@en ;
        rdfs:domain         sdmx:Report ;
        rdfs:label          "report contains"@en ;
        rdfs:range          sdmx:ReportEntry ;
        rdfs:subPropertyOf  dcterms:hasPart .

sdmx-concept:repAgency
        a                 sdmx:Concept , skos:Concept ;
        rdfs:comment      "The organisation that supplies the data for a given  instance of the statistics."@en ;
        rdfs:isDefinedBy  <http://sdmx.org/wp-content/uploads/2009/01/01_sdmx_cog_annex_1_cdc_2009.pdf> ;
        rdfs:label        "Reporting Agency"@en ;
        skos:inScheme     sdmx-concept:cog ;
        skos:notation     "urn:sdmx:org.sdmx.infomodel.conceptscheme.Concept=SDMX:CROSS_DOMAIN_CONCEPTS[1.0].REP_AGENCY" .

sdmx:AttributeProperty
        a                 rdfs:Class , owl:Class ;
        rdfs:label        "Attribute property"@en ;
        rdfs:subClassOf   sdmx:ComponentProperty , sdmx:DimensionOrAttributeProperty ;
        owl:disjointWith  sdmx:MeasureProperty .

sdmx-attribute:comparTime
        a                 qb:AttributeProperty , rdf:Property ;
        rdfs:comment      "Extent to which statistics are comparable or reconcilable over time."@en ;
        rdfs:isDefinedBy  <http://sdmx.org/wp-content/uploads/2009/01/01_sdmx_cog_annex_1_cdc_2009.pdf> ;
        rdfs:label        "Comparability - over time"@en ;
        qb:concept        sdmx-concept:comparTime .

sdmx:primaryMeasure  a  rdf:Property , owl:ObjectProperty ;
        rdfs:comment  "Indicates an additional component used as the primary measure within the SDMX data. In the case of multi-measure data sets the RDF representation uses the specific measure rather than a subsuming overall measure. This property records the subsuming primary measure (typically sdmx-measure:obsValue) to enable round tripping of this information."@en ;
        rdfs:domain   sdmx:DataStructureDefinition ;
        rdfs:label    "primary measure"@en ;
        rdfs:range    qb:MeasureProperty .

sdmx-attribute:indType
        a                 qb:AttributeProperty , rdf:Property ;
        rdfs:comment      "The type of index number used in the statistical production process."@en ;
        rdfs:isDefinedBy  <http://sdmx.org/wp-content/uploads/2009/01/01_sdmx_cog_annex_1_cdc_2009.pdf> ;
        rdfs:label        "Index Type"@en ;
        qb:concept        sdmx-concept:indType .

sdmx-concept:dataPres
        a                 sdmx:Concept , skos:Concept ;
        rdfs:comment      "Description of the disseminated data."@en ;
        rdfs:isDefinedBy  <http://sdmx.org/wp-content/uploads/2009/01/01_sdmx_cog_annex_1_cdc_2009.pdf> ;
        rdfs:label        "Data Presentation"@en ;
        skos:inScheme     sdmx-concept:cog ;
        skos:notation     "urn:sdmx:org.sdmx.infomodel.conceptscheme.Concept=SDMX:CROSS_DOMAIN_CONCEPTS[1.0].DATA_PRES" .

sdmx-dimension:refPeriod
        a                 qb:DimensionProperty , rdf:Property ;
        rdfs:comment      "The period of time or point in time to which the measured observation is intended to refer."@en ;
        rdfs:isDefinedBy  <http://sdmx.org/wp-content/uploads/2009/01/01_sdmx_cog_annex_1_cdc_2009.pdf> ;
        rdfs:label        "Reference Period"@en ;
        rdfs:range        rdfs:Resource ;
        qb:concept        sdmx-concept:refPeriod .

sdmx:metadataReport  a  rdf:Property , owl:ObjectProperty ;
        rdfs:comment  "Links a Metadata set to one or more component reports"@en ;
        rdfs:domain   sdmx:MetadataSet , sdmx:MetadataReport ;
        rdfs:label    "metadata report"@en .

sdmx-attribute:prof  a    qb:AttributeProperty , rdf:Property ;
        rdfs:comment      "The standard, skill and ability suitable for producing statistics of good quality."@en ;
        rdfs:isDefinedBy  <http://sdmx.org/wp-content/uploads/2009/01/01_sdmx_cog_annex_1_cdc_2009.pdf> ;
        rdfs:label        "Professionalism"@en ;
        qb:concept        sdmx-concept:prof .

sdmx:slice  a         rdf:Property , owl:ObjectProperty ;
        rdfs:comment  "Links a data set to a subset such as a Group, Section or TimeSeries"@en ;
        rdfs:domain   sdmx:DataSet ;
        rdfs:label    "slice"@en ;
        rdfs:range    sdmx:Slice .

sdmx-concept:coverageTime
        a                 sdmx:Concept , skos:Concept ;
        rdfs:comment      "The length of time for which data are available."@en ;
        rdfs:isDefinedBy  <http://sdmx.org/wp-content/uploads/2009/01/01_sdmx_cog_annex_1_cdc_2009.pdf> ;
        rdfs:label        "Coverage- time"@en ;
        skos:broader      sdmx-concept:coverage ;
        skos:inScheme     sdmx-concept:cog ;
        skos:notation     "urn:sdmx:org.sdmx.infomodel.conceptscheme.Concept=SDMX:CROSS_DOMAIN_CONCEPTS[1.0].COVERAGE_TIME" .

sdmx-concept:dataUpdate
        a                 sdmx:Concept , skos:Concept ;
        rdfs:comment      "The date on which the data element was inserted or modified in the database."@en ;
        rdfs:isDefinedBy  <http://sdmx.org/wp-content/uploads/2009/01/01_sdmx_cog_annex_1_cdc_2009.pdf> ;
        rdfs:label        "Data Update"@en ;
        skos:inScheme     sdmx-concept:cog ;
        skos:notation     "urn:sdmx:org.sdmx.infomodel.conceptscheme.Concept=SDMX:CROSS_DOMAIN_CONCEPTS[1.0].DATA_UPDATE" .

sdmx-metadata:qualityAssure
        a                 sdmx:MetadataProperty , rdf:Property ;
        rdfs:comment      "Guidelines focusing on quality in general and dealing with quality of statistical programmes, including measures for ensuring the efficient use of resources."@en ;
        rdfs:isDefinedBy  <http://sdmx.org/wp-content/uploads/2009/01/01_sdmx_cog_annex_1_cdc_2009.pdf> ;
        rdfs:label        "Quality Management - assurance"@en ;
        qb:concept        sdmx-concept:qualityAssure .

sdmx-attribute:relevance
        a                 qb:AttributeProperty , rdf:Property ;
        rdfs:comment      "The degree to which statistical information meets the real or perceived needs of clients."@en ;
        rdfs:isDefinedBy  <http://sdmx.org/wp-content/uploads/2009/01/01_sdmx_cog_annex_1_cdc_2009.pdf> ;
        rdfs:label        "Relevance"@en ;
        qb:concept        sdmx-concept:relevance .

sdmx-subject:2  a          skos:Concept , sdmx:Concept , sdmx-subject:SubjectMatterDomain ;
        skos:definition    ""@en ;
        skos:notation      "2" ;
        skos:prefLabel     "Economic statistics"@en ;
        skos:topConceptOf  sdmx-subject:subjectMatterDomain .

sdmx-concept:profMeth
        a                 sdmx:Concept , skos:Concept ;
        rdfs:comment      "Describes the elements providing assurances that the choices of sources and statistical techniques as well as decisions about dissemination are informed solely by statistical considerations."@en ;
        rdfs:isDefinedBy  <http://sdmx.org/wp-content/uploads/2009/01/01_sdmx_cog_annex_1_cdc_2009.pdf> ;
        rdfs:label        "Professionalism - methodology"@en ;
        skos:broader      sdmx-concept:prof ;
        skos:inScheme     sdmx-concept:cog ;
        skos:notation     "urn:sdmx:org.sdmx.infomodel.conceptscheme.Concept=SDMX:CROSS_DOMAIN_CONCEPTS[1.0].PROF_METH" .

sdmx-metadata:contactOrganisation
        a                   sdmx:MetadataProperty , rdf:Property ;
        rdfs:comment        "The name of the organisation of the contact points for the data or metadata."@en ;
        rdfs:isDefinedBy    <http://sdmx.org/wp-content/uploads/2009/01/01_sdmx_cog_annex_1_cdc_2009.pdf> ;
        rdfs:label          "Contact organisation"@en ;
        rdfs:subPropertyOf  vcard:organization-name ;
        qb:concept          sdmx-concept:contactOrganisation .

sdmx-metadata:profMeth
        a                 sdmx:MetadataProperty , rdf:Property ;
        rdfs:comment      "Describes the elements providing assurances that the choices of sources and statistical techniques as well as decisions about dissemination are informed solely by statistical considerations."@en ;
        rdfs:isDefinedBy  <http://sdmx.org/wp-content/uploads/2009/01/01_sdmx_cog_annex_1_cdc_2009.pdf> ;
        rdfs:label        "Professionalism - methodology"@en ;
        qb:concept        sdmx-concept:profMeth .

sdmx-metadata:repAgency
        a                 sdmx:MetadataProperty , rdf:Property ;
        rdfs:comment      "The organisation that supplies the data for a given  instance of the statistics."@en ;
        rdfs:isDefinedBy  <http://sdmx.org/wp-content/uploads/2009/01/01_sdmx_cog_annex_1_cdc_2009.pdf> ;
        rdfs:label        "Reporting Agency"@en ;
        qb:concept        sdmx-concept:repAgency .

sdmx-code:freq-W  a        skos:Concept , sdmx:Concept , sdmx-code:Freq ;
        skos:inScheme      sdmx-code:freq ;
        skos:notation      "W" ;
        skos:prefLabel     "Weekly"@en ;
        skos:topConceptOf  sdmx-code:freq .

sdmx-concept:adjustCoded
        a                 sdmx:Concept , skos:Concept ;
        rdfs:comment      "Type of adjustment used, represented by a code."@en ;
        rdfs:isDefinedBy  <http://sdmx.org/wp-content/uploads/2009/01/01_sdmx_cog_annex_1_cdc_2009.pdf> ;
        rdfs:label        "Adjustment - coded"@en ;
        skos:broader      sdmx-concept:adjustment ;
        skos:inScheme     sdmx-concept:cog ;
        skos:notation     "urn:sdmx:org.sdmx.infomodel.conceptscheme.Concept=SDMX:CROSS_DOMAIN_CONCEPTS[1.0].ADJUST_CODED" .

sdmx-concept:dataValidation
        a                 sdmx:Concept , skos:Concept ;
        rdfs:comment      "Process of monitoring the results of data compilation and ensuring the quality of the statistical results."@en ;
        rdfs:isDefinedBy  <http://sdmx.org/wp-content/uploads/2009/01/01_sdmx_cog_annex_1_cdc_2009.pdf> ;
        rdfs:label        "Data Validation"@en ;
        skos:inScheme     sdmx-concept:cog ;
        skos:notation     "urn:sdmx:org.sdmx.infomodel.conceptscheme.Concept=SDMX:CROSS_DOMAIN_CONCEPTS[1.0].DATA_VALIDATION" .

sdmx-code:timeFormat-P3M
        a                  skos:Concept , sdmx:Concept , sdmx-code:TimeFormat ;
        skos:inScheme      sdmx-code:timeFormat ;
        skos:notation      "P3M" ;
        skos:prefLabel     "Quarterly"@en ;
        skos:topConceptOf  sdmx-code:timeFormat .

eg:slice2  a                qb:Slice ;
        eg:refPeriod        <http://reference.data.gov.uk/id/gregorian-interval/2004-01-01T00:00:00/P3Y> ;
        qb:observation      eg:o21 , eg:o22 , eg:o23 , eg:o24 ;
        qb:sliceStructure   eg:sliceByRegion ;
        sdmx-dimension:sex  sdmx-code:sex-F .

sdmx:MandatoryAttributeProperty
        a                rdfs:Class , owl:Class ;
        rdfs:label       "Mandatory attribute property"@en ;
        rdfs:subClassOf  sdmx:AttributeProperty .

sdmx-subject:2.4.4  a    skos:Concept , sdmx:Concept , sdmx-subject:SubjectMatterDomain ;
        skos:broader     sdmx-subject:2.4 ;
        skos:definition  "Transport - covers statistics on all modes of transport (air, rail, road, inland waterways, sea), includes topics like transport infrastructure, equipment, traffic flows, personal mobility, safety, energy consumption, transport enterprises, passengers and freight transport, transport sector trends, road traffic accidents.\nExcludes\n- transport prices (2.7)"@en ;
        skos:notation    "2.4.4" ;
        skos:prefLabel   "Transport"@en .

sdmx-attribute:comment
        a                 qb:AttributeProperty , rdf:Property ;
        rdfs:comment      "Supplementary descriptive text which can be attached to data or metadata."@en ;
        rdfs:isDefinedBy  <http://sdmx.org/wp-content/uploads/2009/01/01_sdmx_cog_annex_1_cdc_2009.pdf> ;
        rdfs:label        "Comment"@en ;
        qb:concept        sdmx-concept:comment .

sdmx-concept:relPolicy
        a                 sdmx:Concept , skos:Concept ;
        rdfs:comment      "Rules for disseminating statistical data to interested parties."@en ;
        rdfs:isDefinedBy  <http://sdmx.org/wp-content/uploads/2009/01/01_sdmx_cog_annex_1_cdc_2009.pdf> ;
        rdfs:label        "Release Policy"@en ;
        skos:inScheme     sdmx-concept:cog ;
        skos:notation     "urn:sdmx:org.sdmx.infomodel.conceptscheme.Concept=SDMX:CROSS_DOMAIN_CONCEPTS[1.0].REL_POLICY" .

sdmx-subject:1.5  a      skos:Concept , sdmx:Concept , sdmx-subject:SubjectMatterDomain ;
        skos:broader     sdmx-subject:1 ;
        skos:definition  "Income and consumption - covers statistics on household income and expenditures from household viewpoint (all types of income and expenditure), including topics like distribution of incomes, in-kind income, income transfers received and paid, income- or expenditure-based measures of poverty, consumer protection, consumption patterns, consumer goods and durables, household wealth and debts.\nExcludes \n- social protection schemes against various risks (1.6)\n- tax schemes (2.5)\n- poverty in a multidimensional sense (3.3.1) \n- living conditions (3.3.1)\n- social inclusion/exclusion (3.3.1)"@en ;
        skos:notation    "1.5" ;
        skos:prefLabel   "Income and consumption"@en .

sdmx:effectiveDate  a       rdf:Property , owl:DatatypeProperty ;
        rdfs:comment        "The date on which all the effectiveDate metadata in the metadata set is effective."@en ;
        rdfs:label          "effective date"@en ;
        rdfs:range          xsd:dateTime ;
        rdfs:subPropertyOf  dcterms:date .

sdmx-concept:confPolicy
        a                 sdmx:Concept , skos:Concept ;
        rdfs:comment      "Legislative measures or other formal procedures which prevent unauthorised disclosure of data that identify a person or economic entity either directly or indirectly."@en ;
        rdfs:isDefinedBy  <http://sdmx.org/wp-content/uploads/2009/01/01_sdmx_cog_annex_1_cdc_2009.pdf> ;
        rdfs:label        "Confidentiality - policy"@en ;
        skos:broader      sdmx-concept:conf ;
        skos:inScheme     sdmx-concept:cog ;
        skos:notation     "urn:sdmx:org.sdmx.infomodel.conceptscheme.Concept=SDMX:CROSS_DOMAIN_CONCEPTS[1.0].CONF_POLICY" .

sdmx-metadata:refPerWgts
        a                 sdmx:MetadataProperty , rdf:Property ;
        rdfs:comment      "Dates or periods to which the observations used to compile the weights refer."@en ;
        rdfs:isDefinedBy  <http://sdmx.org/wp-content/uploads/2009/01/01_sdmx_cog_annex_1_cdc_2009.pdf> ;
        rdfs:label        "Reference Period - weights"@en ;
        qb:concept        sdmx-concept:refPerWgts .

sdmx-concept:profCond
        a                 sdmx:Concept , skos:Concept ;
        rdfs:comment      "Provision for assuring the qualifications of staff and allowing staff to perform their functions without intervention motivated by non-statistical objectives."@en ;
        rdfs:isDefinedBy  <http://sdmx.org/wp-content/uploads/2009/01/01_sdmx_cog_annex_1_cdc_2009.pdf> ;
        rdfs:label        "Professionalism - code of conduct"@en ;
        skos:broader      sdmx-concept:prof ;
        skos:inScheme     sdmx-concept:cog ;
        skos:notation     "urn:sdmx:org.sdmx.infomodel.conceptscheme.Concept=SDMX:CROSS_DOMAIN_CONCEPTS[1.0].PROF_COND" .

sdmx-code:timeFormat-716
        a                  skos:Concept , sdmx:Concept , sdmx-code:TimeFormat ;
        skos:definition    "(for weekly series)\nfrom year/week to year/week"@en ;
        skos:inScheme      sdmx-code:timeFormat ;
        skos:notation      "716" ;
        skos:prefLabel     "CCYYWWCCYYWW"@en ;
        skos:topConceptOf  sdmx-code:timeFormat .

sdmx-attribute:timePerCollect
        a                 qb:AttributeProperty , rdf:Property ;
        rdfs:comment      "Dates or periods during which the observations have been collected (such as middle, average or end of period) to compile the indicator for the target reference period."@en ;
        rdfs:isDefinedBy  <http://sdmx.org/wp-content/uploads/2009/01/01_sdmx_cog_annex_1_cdc_2009.pdf> ;
        rdfs:label        "Time Period - collection"@en ;
        qb:concept        sdmx-concept:timePerCollect .

sdmx-metadata:relCalPolicy
        a                 sdmx:MetadataProperty , rdf:Property ;
        rdfs:comment      "The schedule of statistical release dates."@en ;
        rdfs:isDefinedBy  <http://sdmx.org/wp-content/uploads/2009/01/01_sdmx_cog_annex_1_cdc_2009.pdf> ;
        rdfs:label        "Release Policy - release calendar"@en ;
        qb:concept        sdmx-concept:relCalPolicy .

sdmx-attribute:relCalPolicy
        a                 qb:AttributeProperty , rdf:Property ;
        rdfs:comment      "The schedule of statistical release dates."@en ;
        rdfs:isDefinedBy  <http://sdmx.org/wp-content/uploads/2009/01/01_sdmx_cog_annex_1_cdc_2009.pdf> ;
        rdfs:label        "Release Policy - release calendar"@en ;
        qb:concept        sdmx-concept:relCalPolicy .

sdmx-metadata:contactFax
        a                   sdmx:MetadataProperty , rdf:Property ;
        rdfs:comment        "Fax number of the contact points for the data or metadata."@en ;
        rdfs:isDefinedBy    <http://sdmx.org/wp-content/uploads/2009/01/01_sdmx_cog_annex_1_cdc_2009.pdf> ;
        rdfs:label          "Contact fax number"@en ;
        rdfs:subPropertyOf  vcard:fax ;
        qb:concept          sdmx-concept:contactFax .

sdmx:metadata  a      rdf:Property , owl:ObjectProperty ;
        rdfs:comment  "Links an entity (from Observation up to DataFlow) to a corresponding metadata record."@en ;
        rdfs:label    "metadata"@en ;
        rdfs:range    sdmx:MetadataSet .

sdmx-code:freq-A  a        skos:Concept , sdmx:Concept , sdmx-code:Freq ;
        skos:definition    "It is typically used for annual data. This can also serve cases of multi-annual data (data that appear once every two, three or, possibly, five years).  Descriptive information on the multiannual characteristics (e.g. frequency of the series in practice and other methodological information can be provided at the dataflow level, as long as these characteristics are applicable for the entire dataflow)."@en ;
        skos:inScheme      sdmx-code:freq ;
        skos:notation      "A" ;
        skos:prefLabel     "Annual"@en ;
        skos:topConceptOf  sdmx-code:freq .

eg:o52  a                  qb:Observation ;
        eg:lifeExpectancy  78.7 ;
        eg:refArea         ex-geo:cardiff_00pt ;
        qb:dataSet         eg:dataset-le3 .

sdmx-subject:2.6  a      skos:Concept , sdmx:Concept , sdmx-subject:SubjectMatterDomain ;
        skos:broader     sdmx-subject:2 ;
        skos:definition  "International trade and balance of payments - deals with statistics on all cross-border transactions recorded in the balance of payments, includes topics like trade in goods and services, external positions and debt, foreign direct investment, foreign affiliated trade, tariffs, market access, foreign aid, development assistance, resource flows to developing countries.\nExcludes: \n- trade in specific commodities/services mentioned in 2.4.1 to 2.4.5\n- multinational companies and activities of foreign affiliates (3.3.4)"@en ;
        skos:notation    "2.6" ;
        skos:prefLabel   "International trade and balance of payments"@en .

sdmx-concept:profStatCom
        a                 sdmx:Concept , skos:Concept ;
        rdfs:comment      "Describes the elements providing assurances that the statistical entity is entitled to comment on erroneous interpretation and misuse of statistics."@en ;
        rdfs:isDefinedBy  <http://sdmx.org/wp-content/uploads/2009/01/01_sdmx_cog_annex_1_cdc_2009.pdf> ;
        rdfs:label        "Professionalism - statistical commentary"@en ;
        skos:broader      sdmx-concept:prof ;
        skos:inScheme     sdmx-concept:cog ;
        skos:notation     "urn:sdmx:org.sdmx.infomodel.conceptscheme.Concept=SDMX:CROSS_DOMAIN_CONCEPTS[1.0].PROF_STAT_COM" .

sdmx-concept:samplingErr
        a                 sdmx:Concept , skos:Concept ;
        rdfs:comment      "That part of the difference between a population value and an estimate thereof, derived from a random sample, which is due to the fact that only a subset of the population is enumerated."@en ;
        rdfs:isDefinedBy  <http://sdmx.org/wp-content/uploads/2009/01/01_sdmx_cog_annex_1_cdc_2009.pdf> ;
        rdfs:label        "Accuracy - sampling error"@en ;
        skos:broader      sdmx-concept:accuracy ;
        skos:inScheme     sdmx-concept:cog ;
        skos:notation     "urn:sdmx:org.sdmx.infomodel.conceptscheme.Concept=SDMX:CROSS_DOMAIN_CONCEPTS[1.0].SAMPLING_ERR" .

sdmx:measureTypeConcept
        a             sdmx:MeasureTypeRole , sdmx:ConceptRole , skos:Concept ;
        rdfs:comment  "The concept corresponding to the generic measure type dimension which indicates which measure is being denoted by the primary measure on an observation"@en ;
        rdfs:label    "measureType"@en .

sdmx-metadata:metaLastUpdate
        a                 sdmx:MetadataProperty , rdf:Property ;
        rdfs:comment      "Date of last update of the content of the metadata."@en ;
        rdfs:isDefinedBy  <http://sdmx.org/wp-content/uploads/2009/01/01_sdmx_cog_annex_1_cdc_2009.pdf> ;
        rdfs:label        "Metadata Update - last update"@en ;
        qb:concept        sdmx-concept:metaLastUpdate .

sdmx-attribute:contactFunct
        a                 qb:AttributeProperty , rdf:Property ;
        rdfs:comment      "The area of technical responsibility of the contact, such as \"methodology\", \"database management\" or \"dissemination\"."@en ;
        rdfs:isDefinedBy  <http://sdmx.org/wp-content/uploads/2009/01/01_sdmx_cog_annex_1_cdc_2009.pdf> ;
        rdfs:label        "Contact person job title"@en ;
        qb:concept        sdmx-concept:contactFunct .

sdmx-attribute:confStatus
        a                 qb:AttributeProperty , rdf:Property , qb:CodedProperty ;
        rdfs:comment      "Information about the confidentiality status of the object to which this attribute is attached."@en ;
        rdfs:isDefinedBy  <http://sdmx.org/wp-content/uploads/2009/01/01_sdmx_cog_annex_1_cdc_2009.pdf> ;
        rdfs:label        "Confidentiality - status"@en ;
        rdfs:range        sdmx-code:ConfStatus ;
        qb:codeList       sdmx-code:confStatus ;
        qb:concept        sdmx-concept:confStatus .

sdmx-concept:contactFunct
        a                 sdmx:Concept , skos:Concept ;
        rdfs:comment      "The area of technical responsibility of the contact, such as \"methodology\", \"database management\" or \"dissemination\"."@en ;
        rdfs:isDefinedBy  <http://sdmx.org/wp-content/uploads/2009/01/01_sdmx_cog_annex_1_cdc_2009.pdf> ;
        rdfs:label        "Contact person job title"@en ;
        skos:broader      sdmx-concept:contact ;
        skos:inScheme     sdmx-concept:cog ;
        skos:notation     "urn:sdmx:org.sdmx.infomodel.conceptscheme.Concept=SDMX:CROSS_DOMAIN_CONCEPTS[1.0].CONTACT_FUNCT" .

sdmx-concept:dsi  a       sdmx:Concept , skos:Concept ;
        rdfs:comment      "Sequence of characters identifying the data set with which it is associated."@en ;
        rdfs:isDefinedBy  <http://sdmx.org/wp-content/uploads/2009/01/01_sdmx_cog_annex_1_cdc_2009.pdf> ;
        rdfs:label        "Data Set Identifier"@en ;
        skos:inScheme     sdmx-concept:cog ;
        skos:notation     "urn:sdmx:org.sdmx.infomodel.conceptscheme.Concept=SDMX:CROSS_DOMAIN_CONCEPTS[1.0].DSI" .

sdmx-attribute:coherInternal
        a                 qb:AttributeProperty , rdf:Property ;
        rdfs:comment      "Extent to which statistics are consistent within a given data set."@en ;
        rdfs:isDefinedBy  <http://sdmx.org/wp-content/uploads/2009/01/01_sdmx_cog_annex_1_cdc_2009.pdf> ;
        rdfs:label        "Coherence - Internal"@en ;
        qb:concept        sdmx-concept:coherInternal .

sdmx-attribute:obsStatus
        a                 qb:AttributeProperty , rdf:Property , qb:CodedProperty ;
        rdfs:comment      "Information on the quality of a value or an unusual or missing value."@en ;
        rdfs:isDefinedBy  <http://sdmx.org/wp-content/uploads/2009/01/01_sdmx_cog_annex_1_cdc_2009.pdf> ;
        rdfs:label        "Observation Status"@en ;
        rdfs:range        sdmx-code:ObsStatus ;
        qb:codeList       sdmx-code:obsStatus ;
        qb:concept        sdmx-concept:obsStatus .

sdmx-concept:recording
        a                 sdmx:Concept , skos:Concept ;
        rdfs:comment      "Processes and standards employed in calculating statistical aggregates."@en ;
        rdfs:isDefinedBy  <http://sdmx.org/wp-content/uploads/2009/01/01_sdmx_cog_annex_1_cdc_2009.pdf> ;
        rdfs:label        "Recording Basis"@en ;
        skos:inScheme     sdmx-concept:cog ;
        skos:notation     "urn:sdmx:org.sdmx.infomodel.conceptscheme.Concept=SDMX:CROSS_DOMAIN_CONCEPTS[1.0].RECORDING" .

sdmx-code:timeFormat-610
        a                  skos:Concept , sdmx:Concept , sdmx-code:TimeFormat ;
        skos:definition    "(for monthly series)\nyear/month"@en ;
        skos:inScheme      sdmx-code:timeFormat ;
        skos:notation      "610" ;
        skos:prefLabel     "CCYYMM"@en ;
        skos:topConceptOf  sdmx-code:timeFormat .

sdmx-metadata:relPolicy
        a                 sdmx:MetadataProperty , rdf:Property ;
        rdfs:comment      "Rules for disseminating statistical data to interested parties."@en ;
        rdfs:isDefinedBy  <http://sdmx.org/wp-content/uploads/2009/01/01_sdmx_cog_annex_1_cdc_2009.pdf> ;
        rdfs:label        "Release Policy"@en ;
        qb:concept        sdmx-concept:relPolicy .

sdmx-attribute:statPop
        a                 qb:AttributeProperty , rdf:Property ;
        rdfs:comment      "The total membership or population or \"universe\" of a defined class of people, objects or events."@en ;
        rdfs:isDefinedBy  <http://sdmx.org/wp-content/uploads/2009/01/01_sdmx_cog_annex_1_cdc_2009.pdf> ;
        rdfs:label        "Statistical Population"@en ;
        qb:concept        sdmx-concept:statPop .

sdmx-metadata:revStudy
        a                 sdmx:MetadataProperty , rdf:Property ;
        rdfs:comment      "Information about data revision studies and analyses."@en ;
        rdfs:isDefinedBy  <http://sdmx.org/wp-content/uploads/2009/01/01_sdmx_cog_annex_1_cdc_2009.pdf> ;
        rdfs:label        "Data Revision - studies"@en ;
        qb:concept        sdmx-concept:revStudy .

sdmx-attribute:timeliness
        a                 qb:AttributeProperty , rdf:Property ;
        rdfs:comment      "Length of time between data availability and the event or phenomenon they describe."@en ;
        rdfs:isDefinedBy  <http://sdmx.org/wp-content/uploads/2009/01/01_sdmx_cog_annex_1_cdc_2009.pdf> ;
        rdfs:label        "Timelinesst"@en ;
        qb:concept        sdmx-concept:timeliness .

sdmx-subject:3.3.3  a    skos:Concept , sdmx:Concept , sdmx-subject:SubjectMatterDomain ;
        skos:broader     sdmx-subject:3.3 ;
        skos:definition  "Information society - statistics allowing to assess the use and impact of information and communication technologies on society, includes access and use of ICTs (including Internet), ICT expenditure and investment, ICT infrastructure, telecommunication networks, electronic communications, e-government, electronic commerce, e-learning, broadband penetration, ICT services, communication tariffs, network infrastructure, revenues, expenses and investment of operators, Internet indicators, trade in telecommunications equipment."@en ;
        skos:notation    "3.3.3" ;
        skos:prefLabel   "Information society"@en .

sdmx-concept:contactFax
        a                 sdmx:Concept , skos:Concept ;
        rdfs:comment      "Fax number of the contact points for the data or metadata."@en ;
        rdfs:isDefinedBy  <http://sdmx.org/wp-content/uploads/2009/01/01_sdmx_cog_annex_1_cdc_2009.pdf> ;
        rdfs:label        "Contact fax number"@en ;
        skos:broader      sdmx-concept:contact ;
        skos:inScheme     sdmx-concept:cog ;
        skos:notation     "urn:sdmx:org.sdmx.infomodel.conceptscheme.Concept=SDMX:CROSS_DOMAIN_CONCEPTS[1.0].CONTACT_FAX" .

sdmx-concept:obsValue
        a                 sdmx:Concept , skos:Concept , sdmx:PrimaryMeasureRole ;
        rdfs:comment      "The value of a particular variable at a particular period."@en ;
        rdfs:isDefinedBy  <http://sdmx.org/wp-content/uploads/2009/01/01_sdmx_cog_annex_1_cdc_2009.pdf> ;
        rdfs:label        "Observation"@en ;
        skos:inScheme     sdmx-concept:cog ;
        skos:notation     "urn:sdmx:org.sdmx.infomodel.conceptscheme.Concept=SDMX:CROSS_DOMAIN_CONCEPTS[1.0].OBS_VALUE" .

sdmx:Flow  a             rdfs:Class , owl:Class ;
        rdfs:comment     "Abstract information flow, can be either data or metadata"@en ;
        rdfs:label       "Flow"@en ;
        rdfs:subClassOf  sdmx:Structured .

sdmx:CountRole  a        rdfs:Class , owl:Class ;
        rdfs:comment     "concept for a dimension or attribute that plays the role of an identifier where the identifier is taken from a known system of counts (e.g. the Nth current dataset update for a given day)"@en ;
        rdfs:label       "Count property"@en ;
        rdfs:subClassOf  sdmx:ConceptRole .

sdmx-concept:advNotice
        a                 sdmx:Concept , skos:Concept ;
        rdfs:comment      "Policy on notifying the public of changes in methodology, indicating whether the public is notified before a methodological change affects disseminated data and, if so, how long before."@en ;
        rdfs:isDefinedBy  <http://sdmx.org/wp-content/uploads/2009/01/01_sdmx_cog_annex_1_cdc_2009.pdf> ;
        rdfs:label        "Documentation on methodology - advance notice"@en ;
        skos:broader      sdmx-concept:docMethod ;
        skos:inScheme     sdmx-concept:cog ;
        skos:notation     "urn:sdmx:org.sdmx.infomodel.conceptscheme.Concept=SDMX:CROSS_DOMAIN_CONCEPTS[1.0].ADV_NOTICE" .

sdmx-concept:comparability
        a                 sdmx:Concept , skos:Concept ;
        rdfs:comment      "The extent to which differences between statistics can be attributed to differences between the true values of the statistical characteristics."@en ;
        rdfs:isDefinedBy  <http://sdmx.org/wp-content/uploads/2009/01/01_sdmx_cog_annex_1_cdc_2009.pdf> ;
        rdfs:label        "Comparability"@en ;
        skos:inScheme     sdmx-concept:cog ;
        skos:notation     "urn:sdmx:org.sdmx.infomodel.conceptscheme.Concept=SDMX:CROSS_DOMAIN_CONCEPTS[1.0].COMPARABILITY" .

sdmx-metadata:obsValue
        a                 sdmx:MetadataProperty , rdf:Property ;
        rdfs:comment      "The value of a particular variable at a particular period."@en ;
        rdfs:isDefinedBy  <http://sdmx.org/wp-content/uploads/2009/01/01_sdmx_cog_annex_1_cdc_2009.pdf> ;
        rdfs:label        "Observation"@en ;
        qb:concept        sdmx-concept:obsValue .

sdmx-metadata:docMethod
        a                 sdmx:MetadataProperty , rdf:Property ;
        rdfs:comment      "Descriptive text and references to methodological documents available."@en ;
        rdfs:isDefinedBy  <http://sdmx.org/wp-content/uploads/2009/01/01_sdmx_cog_annex_1_cdc_2009.pdf> ;
        rdfs:label        "Documentation on methodology"@en ;
        qb:concept        sdmx-concept:docMethod .

sdmx:component  a    rdf:Property , owl:ObjectProperty ;
        rdfs:domain  sdmx:DataStructureDefinition , sdmx:Structure ;
        rdfs:label   "component"@en ;
        rdfs:range   sdmx:ComponentProperty .

sdmx-code:timeFormat-PT1M
        a                  skos:Concept , sdmx:Concept , sdmx-code:TimeFormat ;
        skos:inScheme      sdmx-code:timeFormat ;
        skos:notation      "PT1M" ;
        skos:prefLabel     "Minutely"@en ;
        skos:topConceptOf  sdmx-code:timeFormat .

sdmx-attribute:coverageSector
        a                 qb:AttributeProperty , rdf:Property ;
        rdfs:comment      "Main economic or other sectors covered by the statistics."@en ;
        rdfs:isDefinedBy  <http://sdmx.org/wp-content/uploads/2009/01/01_sdmx_cog_annex_1_cdc_2009.pdf> ;
        rdfs:label        "Coverage - sector"@en ;
        qb:concept        sdmx-concept:coverageSector .

sdmx-attribute:relComment
        a                 qb:AttributeProperty , rdf:Property ;
        rdfs:comment      "Legal acts and other agreements pertaining to data access."@en ;
        rdfs:isDefinedBy  <http://sdmx.org/wp-content/uploads/2009/01/01_sdmx_cog_annex_1_cdc_2009.pdf> ;
        rdfs:label        "Release Policy - policy commentary"@en ;
        qb:concept        sdmx-concept:relComment .

sdmx-attribute:adjustment
        a                 qb:AttributeProperty , rdf:Property ;
        rdfs:comment      "The set of procedures employed to modify statistical data to enable it to conform to national or international standards or to address data quality differences when compiling specific data sets."@en ;
        rdfs:isDefinedBy  <http://sdmx.org/wp-content/uploads/2009/01/01_sdmx_cog_annex_1_cdc_2009.pdf> ;
        rdfs:label        "Adjustment"@en ;
        qb:concept        sdmx-concept:adjustment .

sdmx-metadata:coherInternal
        a                 sdmx:MetadataProperty , rdf:Property ;
        rdfs:comment      "Extent to which statistics are consistent within a given data set."@en ;
        rdfs:isDefinedBy  <http://sdmx.org/wp-content/uploads/2009/01/01_sdmx_cog_annex_1_cdc_2009.pdf> ;
        rdfs:label        "Coherence - Internal"@en ;
        qb:concept        sdmx-concept:coherInternal .

sdmx-attribute:sampling
        a                 qb:AttributeProperty , rdf:Property ;
        rdfs:comment      "The process of selecting a number of cases from all the cases in a particular group or universe."@en ;
        rdfs:isDefinedBy  <http://sdmx.org/wp-content/uploads/2009/01/01_sdmx_cog_annex_1_cdc_2009.pdf> ;
        rdfs:label        "Sampling"@en ;
        qb:concept        sdmx-concept:sampling .

sdmx-code:confStatus-S
        a                  skos:Concept , sdmx:Concept , sdmx-code:ConfStatus ;
        skos:definition    "If senders do not manage the secondary confidentiality in their data and/or there are also other countries' data involved (with the intention to eventually compile a regional-wide aggregate that is going to be published), the value \"S\" is used by the receiver to flag additional suppressed observations (within sender's data and/or within the datasets of other senders) in subsequent stages of processing (especially, dissemination) in order to prevent third parties to indirectly deduct the observations that were genuinely flagged with \"C\" by the sender."@en ;
        skos:inScheme      sdmx-code:confStatus ;
        skos:notation      "S" ;
        skos:prefLabel     "Secondary confidentiality set and managed by the receiver, not for publication"@en ;
        skos:topConceptOf  sdmx-code:confStatus .

sdmx-code:timeFormat-711
        a                  skos:Concept , sdmx:Concept , sdmx-code:TimeFormat ;
        skos:definition    "(for daily and business series)\nfrom year/month/day to year/month/day"@en ;
        skos:inScheme      sdmx-code:timeFormat ;
        skos:notation      "711" ;
        skos:prefLabel     "CCYYMMDDCCYYMMDD"@en ;
        skos:topConceptOf  sdmx-code:timeFormat .

sdmx-metadata:publications
        a                 sdmx:MetadataProperty , rdf:Property ;
        rdfs:comment      "Regular or ad-hoc publications in which the data are made available to the public."@en ;
        rdfs:isDefinedBy  <http://sdmx.org/wp-content/uploads/2009/01/01_sdmx_cog_annex_1_cdc_2009.pdf> ;
        rdfs:label        "Dissemination Format - publications"@en ;
        qb:concept        sdmx-concept:publications .

sdmx-concept:profImp  a   sdmx:Concept , skos:Concept ;
        rdfs:comment      "Description of the elements providing assurances that statistics are produced on an impartial basis."@en ;
        rdfs:isDefinedBy  <http://sdmx.org/wp-content/uploads/2009/01/01_sdmx_cog_annex_1_cdc_2009.pdf> ;
        rdfs:label        "Professionalism - impartiality"@en ;
        skos:broader      sdmx-concept:prof ;
        skos:inScheme     sdmx-concept:cog ;
        skos:notation     "urn:sdmx:org.sdmx.infomodel.conceptscheme.Concept=SDMX:CROSS_DOMAIN_CONCEPTS[1.0].PROF_IMP" .

eg:refPeriod  a             rdf:Property , qb:DimensionProperty ;
        rdfs:label          "reference period"@en ;
        rdfs:range          interval:Interval ;
        rdfs:subPropertyOf  sdmx-dimension:refPeriod ;
        qb:concept          sdmx-concept:refPeriod .

sdmx-attribute:publications
        a                 qb:AttributeProperty , rdf:Property ;
        rdfs:comment      "Regular or ad-hoc publications in which the data are made available to the public."@en ;
        rdfs:isDefinedBy  <http://sdmx.org/wp-content/uploads/2009/01/01_sdmx_cog_annex_1_cdc_2009.pdf> ;
        rdfs:label        "Dissemination Format - publications"@en ;
        qb:concept        sdmx-concept:publications .

<http://purl.org/linked-data/sdmx>
        a                    owl:Ontology ;
        rdfs:comment         "This vocabulary extends the data cube vocabulary to support publication of statistical data in RDF, using an information model based on SDMX" , "This vocabulary allows statistical data to be published in RDF, using an information model based on SDMX" ;
        rdfs:label           "SDMX-RDF vocabulary" ;
        dcterms:contributor  [ foaf:mbox  "richard@cyganiak.de" ] ;
        dcterms:contributor  [ foaf:mbox  "ian@epimorphics.com" ] ;
        dcterms:contributor  [ foaf:mbox  "dave@epimorphics.com" ] ;
        dcterms:contributor  [ foaf:mbox  "ian@epimorphics.com" ] ;
        dcterms:contributor  [ foaf:mbox  "jeni@jenitennison.com" ] ;
        dcterms:contributor  [ foaf:mbox  "jeni@jenitennison.com" ] ;
        dcterms:contributor  [ foaf:mbox  "arofan.gregory@earthlink.net" ] ;
        dcterms:contributor  [ foaf:mbox  "arofan.gregory@earthlink.net" ] ;
        dcterms:contributor  [ foaf:mbox  "dave@epimorphics.com" ] ;
        dcterms:contributor  [ foaf:mbox  "richard@cyganiak.de" ] ;
        dcterms:created      "2010-02-05"^^xsd:date ;
        dcterms:modified     "2010-04-07"^^xsd:date , "2010-07-22"^^xsd:date ;
        dcterms:references   <http://sdmx.org/?page_id=16#package> ;
        dcterms:source       <http://sdmx.org> ;
        dcterms:title        "Vocabulary for publishing SDMX statistical data in RDF" ;
        owl:versionInfo      "0.3" , "0.2" .

eg:o33  a                  qb:Observation ;
        eg:lifeExpectancy  76.5 ;
        eg:refArea         ex-geo:monmouthshire_00pp ;
        qb:dataSet         eg:dataset-le3 .

sdmx-dimension:educationLev
        a                 qb:DimensionProperty , rdf:Property ;
        rdfs:comment      "The highest level of an educational programme the person has successfully completed."@en ;
        rdfs:isDefinedBy  <http://sdmx.org/wp-content/uploads/2009/01/01_sdmx_cog_annex_1_cdc_2009.pdf> ;
        rdfs:label        "Education Level"@en ;
        rdfs:range        rdfs:Resource ;
        qb:concept        sdmx-concept:educationLev .

sdmx-concept:indType  a   sdmx:Concept , skos:Concept ;
        rdfs:comment      "The type of index number used in the statistical production process."@en ;
        rdfs:isDefinedBy  <http://sdmx.org/wp-content/uploads/2009/01/01_sdmx_cog_annex_1_cdc_2009.pdf> ;
        rdfs:label        "Index Type"@en ;
        skos:inScheme     sdmx-concept:cog ;
        skos:notation     "urn:sdmx:org.sdmx.infomodel.conceptscheme.Concept=SDMX:CROSS_DOMAIN_CONCEPTS[1.0].IND_TYPE" .

sdmx:metadataReportStructure
        a             rdf:Property , owl:ObjectProperty ;
        rdfs:comment  "designates a single report structure within an overall metadata structure definition"@en ;
        rdfs:domain   sdmx:MetadataStructureDefinition ;
        rdfs:label    "metadata report structure"@en ;
        rdfs:range    sdmx:MetadataReportStructure .

sdmx-metadata:recording
        a                 sdmx:MetadataProperty , rdf:Property ;
        rdfs:comment      "Processes and standards employed in calculating statistical aggregates."@en ;
        rdfs:isDefinedBy  <http://sdmx.org/wp-content/uploads/2009/01/01_sdmx_cog_annex_1_cdc_2009.pdf> ;
        rdfs:label        "Recording Basis"@en ;
        qb:concept        sdmx-concept:recording .

sdmx-subject:2.1  a      skos:Concept , sdmx:Concept , sdmx-subject:SubjectMatterDomain ;
        skos:broader     sdmx-subject:2 ;
        skos:definition  "Macroeconomic statistics - all activities that are dealing with economy wide statistics at macro level that go beyond, or are different from National Accounts, whether annual, quarterly or monthly. Examples are macroeconomic databases that combine national accounts and other macroeconomic indicators like Main Economic Indicators (OECD), Principal European Economic Indicators (Eurostat), etc. ; business tendency and consumer opinion surveys, economic growth, stability and structural adjustment, cyclical indicators, statistics for business cycle analysis.\nExcludes: \n- methodology and frameworks of national accounts (2.2.)\n- collection and dissemination of national accounts and productivity data not linked to other macroeconomic statistics (2.2)"@en ;
        skos:notation    "2.1" ;
        skos:prefLabel   "Macroeconomic statistics"@en .

sdmx:CodeList  a         rdfs:Class , owl:Class ;
        rdfs:label       "Concept scheme"@en ;
        rdfs:subClassOf  skos:ConceptScheme .

sdmx-metadata:timeFormat
        a                 sdmx:MetadataProperty , rdf:Property , qb:CodedProperty ;
        rdfs:comment      "Technical format in which time is represented for the measured phenomenon."@en ;
        rdfs:isDefinedBy  <http://sdmx.org/wp-content/uploads/2009/01/01_sdmx_cog_annex_1_cdc_2009.pdf> ;
        rdfs:label        "Time Format"@en ;
        rdfs:range        sdmx-code:TimeFormat ;
        qb:codeList       sdmx-code:timeFormat ;
        qb:concept        sdmx-concept:timeFormat .

sdmx:MeasureProperty  a   rdfs:Class , owl:Class ;
        rdfs:label        "Measure property"@en ;
        rdfs:subClassOf   sdmx:ComponentProperty ;
        owl:disjointWith  sdmx:AttributeProperty , sdmx:DimensionProperty .

sdmx-metadata:dataValidation
        a                 sdmx:MetadataProperty , rdf:Property ;
        rdfs:comment      "Process of monitoring the results of data compilation and ensuring the quality of the statistical results."@en ;
        rdfs:isDefinedBy  <http://sdmx.org/wp-content/uploads/2009/01/01_sdmx_cog_annex_1_cdc_2009.pdf> ;
        rdfs:label        "Data Validation"@en ;
        qb:concept        sdmx-concept:dataValidation .

sdmx:TimeSeries  a       rdfs:Class , owl:Class ;
        rdfs:label       "Time series"@en ;
        rdfs:subClassOf  sdmx:Attachable , sdmx:Slice .

sdmx-code:freq-M  a        skos:Concept , sdmx:Concept , sdmx-code:Freq ;
        skos:inScheme      sdmx-code:freq ;
        skos:notation      "M" ;
        skos:prefLabel     "Monthly"@en ;
        skos:topConceptOf  sdmx-code:freq .

sdmx-code:obsStatus-B
        a                  skos:Concept , sdmx:Concept , sdmx-code:ObsStatus ;
        skos:definition    "Break observations are characterised as such when different content exist or a different methodology has been applied to this observation as compared with the preceding one (the one given for the previous period)."@en ;
        skos:inScheme      sdmx-code:obsStatus ;
        skos:notation      "B" ;
        skos:prefLabel     "Break"@en ;
        skos:topConceptOf  sdmx-code:obsStatus .

sdmx-concept:contactMail
        a                 sdmx:Concept , skos:Concept ;
        rdfs:comment      "The postal address of the contact points for the data or metadata."@en ;
        rdfs:isDefinedBy  <http://sdmx.org/wp-content/uploads/2009/01/01_sdmx_cog_annex_1_cdc_2009.pdf> ;
        rdfs:label        "Contact mail address"@en ;
        skos:broader      sdmx-concept:contact ;
        skos:inScheme     sdmx-concept:cog ;
        skos:notation     "urn:sdmx:org.sdmx.infomodel.conceptscheme.Concept=SDMX:CROSS_DOMAIN_CONCEPTS[1.0].CONTACT_MAIL" .

sdmx-metadata:accessibility
        a                 sdmx:MetadataProperty , rdf:Property ;
        rdfs:comment      "The ease and the conditions under which statistical information can be obtained."@en ;
        rdfs:isDefinedBy  <http://sdmx.org/wp-content/uploads/2009/01/01_sdmx_cog_annex_1_cdc_2009.pdf> ;
        rdfs:label        "Accessibility"@en ;
        qb:concept        sdmx-concept:accessibility .

sdmx-code:decimals-5  a    skos:Concept , sdmx:Concept , sdmx-code:Decimals ;
        skos:inScheme      sdmx-code:decimals ;
        skos:notation      "5" ;
        skos:prefLabel     "Five"@en ;
        skos:topConceptOf  sdmx-code:decimals .

sdmx-concept:age  a       sdmx:Concept , skos:Concept ;
        rdfs:comment      "The length of time that a person has lived or a thing has existed."@en ;
        rdfs:isDefinedBy  <http://sdmx.org/wp-content/uploads/2009/01/01_sdmx_cog_annex_1_cdc_2009.pdf> ;
        rdfs:label        "Age"@en ;
        skos:inScheme     sdmx-concept:cog ;
        skos:notation     "urn:sdmx:org.sdmx.infomodel.conceptscheme.Concept=SDMX:CROSS_DOMAIN_CONCEPTS[1.0].AGE" .

sdmx-concept:completeness
        a                 sdmx:Concept , skos:Concept ;
        rdfs:comment      "The extent to which all statistics that are needed are available."@en ;
        rdfs:isDefinedBy  <http://sdmx.org/wp-content/uploads/2009/01/01_sdmx_cog_annex_1_cdc_2009.pdf> ;
        rdfs:label        "Relevance - Completeness"@en ;
        skos:broader      sdmx-concept:relevance ;
        skos:inScheme     sdmx-concept:cog ;
        skos:notation     "urn:sdmx:org.sdmx.infomodel.conceptscheme.Concept=SDMX:CROSS_DOMAIN_CONCEPTS[1.0].COMPLETENESS" .

sdmx-subject:3.2  a      skos:Concept , sdmx:Concept , sdmx-subject:SubjectMatterDomain ;
        skos:broader     sdmx-subject:3 ;
        skos:definition  "Regional and small area statistics - activities dealing with regional statistics and statistics referring to sub-national areas or areas based on administrative units, urban and rural statistics, rural development, regional accounts, regional typologies, and regional disparities."@en ;
        skos:notation    "3.2" ;
        skos:prefLabel   "Regional and small area statistics"@en .

sdmx-metadata:comparTime
        a                 sdmx:MetadataProperty , rdf:Property ;
        rdfs:comment      "Extent to which statistics are comparable or reconcilable over time."@en ;
        rdfs:isDefinedBy  <http://sdmx.org/wp-content/uploads/2009/01/01_sdmx_cog_annex_1_cdc_2009.pdf> ;
        rdfs:label        "Comparability - over time"@en ;
        qb:concept        sdmx-concept:comparTime .

sdmx-concept:timeFormat
        a                 sdmx:Concept , skos:Concept ;
        rdfs:comment      "Technical format in which time is represented for the measured phenomenon."@en ;
        rdfs:isDefinedBy  <http://sdmx.org/wp-content/uploads/2009/01/01_sdmx_cog_annex_1_cdc_2009.pdf> ;
        rdfs:label        "Time Format"@en ;
        skos:inScheme     sdmx-concept:cog ;
        skos:notation     "urn:sdmx:org.sdmx.infomodel.conceptscheme.Concept=SDMX:CROSS_DOMAIN_CONCEPTS[1.0].TIME_FORMAT" .

sdmx-metadata:unitMeasure
        a                 sdmx:MetadataProperty , rdf:Property ;
        rdfs:comment      "The unit in which the data values are measured."@en ;
        rdfs:isDefinedBy  <http://sdmx.org/wp-content/uploads/2009/01/01_sdmx_cog_annex_1_cdc_2009.pdf> ;
        rdfs:label        "Unit of Measure"@en ;
        qb:concept        sdmx-concept:unitMeasure .

sdmx-code:unitMult-6  a    skos:Concept , sdmx:Concept , sdmx-code:UnitMult ;
        skos:inScheme      sdmx-code:unitMult ;
        skos:notation      "6" ;
        skos:prefLabel     "Millions"@en ;
        skos:topConceptOf  sdmx-code:unitMult .

sdmx-code:confStatus-N
        a                  skos:Concept , sdmx:Concept , sdmx-code:ConfStatus ;
        skos:definition    "Used to denote observations that are restricted for internal use only within organisations."@en ;
        skos:inScheme      sdmx-code:confStatus ;
        skos:notation      "N" ;
        skos:prefLabel     "Not for publication, restricted for internal use only"@en ;
        skos:topConceptOf  sdmx-code:confStatus .

eg:o14  a                  qb:Observation ;
        eg:lifeExpectancy  75.5 ;
        eg:refArea         ex-geo:merthyr_tdfil_00ph ;
        qb:dataSet         eg:dataset-le3 .

sdmx-concept:timePerCollect
        a                 sdmx:Concept , skos:Concept ;
        rdfs:comment      "Dates or periods during which the observations have been collected (such as middle, average or end of period) to compile the indicator for the target reference period."@en ;
        rdfs:isDefinedBy  <http://sdmx.org/wp-content/uploads/2009/01/01_sdmx_cog_annex_1_cdc_2009.pdf> ;
        rdfs:label        "Time Period - collection"@en ;
        skos:broader      sdmx-concept:timePeriod ;
        skos:inScheme     sdmx-concept:cog ;
        skos:notation     "urn:sdmx:org.sdmx.infomodel.conceptscheme.Concept=SDMX:CROSS_DOMAIN_CONCEPTS[1.0].TIME_PER_COLLECT" .

sdmx-code:obsStatus-S
        a                  skos:Concept , sdmx:Concept , sdmx-code:ObsStatus ;
        skos:definition    "A known strike that occurred in the corresponding period that may have affected the observation or caused a missing value."@en ;
        skos:inScheme      sdmx-code:obsStatus ;
        skos:notation      "S" ;
        skos:prefLabel     "Strike"@en ;
        skos:topConceptOf  sdmx-code:obsStatus .

sdmx-concept:comment  a   sdmx:Concept , skos:Concept ;
        rdfs:comment      "Supplementary descriptive text which can be attached to data or metadata."@en ;
        rdfs:isDefinedBy  <http://sdmx.org/wp-content/uploads/2009/01/01_sdmx_cog_annex_1_cdc_2009.pdf> ;
        rdfs:label        "Comment"@en ;
        skos:inScheme     sdmx-concept:cog ;
        skos:notation     "urn:sdmx:org.sdmx.infomodel.conceptscheme.Concept=SDMX:CROSS_DOMAIN_CONCEPTS[1.0].COMMENT" .

sdmx-code:timeFormat-604
        a                  skos:Concept , sdmx:Concept , sdmx-code:TimeFormat ;
        skos:definition    "(for half yearly series)\nyear/semester"@en ;
        skos:inScheme      sdmx-code:timeFormat ;
        skos:notation      "604" ;
        skos:prefLabel     "CCYYS"@en ;
        skos:topConceptOf  sdmx-code:timeFormat .

sdmx-attribute:freqDiss
        a                 qb:AttributeProperty , rdf:Property ;
        rdfs:comment      "The time interval at which the statistics are disseminated over a given time period."@en ;
        rdfs:isDefinedBy  <http://sdmx.org/wp-content/uploads/2009/01/01_sdmx_cog_annex_1_cdc_2009.pdf> ;
        rdfs:label        "Frequency of dissemination"@en ;
        qb:concept        sdmx-concept:freqDiss .

sdmx:dataFlow  a     rdf:Property , owl:ObjectProperty ;
        rdfs:domain  sdmx:DataSet ;
        rdfs:label   "data flow"@en ;
        rdfs:range   sdmx:DataFlow .

sdmx:ReportEntry  a   owl:Class , rdfs:Class ;
        rdfs:comment  "Represents the type of things that can be contained in reports" ;
        rdfs:label    "report entry"@en .

sdmx-concept:educationLev
        a                 sdmx:Concept , skos:Concept ;
        rdfs:comment      "The highest level of an educational programme the person has successfully completed."@en ;
        rdfs:isDefinedBy  <http://sdmx.org/wp-content/uploads/2009/01/01_sdmx_cog_annex_1_cdc_2009.pdf> ;
        rdfs:label        "Education Level"@en ;
        skos:inScheme     sdmx-concept:cog ;
        skos:notation     "urn:sdmx:org.sdmx.infomodel.conceptscheme.Concept=SDMX:CROSS_DOMAIN_CONCEPTS[1.0].EDUCATION_LEV" .

sdmx:MetadataReportStructure
        a             rdfs:Class , owl:Class ;
        rdfs:comment  "Defines the structure of a single report within an MSD"@en ;
        rdfs:label    "Metadata report structure"@en .

sdmx-metadata:nonsamplingErr
        a                 sdmx:MetadataProperty , rdf:Property ;
        rdfs:comment      "Error in sample estimates which cannot be attributed to sampling fluctuations."@en ;
        rdfs:isDefinedBy  <http://sdmx.org/wp-content/uploads/2009/01/01_sdmx_cog_annex_1_cdc_2009.pdf> ;
        rdfs:label        "Accuracy - nonsampling error"@en ;
        qb:concept        sdmx-concept:nonsamplingErr .

sdmx-attribute:basePer
        a                 qb:AttributeProperty , rdf:Property ;
        rdfs:comment      "The period of time used as the base of an index number, or to which a constant price series refers."@en ;
        rdfs:isDefinedBy  <http://sdmx.org/wp-content/uploads/2009/01/01_sdmx_cog_annex_1_cdc_2009.pdf> ;
        rdfs:label        "Base Period"@en ;
        qb:concept        sdmx-concept:basePer .

sdmx-metadata:classSystem
        a                 sdmx:MetadataProperty , rdf:Property ;
        rdfs:comment      "Arrangement or division of objects into groups based on characteristics which the objects have in common."@en ;
        rdfs:isDefinedBy  <http://sdmx.org/wp-content/uploads/2009/01/01_sdmx_cog_annex_1_cdc_2009.pdf> ;
        rdfs:label        "Classification systems"@en ;
        qb:concept        sdmx-concept:classSystem .

sdmx-metadata:compilingOrg
        a                 sdmx:MetadataProperty , rdf:Property ;
        rdfs:comment      "The organisation compiling the data being reported."@en ;
        rdfs:isDefinedBy  <http://sdmx.org/wp-content/uploads/2009/01/01_sdmx_cog_annex_1_cdc_2009.pdf> ;
        rdfs:label        "Compiling agency"@en ;
        qb:concept        sdmx-concept:compilingOrg .

sdmx-attribute:compilingOrg
        a                 qb:AttributeProperty , rdf:Property ;
        rdfs:comment      "The organisation compiling the data being reported."@en ;
        rdfs:isDefinedBy  <http://sdmx.org/wp-content/uploads/2009/01/01_sdmx_cog_annex_1_cdc_2009.pdf> ;
        rdfs:label        "Compiling agency"@en ;
        qb:concept        sdmx-concept:compilingOrg .

sdmx-code:UnitMult  a    rdfs:Class , owl:Class ;
        rdfs:comment     "it provides code values for indicating the magnitude in the units of measurements."@en ;
        rdfs:label       "code list for the Unit Multiplier (UNIT_MULT) - codelist class"@en ;
        rdfs:seeAlso     sdmx-code:unitMult ;
        rdfs:subClassOf  skos:Concept .

sdmx-attribute:obsPreBreak
        a                 qb:AttributeProperty , rdf:Property ;
        rdfs:comment      "The observation, at a time series break period, that was calculated using the old methodology."@en ;
        rdfs:isDefinedBy  <http://sdmx.org/wp-content/uploads/2009/01/01_sdmx_cog_annex_1_cdc_2009.pdf> ;
        rdfs:label        "Observation Pre-break Value"@en ;
        qb:concept        sdmx-concept:obsPreBreak .

sdmx-metadata:dissOrg
        a                 sdmx:MetadataProperty , rdf:Property ;
        rdfs:comment      "The organisation disseminating the data."@en ;
        rdfs:isDefinedBy  <http://sdmx.org/wp-content/uploads/2009/01/01_sdmx_cog_annex_1_cdc_2009.pdf> ;
        rdfs:label        "Data Dissemination Agency"@en ;
        qb:concept        sdmx-concept:dissOrg .

sdmx-code:timeFormat-P1D
        a                  skos:Concept , sdmx:Concept , sdmx-code:TimeFormat ;
        skos:inScheme      sdmx-code:timeFormat ;
        skos:notation      "P1D" ;
        skos:prefLabel     "Daily (or Business)"@en ;
        skos:topConceptOf  sdmx-code:timeFormat .

sdmx-concept:userSat  a   sdmx:Concept , skos:Concept ;
        rdfs:comment      "Measure to determine user satisfaction."@en ;
        rdfs:isDefinedBy  <http://sdmx.org/wp-content/uploads/2009/01/01_sdmx_cog_annex_1_cdc_2009.pdf> ;
        rdfs:label        "Relevance - user satisifaction"@en ;
        skos:broader      sdmx-concept:relevance ;
        skos:inScheme     sdmx-concept:cog ;
        skos:notation     "urn:sdmx:org.sdmx.infomodel.conceptscheme.Concept=SDMX:CROSS_DOMAIN_CONCEPTS[1.0].USER_SAT" .

sdmx:EntityProperty  a    rdfs:Class , owl:Class ;
        rdfs:label        "Entity property"@en ;
        rdfs:subClassOf   sdmx:ConceptRoleProperty ;
        owl:disjointWith  sdmx:MeasureProperty .

sdmx-attribute:onlineDb
        a                 qb:AttributeProperty , rdf:Property ;
        rdfs:comment      "Information about on-line databases in which the disseminated data can be accessed."@en ;
        rdfs:isDefinedBy  <http://sdmx.org/wp-content/uploads/2009/01/01_sdmx_cog_annex_1_cdc_2009.pdf> ;
        rdfs:label        "Dissemination Format - online database"@en ;
        qb:concept        sdmx-concept:onlineDb .

sdmx:PrimaryMeasureRole
        a                rdfs:Class , owl:Class ;
        rdfs:comment     "concept for a measure that plays the role of the observation in a time series"@en ;
        rdfs:label       "Primary measure property"@en ;
        rdfs:subClassOf  sdmx:ConceptRole .

sdmx-code:decimals-0  a    skos:Concept , sdmx:Concept , sdmx-code:Decimals ;
        skos:inScheme      sdmx-code:decimals ;
        skos:notation      "0" ;
        skos:prefLabel     "Zero"@en ;
        skos:topConceptOf  sdmx-code:decimals .

sdmx-metadata:instMandate
        a                 sdmx:MetadataProperty , rdf:Property ;
        rdfs:comment      "Set of rules or other formal set of instructions assigning responsibility as well as the authority to an organisation for the collection, processing, and dissemination of statistics."@en ;
        rdfs:isDefinedBy  <http://sdmx.org/wp-content/uploads/2009/01/01_sdmx_cog_annex_1_cdc_2009.pdf> ;
        rdfs:label        "Institutional Mandate"@en ;
        qb:concept        sdmx-concept:instMandate .

sdmx-dimension:age  a     qb:DimensionProperty , rdf:Property ;
        rdfs:comment      "The length of time that a person has lived or a thing has existed."@en ;
        rdfs:isDefinedBy  <http://sdmx.org/wp-content/uploads/2009/01/01_sdmx_cog_annex_1_cdc_2009.pdf> ;
        rdfs:label        "Age"@en ;
        rdfs:range        rdfs:Resource ;
        qb:concept        sdmx-concept:age .

sdmx-metadata:freq  a     sdmx:MetadataProperty , rdf:Property , qb:CodedProperty ;
        rdfs:comment      "The time interval at which observations occur over a given time period."@en ;
        rdfs:isDefinedBy  <http://sdmx.org/wp-content/uploads/2009/01/01_sdmx_cog_annex_1_cdc_2009.pdf> ;
        rdfs:label        "Frequency"@en ;
        rdfs:range        sdmx-code:Freq ;
        qb:codeList       sdmx-code:freq ;
        qb:concept        sdmx-concept:freq .

sdmx-metadata:statConcDef
        a                 sdmx:MetadataProperty , rdf:Property ;
        rdfs:comment      "Statistical characteristics of statistical observations."@en ;
        rdfs:isDefinedBy  <http://sdmx.org/wp-content/uploads/2009/01/01_sdmx_cog_annex_1_cdc_2009.pdf> ;
        rdfs:label        "Statistical Concepts and Definitions"@en ;
        qb:concept        sdmx-concept:statConcDef .

sdmx-concept:sampling
        a                 sdmx:Concept , skos:Concept ;
        rdfs:comment      "The process of selecting a number of cases from all the cases in a particular group or universe."@en ;
        rdfs:isDefinedBy  <http://sdmx.org/wp-content/uploads/2009/01/01_sdmx_cog_annex_1_cdc_2009.pdf> ;
        rdfs:label        "Sampling"@en ;
        skos:inScheme     sdmx-concept:cog ;
        skos:notation     "urn:sdmx:org.sdmx.infomodel.conceptscheme.Concept=SDMX:CROSS_DOMAIN_CONCEPTS[1.0].SAMPLING" .

sdmx-concept:coverageSector
        a                 sdmx:Concept , skos:Concept ;
        rdfs:comment      "Main economic or other sectors covered by the statistics."@en ;
        rdfs:isDefinedBy  <http://sdmx.org/wp-content/uploads/2009/01/01_sdmx_cog_annex_1_cdc_2009.pdf> ;
        rdfs:label        "Coverage - sector"@en ;
        skos:broader      sdmx-concept:coverage ;
        skos:inScheme     sdmx-concept:cog ;
        skos:notation     "urn:sdmx:org.sdmx.infomodel.conceptscheme.Concept=SDMX:CROSS_DOMAIN_CONCEPTS[1.0].COVERAGE_SECTOR" .

sdmx:NonObsTimeRole  a   rdfs:Class , owl:Class ;
        rdfs:comment     "concept for a dimension or attribute that plays the role of a date/time identifier in the KeyFamily which is not related to the time of the observation"@en ;
        rdfs:label       "Non-observation time property"@en ;
        rdfs:subClassOf  sdmx:ConceptRole .

sdmx-concept:statPop  a   sdmx:Concept , skos:Concept ;
        rdfs:comment      "The total membership or population or \"universe\" of a defined class of people, objects or events."@en ;
        rdfs:isDefinedBy  <http://sdmx.org/wp-content/uploads/2009/01/01_sdmx_cog_annex_1_cdc_2009.pdf> ;
        rdfs:label        "Statistical Population"@en ;
        skos:inScheme     sdmx-concept:cog ;
        skos:notation     "urn:sdmx:org.sdmx.infomodel.conceptscheme.Concept=SDMX:CROSS_DOMAIN_CONCEPTS[1.0].STAT_POP" .

eg:o41  a                  qb:Observation ;
        eg:lifeExpectancy  80.9 ;
        eg:refArea         ex-geo:newport_00pr ;
        qb:dataSet         eg:dataset-le3 .

sdmx-attribute:dissFormat
        a                 qb:AttributeProperty , rdf:Property ;
        rdfs:comment      "Media by which statistical data and metadata are disseminated."@en ;
        rdfs:isDefinedBy  <http://sdmx.org/wp-content/uploads/2009/01/01_sdmx_cog_annex_1_cdc_2009.pdf> ;
        rdfs:label        "Dissemination Format"@en ;
        qb:concept        sdmx-concept:dissFormat .

sdmx-metadata:sampling
        a                 sdmx:MetadataProperty , rdf:Property ;
        rdfs:comment      "The process of selecting a number of cases from all the cases in a particular group or universe."@en ;
        rdfs:isDefinedBy  <http://sdmx.org/wp-content/uploads/2009/01/01_sdmx_cog_annex_1_cdc_2009.pdf> ;
        rdfs:label        "Sampling"@en ;
        qb:concept        sdmx-concept:sampling .

sdmx:Structure  a     rdfs:Class , owl:Class ;
        rdfs:comment  "Abstract class for defining the structure (ComponentProperties) that can be used in some data or metadata set"@en ;
        rdfs:label    "Structure"@en .

sdmx-code:unitMult-1  a    skos:Concept , sdmx:Concept , sdmx-code:UnitMult ;
        skos:inScheme      sdmx-code:unitMult ;
        skos:notation      "1" ;
        skos:prefLabel     "Tens"@en ;
        skos:topConceptOf  sdmx-code:unitMult .

sdmx-code:sex-N  a         skos:Concept , sdmx:Concept , sdmx-code:Sex ;
        skos:inScheme      sdmx-code:sex ;
        skos:notation      "N" ;
        skos:prefLabel     "Not applicable"@en ;
        skos:topConceptOf  sdmx-code:sex .

eg:slice4  a                qb:Slice ;
        eg:refPeriod        <http://reference.data.gov.uk/id/gregorian-interval/2005-01-01T00:00:00/P3Y> ;
        qb:observation      eg:o41 , eg:o42 , eg:o43 , eg:o44 ;
        qb:sliceStructure   eg:sliceByRegion ;
        sdmx-dimension:sex  sdmx-code:sex-F .

sdmx-metadata:visArea
        a                 sdmx:MetadataProperty , rdf:Property ;
        rdfs:comment      "The secondary area, as opposed to reference area, to which the measured data is in relation."@en ;
        rdfs:isDefinedBy  <http://sdmx.org/wp-content/uploads/2009/01/01_sdmx_cog_annex_1_cdc_2009.pdf> ;
        rdfs:label        "Counterpart Reference Area"@en ;
        qb:concept        sdmx-concept:visArea .

sdmx-subject:2.4.6  a    skos:Concept , sdmx:Concept , sdmx-subject:SubjectMatterDomain ;
        skos:broader     sdmx-subject:2.4 ;
        skos:definition  "Banking, insurance, financial statistics - money, banking and financial market statistics, including financial accounts, money supply, interest rates, exchange rates, stock market indicators, securities, bank profitability, private sector insurance and pension fund statistics, Financial Soundness Indicators. \nExcludes \n- beneficiaries of private pension funds (1.6) \n- financing of state pension and of other state social security schemes (2.5)"@en ;
        skos:notation    "2.4.6" ;
        skos:prefLabel   "Banking, insurance, financial statistics"@en .

sdmx-metadata:relevance
        a                 sdmx:MetadataProperty , rdf:Property ;
        rdfs:comment      "The degree to which statistical information meets the real or perceived needs of clients."@en ;
        rdfs:isDefinedBy  <http://sdmx.org/wp-content/uploads/2009/01/01_sdmx_cog_annex_1_cdc_2009.pdf> ;
        rdfs:label        "Relevance"@en ;
        qb:concept        sdmx-concept:relevance .

sdmx-subject:1.7  a      skos:Concept , sdmx:Concept , sdmx-subject:SubjectMatterDomain ;
        skos:broader     sdmx-subject:1 ;
        skos:definition  "Human settlements and housing - covers statistical activities on housing, dwellings and human settlements\nExcludes \n- rents (2.7)"@en ;
        skos:notation    "1.7" ;
        skos:prefLabel   "Human settlements and housing"@en .

sdmx-metadata:confStatus
        a                 sdmx:MetadataProperty , rdf:Property , qb:CodedProperty ;
        rdfs:comment      "Information about the confidentiality status of the object to which this attribute is attached."@en ;
        rdfs:isDefinedBy  <http://sdmx.org/wp-content/uploads/2009/01/01_sdmx_cog_annex_1_cdc_2009.pdf> ;
        rdfs:label        "Confidentiality - status"@en ;
        rdfs:range        sdmx-code:ConfStatus ;
        qb:codeList       sdmx-code:confStatus ;
        qb:concept        sdmx-concept:confStatus .

sdmx-attribute:metaUpdate
        a                 qb:AttributeProperty , rdf:Property ;
        rdfs:comment      "The date on which the metadata element was inserted or modified in the database."@en ;
        rdfs:isDefinedBy  <http://sdmx.org/wp-content/uploads/2009/01/01_sdmx_cog_annex_1_cdc_2009.pdf> ;
        rdfs:label        "Metadata Update"@en ;
        qb:concept        sdmx-concept:metaUpdate .

sdmx:Annotation  a    rdfs:Class , owl:Class ;
        rdfs:comment  "A resource denoting some type of annotation on a statistic, which may be at the observation, time series or dataset level" ;
        rdfs:label    "annotation"@en .

sdmx:EntityRole  a       rdfs:Class , owl:Class ;
        rdfs:comment     "concept for a dimension or attribute that plays the role of the DataAttribute subject to whom the data refers (e.g. the reporting agent for primary reporting, the country for secondary reporting)"@en ;
        rdfs:label       "Entity property"@en ;
        rdfs:subClassOf  sdmx:ConceptRole .

qb:measureType  qb:concept  sdmx:measureTypeConcept .

sdmx-attribute:metaCertified
        a                 qb:AttributeProperty , rdf:Property ;
        rdfs:comment      "Date of the latest certification provided by the domain manager to confirm that the metadata posted are still up-to-date, even if the content has not been amended."@en ;
        rdfs:isDefinedBy  <http://sdmx.org/wp-content/uploads/2009/01/01_sdmx_cog_annex_1_cdc_2009.pdf> ;
        rdfs:label        "Metadata Update - last certified"@en ;
        qb:concept        sdmx-concept:metaCertified .

sdmx-concept:dataProvider
        a                 sdmx:Concept , skos:Concept ;
        rdfs:comment      "Organisation which produces data or metadata"@en ;
        rdfs:isDefinedBy  <http://sdmx.org/wp-content/uploads/2009/01/01_sdmx_cog_annex_1_cdc_2009.pdf> ;
        rdfs:label        "Data Provider"@en ;
        skos:inScheme     sdmx-concept:cog ;
        skos:notation     "urn:sdmx:org.sdmx.infomodel.conceptscheme.Concept=SDMX:CROSS_DOMAIN_CONCEPTS[1.0].DATA_PROVIDER" .

sdmx:componentOrder  a  rdf:Property , owl:ObjectProperty ;
        rdfs:comment  "Optional specification of the order in which dimensions (and optionally other components) should be used. Value is an rdf:List of sdmxComponents" , "Optional specification of the order in which dimensions (and optionally other components) should be used. Value is an rdf:List of sdmx:ComponentProperties or sdmx:ComponentSpecifications"@en ;
        rdfs:domain   sdmx:DataStructureDefinition , sdmx:Structure ;
        rdfs:label    "component order"@en ;
        rdfs:range    rdf:List .

sdmx-attribute:coherXDom
        a                 qb:AttributeProperty , rdf:Property ;
        rdfs:comment      "Extent to which statistics are reconcilable with those obtained through other data sources or statistical domains."@en ;
        rdfs:isDefinedBy  <http://sdmx.org/wp-content/uploads/2009/01/01_sdmx_cog_annex_1_cdc_2009.pdf> ;
        rdfs:label        "Coherence - cross domain"@en ;
        qb:concept        sdmx-concept:coherXDom .

sdmx-measure:age  a       qb:MeasureProperty , rdf:Property ;
        rdfs:comment      "The length of time that a person has lived or a thing has existed."@en ;
        rdfs:isDefinedBy  <http://sdmx.org/wp-content/uploads/2009/01/01_sdmx_cog_annex_1_cdc_2009.pdf> ;
        rdfs:label        "Age"@en ;
        qb:concept        sdmx-concept:age .

sdmx-metadata:timeliness
        a                 sdmx:MetadataProperty , rdf:Property ;
        rdfs:comment      "Length of time between data availability and the event or phenomenon they describe."@en ;
        rdfs:isDefinedBy  <http://sdmx.org/wp-content/uploads/2009/01/01_sdmx_cog_annex_1_cdc_2009.pdf> ;
        rdfs:label        "Timelinesst"@en ;
        qb:concept        sdmx-concept:timeliness .

sdmx:Group  a            rdfs:Class , owl:Class ;
        rdfs:label       "Group"@en ;
        rdfs:subClassOf  sdmx:Attachable , sdmx:Slice .

sdmx-concept:relCalAccess
        a                 sdmx:Concept , skos:Concept ;
        rdfs:comment      "Access to the release calendar information."@en ;
        rdfs:isDefinedBy  <http://sdmx.org/wp-content/uploads/2009/01/01_sdmx_cog_annex_1_cdc_2009.pdf> ;
        rdfs:label        "Release Policy - release calendar access"@en ;
        skos:broader      sdmx-concept:relPolicy ;
        skos:inScheme     sdmx-concept:cog ;
        skos:notation     "urn:sdmx:org.sdmx.infomodel.conceptscheme.Concept=SDMX:CROSS_DOMAIN_CONCEPTS[1.0].REL_CAL_ACCESS" .

sdmx:agreement  a    rdf:Property , owl:ObjectProperty ;
        rdfs:domain  sdmx:DataProvider ;
        rdfs:label   "agreement"@en ;
        rdfs:range   sdmx:ProvisionAgreement .

eg:o54  a                  qb:Observation ;
        eg:lifeExpectancy  74.9 ;
        eg:refArea         ex-geo:merthyr_tdfil_00ph ;
        qb:dataSet         eg:dataset-le3 .

sdmx-subject:2.8  a      skos:Concept , sdmx:Concept , sdmx-subject:SubjectMatterDomain ;
        skos:broader     sdmx-subject:2 ;
        skos:definition  "Labour cost - statistics activities on labour cost, earning and wages, both for structural and short-term statistics. \nExcludes\n- wages as part of total income of private households (1.5)"@en ;
        skos:notation    "2.8" ;
        skos:prefLabel   "Labor cost"@en .

eg:o22  a                  qb:Observation ;
        eg:lifeExpectancy  83.3 ;
        eg:refArea         ex-geo:cardiff_00pt ;
        qb:dataSet         eg:dataset-le3 .

sdmx-code:Freq  a        rdfs:Class , owl:Class ;
        rdfs:comment     "It provides a list of values indicating the \"frequency\" of the data (e.g. monthly) and, thus, indirectly, also implying the type of \"time reference\" that could be used for identifying the data with respect time."@en ;
        rdfs:label       "Code list for Frequency (FREQ) - codelist class"@en ;
        rdfs:seeAlso     sdmx-code:freq ;
        rdfs:subClassOf  skos:Concept .

sdmx-measure:currency
        a                 qb:MeasureProperty , rdf:Property , qb:CodedProperty ;
        rdfs:comment      "Monetary denomination of the object being measured."@en ;
        rdfs:isDefinedBy  <http://sdmx.org/wp-content/uploads/2009/01/01_sdmx_cog_annex_1_cdc_2009.pdf> ;
        rdfs:label        "Currency"@en ;
        rdfs:range        sdmx-code:Currency ;
        qb:codeList       sdmx-code:currency ;
        qb:concept        sdmx-concept:currency .

sdmx-concept:confStatus
        a                 sdmx:Concept , skos:Concept ;
        rdfs:comment      "Information about the confidentiality status of the object to which this attribute is attached."@en ;
        rdfs:isDefinedBy  <http://sdmx.org/wp-content/uploads/2009/01/01_sdmx_cog_annex_1_cdc_2009.pdf> ;
        rdfs:label        "Confidentiality - status"@en ;
        skos:broader      sdmx-concept:conf ;
        skos:inScheme     sdmx-concept:cog ;
        skos:notation     "urn:sdmx:org.sdmx.infomodel.conceptscheme.Concept=SDMX:CROSS_DOMAIN_CONCEPTS[1.0].CONF_STATUS" .

sdmx-metadata:timePerCollect
        a                 sdmx:MetadataProperty , rdf:Property ;
        rdfs:comment      "Dates or periods during which the observations have been collected (such as middle, average or end of period) to compile the indicator for the target reference period."@en ;
        rdfs:isDefinedBy  <http://sdmx.org/wp-content/uploads/2009/01/01_sdmx_cog_annex_1_cdc_2009.pdf> ;
        rdfs:label        "Time Period - collection"@en ;
        qb:concept        sdmx-concept:timePerCollect .

sdmx-attribute:revPractice
        a                 qb:AttributeProperty , rdf:Property ;
        rdfs:comment      "Information on the data revision practice."@en ;
        rdfs:isDefinedBy  <http://sdmx.org/wp-content/uploads/2009/01/01_sdmx_cog_annex_1_cdc_2009.pdf> ;
        rdfs:label        "Data Revision - practice"@en ;
        qb:concept        sdmx-concept:revPractice .

sdmx-attribute:freqColl
        a                 qb:AttributeProperty , rdf:Property ;
        rdfs:comment      "Frequency with which the source data are collected."@en ;
        rdfs:isDefinedBy  <http://sdmx.org/wp-content/uploads/2009/01/01_sdmx_cog_annex_1_cdc_2009.pdf> ;
        rdfs:label        "Frequency of data collection"@en ;
        qb:concept        sdmx-concept:freqColl .

sdmx-metadata:relComment
        a                 sdmx:MetadataProperty , rdf:Property ;
        rdfs:comment      "Legal acts and other agreements pertaining to data access."@en ;
        rdfs:isDefinedBy  <http://sdmx.org/wp-content/uploads/2009/01/01_sdmx_cog_annex_1_cdc_2009.pdf> ;
        rdfs:label        "Release Policy - policy commentary"@en ;
        qb:concept        sdmx-concept:relComment .

sdmx-metadata:adjustment
        a                 sdmx:MetadataProperty , rdf:Property ;
        rdfs:comment      "The set of procedures employed to modify statistical data to enable it to conform to national or international standards or to address data quality differences when compiling specific data sets."@en ;
        rdfs:isDefinedBy  <http://sdmx.org/wp-content/uploads/2009/01/01_sdmx_cog_annex_1_cdc_2009.pdf> ;
        rdfs:label        "Adjustment"@en ;
        qb:concept        sdmx-concept:adjustment .

sdmx-metadata:metaCertified
        a                 sdmx:MetadataProperty , rdf:Property ;
        rdfs:comment      "Date of the latest certification provided by the domain manager to confirm that the metadata posted are still up-to-date, even if the content has not been amended."@en ;
        rdfs:isDefinedBy  <http://sdmx.org/wp-content/uploads/2009/01/01_sdmx_cog_annex_1_cdc_2009.pdf> ;
        rdfs:label        "Metadata Update - last certified"@en ;
        qb:concept        sdmx-concept:metaCertified .

sdmx-attribute:qualityAssmnt
        a                 qb:AttributeProperty , rdf:Property ;
        rdfs:comment      "Overall assessment of data quality, based on standard quality criteria."@en ;
        rdfs:isDefinedBy  <http://sdmx.org/wp-content/uploads/2009/01/01_sdmx_cog_annex_1_cdc_2009.pdf> ;
        rdfs:label        "Quality Management - assessment"@en ;
        qb:concept        sdmx-concept:qualityAssmnt .

sdmx:MetadataProperty
        a                 rdfs:Class , owl:Class ;
        rdfs:comment      "Class of properties used to provide metadata values in metadata reports (sdmx:MetadataSet)"@en ;
        rdfs:label        "Metadata property"@en ;
        rdfs:subClassOf   sdmx:ComponentProperty ;
        owl:disjointWith  sdmx:MeasureProperty , sdmx:AttributeProperty , sdmx:DimensionProperty .

sdmx:DataStructureDefinition
        a                rdfs:Class , owl:Class ;
        rdfs:comment     "A specialization of qb:DataStructureDefinition which additional constraints: if there are multiple measures then a MeasureDimensionProperty must be included in the DSD"@en ;
        rdfs:label       "Data Structure Definition"@en , "Data structure definition"@en ;
        rdfs:subClassOf  qb:DataStructureDefinition , sdmx:Structure .

sdmx-code:confStatus-D
        a                  skos:Concept , sdmx:Concept , sdmx-code:ConfStatus ;
        skos:definition    "Used by the sender of the data to flag (beyond the confidential statistical information) one or more additional observations of the dataset so that the receiver knows that he/she should suppress these observations in subsequent stages of processing (especially, dissemination) in order to prevent third parties to indirectly deduct (e.g. through accounting identities or other formulas) the observations that are genuinely flagged with \"C\"."@en ;
        skos:inScheme      sdmx-code:confStatus ;
        skos:notation      "D" ;
        skos:prefLabel     "Secondary confidentiality set by the sender, not for publication"@en ;
        skos:topConceptOf  sdmx-code:confStatus .

sdmx-concept:refArea  a   sdmx:Concept , skos:Concept ;
        rdfs:comment      "The country or geographic area to which the measured statistical phenomenon relates."@en ;
        rdfs:isDefinedBy  <http://sdmx.org/wp-content/uploads/2009/01/01_sdmx_cog_annex_1_cdc_2009.pdf> ;
        rdfs:label        "Reference Area"@en ;
        skos:inScheme     sdmx-concept:cog ;
        skos:notation     "urn:sdmx:org.sdmx.infomodel.conceptscheme.Concept=SDMX:CROSS_DOMAIN_CONCEPTS[1.0].REF_AREA" .

sdmx-code:obsStatus-I
        a                  skos:Concept , sdmx:Concept , sdmx-code:ObsStatus ;
        skos:definition    "Observation imputed by international organisations to replace or fill gaps in national data series, in line with the recommendations of the Committee for the Coordination of Statistical Activities (CCSA)."@en ;
        skos:inScheme      sdmx-code:obsStatus ;
        skos:notation      "I" ;
        skos:prefLabel     "Imputed value (CCSA definition)"@en ;
        skos:topConceptOf  sdmx-code:obsStatus .

sdmx-concept:freqDiss
        a                 sdmx:Concept , skos:Concept ;
        rdfs:comment      "The time interval at which the statistics are disseminated over a given time period."@en ;
        rdfs:isDefinedBy  <http://sdmx.org/wp-content/uploads/2009/01/01_sdmx_cog_annex_1_cdc_2009.pdf> ;
        rdfs:label        "Frequency of dissemination"@en ;
        skos:broader      sdmx-concept:freq ;
        skos:inScheme     sdmx-concept:cog ;
        skos:notation     "urn:sdmx:org.sdmx.infomodel.conceptscheme.Concept=SDMX:CROSS_DOMAIN_CONCEPTS[1.0].FREQ_DISS" .

sdmx-metadata:contact
        a                 sdmx:MetadataProperty , rdf:Property ;
        rdfs:comment      "Individual or organisational contact points for the data or metadata, including information on how to reach the contact points."@en ;
        rdfs:isDefinedBy  <http://sdmx.org/wp-content/uploads/2009/01/01_sdmx_cog_annex_1_cdc_2009.pdf> ;
        rdfs:label        "Contact"@en ;
        qb:concept        sdmx-concept:contact .

sdmx-subject:3.3.5  a    skos:Concept , sdmx:Concept , sdmx-subject:SubjectMatterDomain ;
        skos:broader     sdmx-subject:3.3 ;
        skos:definition  "Indicators related to the Millennium Development Goals - work on sets of indicators to monitor the achievement of the Millennium Development Goals agreed upon at the UN Millennium Summit."@en ;
        skos:notation    "3.3.5" ;
        skos:prefLabel   "Indicators related to the Millennium Development Goals"@en .

sdmx-concept:instManShar
        a                 sdmx:Concept , skos:Concept ;
        rdfs:comment      "Arrangements or procedures for data sharing and coordination between data producing agencies."@en ;
        rdfs:isDefinedBy  <http://sdmx.org/wp-content/uploads/2009/01/01_sdmx_cog_annex_1_cdc_2009.pdf> ;
        rdfs:label        "Institutional Mandate - data sharing"@en ;
        skos:broader      sdmx-concept:instMandate ;
        skos:inScheme     sdmx-concept:cog ;
        skos:notation     "urn:sdmx:org.sdmx.infomodel.conceptscheme.Concept=SDMX:CROSS_DOMAIN_CONCEPTS[1.0].INST_MAN_SHAR" .

sdmx-concept:timeliness
        a                 sdmx:Concept , skos:Concept ;
        rdfs:comment      "Length of time between data availability and the event or phenomenon they describe."@en ;
        rdfs:isDefinedBy  <http://sdmx.org/wp-content/uploads/2009/01/01_sdmx_cog_annex_1_cdc_2009.pdf> ;
        rdfs:label        "Timelinesst"@en ;
        skos:inScheme     sdmx-concept:cog ;
        skos:notation     "urn:sdmx:org.sdmx.infomodel.conceptscheme.Concept=SDMX:CROSS_DOMAIN_CONCEPTS[1.0].TIMELINESS" .

sdmx-concept:obsPreBreak
        a                 sdmx:Concept , skos:Concept ;
        rdfs:comment      "The observation, at a time series break period, that was calculated using the old methodology."@en ;
        rdfs:isDefinedBy  <http://sdmx.org/wp-content/uploads/2009/01/01_sdmx_cog_annex_1_cdc_2009.pdf> ;
        rdfs:label        "Observation Pre-break Value"@en ;
        skos:inScheme     sdmx-concept:cog ;
        skos:notation     "urn:sdmx:org.sdmx.infomodel.conceptscheme.Concept=SDMX:CROSS_DOMAIN_CONCEPTS[1.0].OBS_PRE_BREAK" .

sdmx-metadata:freqDiss
        a                 sdmx:MetadataProperty , rdf:Property ;
        rdfs:comment      "The time interval at which the statistics are disseminated over a given time period."@en ;
        rdfs:isDefinedBy  <http://sdmx.org/wp-content/uploads/2009/01/01_sdmx_cog_annex_1_cdc_2009.pdf> ;
        rdfs:label        "Frequency of dissemination"@en ;
        qb:concept        sdmx-concept:freqDiss .

sdmx-concept:costBurdenEff
        a                 sdmx:Concept , skos:Concept ;
        rdfs:comment      "Cost benefit analysis, effectiveness of execution of medium term statistical programs, and ensuring efficient use of resources."@en ;
        rdfs:isDefinedBy  <http://sdmx.org/wp-content/uploads/2009/01/01_sdmx_cog_annex_1_cdc_2009.pdf> ;
        rdfs:label        "Cost and Burden - efficiency management"@en ;
        skos:broader      sdmx-concept:costBurden ;
        skos:inScheme     sdmx-concept:cog ;
        skos:notation     "urn:sdmx:org.sdmx.infomodel.conceptscheme.Concept=SDMX:CROSS_DOMAIN_CONCEPTS[1.0].COST_BURDEN_EFF" .

sdmx-subject:2.4.1  a    skos:Concept , sdmx:Concept , sdmx-subject:SubjectMatterDomain ;
        skos:broader     sdmx-subject:2.4 ;
        skos:definition  "Agriculture, forestry, fisheries - includes all agriculture, forestry and fishery related statistics, e.g. agricultural monetary statistics (agricultural economic accounts), agricultural structures (farm structure), trade in agricultural products, agricultural labour input, crop and animal production, agricultural commodities, agro-industry statistics (including food production and safety), organic farming and organic food, government expenditure for agriculture, fishing and forestry, products source and use tables, forest and forest product statistics, forest resource assessment and forest fire, trade in forest products, fisheries.\nExcludes \n- agricultural and similar prices (2.7)\n- rural development (3.2)"@en ;
        skos:notation    "2.4.1" ;
        skos:prefLabel   "Agriculture, forestry, fisheries"@en .

sdmx:ConceptRole  a      rdfs:Class , owl:Class ;
        rdfs:comment     "Abstract superclass of classes denoting statistical roles which be played by concepts"@en ;
        rdfs:label       "Concept role (abstract)"@en ;
        rdfs:subClassOf  sdmx:Concept .

sdmx-subject:1.2  a      skos:Concept , sdmx:Concept , sdmx-subject:SubjectMatterDomain ;
        skos:broader     sdmx-subject:1 ;
        skos:definition  "Labour -  covers statistics on labour force, labour market, employment and unemployment; the more detailed topics include economically active population, labour conditions, health and safety at work (accidents at work, occupational injuries and diseases, work-related health problems), working time and other working conditions, strikes and lockouts, job vacancies, job creation. \nExcludes \n- migrant workers (1.1)\n- unemployment insurance and unemployment benefits (1.6)\n- trade union membership (1.10)\n- unpaid work (1.11)\n- statistics on earnings, wages and salaries (2.8)\n- labour cost (2.8)"@en ;
        skos:notation    "1.2" ;
        skos:prefLabel   "Labour"@en .

sdmx-metadata:valuation
        a                 sdmx:MetadataProperty , rdf:Property ;
        rdfs:comment      "The definition of the price per unit, for goods and services flows and asset stocks."@en ;
        rdfs:isDefinedBy  <http://sdmx.org/wp-content/uploads/2009/01/01_sdmx_cog_annex_1_cdc_2009.pdf> ;
        rdfs:label        "Valuation"@en ;
        qb:concept        sdmx-concept:valuation .

sdmx-subject:SubjectMatterDomain
        a                rdfs:Class , owl:Class ;
        rdfs:comment     "The SDMX Content Guidelines for Statistical Subject-Matter Domains."@en ;
        rdfs:label       "SDMX Statistical Subject-Matter Domains - concept class"@en ;
        rdfs:seeAlso     sdmx-subject:subjectMatterDomain ;
        rdfs:subClassOf  skos:Concept .

sdmx-metadata:obsStatus
        a                 sdmx:MetadataProperty , rdf:Property , qb:CodedProperty ;
        rdfs:comment      "Information on the quality of a value or an unusual or missing value."@en ;
        rdfs:isDefinedBy  <http://sdmx.org/wp-content/uploads/2009/01/01_sdmx_cog_annex_1_cdc_2009.pdf> ;
        rdfs:label        "Observation Status"@en ;
        rdfs:range        sdmx-code:ObsStatus ;
        qb:codeList       sdmx-code:obsStatus ;
        qb:concept        sdmx-concept:obsStatus .

sdmx:obsValue  a            rdf:Property , sdmx:MeasureProperty ;
        rdfs:comment        "Denotes the actual value of a given observation. The default measure property for SDMX-RDF." ;
        rdfs:domain         sdmx:Observation ;
        rdfs:label          "observation value"@en ;
        rdfs:subPropertyOf  rdf:value .

sdmx:reportingPeriod  a  rdf:Property , owl:ObjectProperty ;
        rdfs:domain  sdmx:DataSet ;
        rdfs:label   "reporting period"@en .

sdmx:DataProvider  a     rdfs:Class , owl:Class ;
        rdfs:label       "Data provider"@en ;
        rdfs:subClassOf  foaf:Agent .

sdmx-metadata:newsRel
        a                 sdmx:MetadataProperty , rdf:Property ;
        rdfs:comment      "Regular or ad-hoc press releases linked to the data."@en ;
        rdfs:isDefinedBy  <http://sdmx.org/wp-content/uploads/2009/01/01_sdmx_cog_annex_1_cdc_2009.pdf> ;
        rdfs:label        "Dissemination Format - news release"@en ;
        qb:concept        sdmx-concept:newsRel .

sdmx-code:unitMult-15
        a                  skos:Concept , sdmx:Concept , sdmx-code:UnitMult ;
        skos:inScheme      sdmx-code:unitMult ;
        skos:notation      "15" ;
        skos:prefLabel     "Quadrillions"@en ;
        skos:topConceptOf  sdmx-code:unitMult .

sdmx-concept:relComment
        a                 sdmx:Concept , skos:Concept ;
        rdfs:comment      "Legal acts and other agreements pertaining to data access."@en ;
        rdfs:isDefinedBy  <http://sdmx.org/wp-content/uploads/2009/01/01_sdmx_cog_annex_1_cdc_2009.pdf> ;
        rdfs:label        "Release Policy - policy commentary"@en ;
        skos:broader      sdmx-concept:relPolicy ;
        skos:inScheme     sdmx-concept:cog ;
        skos:notation     "urn:sdmx:org.sdmx.infomodel.conceptscheme.Concept=SDMX:CROSS_DOMAIN_CONCEPTS[1.0].REL_COMMENT" .

sdmx-concept:adjustment
        a                 sdmx:Concept , skos:Concept ;
        rdfs:comment      "The set of procedures employed to modify statistical data to enable it to conform to national or international standards or to address data quality differences when compiling specific data sets."@en ;
        rdfs:isDefinedBy  <http://sdmx.org/wp-content/uploads/2009/01/01_sdmx_cog_annex_1_cdc_2009.pdf> ;
        rdfs:label        "Adjustment"@en ;
        skos:inScheme     sdmx-concept:cog ;
        skos:notation     "urn:sdmx:org.sdmx.infomodel.conceptscheme.Concept=SDMX:CROSS_DOMAIN_CONCEPTS[1.0].ADJUSTMENT" .

sdmx-metadata:qualityAssmnt
        a                 sdmx:MetadataProperty , rdf:Property ;
        rdfs:comment      "Overall assessment of data quality, based on standard quality criteria."@en ;
        rdfs:isDefinedBy  <http://sdmx.org/wp-content/uploads/2009/01/01_sdmx_cog_annex_1_cdc_2009.pdf> ;
        rdfs:label        "Quality Management - assessment"@en ;
        qb:concept        sdmx-concept:qualityAssmnt .

sdmx-attribute:confPolicy
        a                 qb:AttributeProperty , rdf:Property ;
        rdfs:comment      "Legislative measures or other formal procedures which prevent unauthorised disclosure of data that identify a person or economic entity either directly or indirectly."@en ;
        rdfs:isDefinedBy  <http://sdmx.org/wp-content/uploads/2009/01/01_sdmx_cog_annex_1_cdc_2009.pdf> ;
        rdfs:label        "Confidentiality - policy"@en ;
        qb:concept        sdmx-concept:confPolicy .

sdmx-concept:onlineDb
        a                 sdmx:Concept , skos:Concept ;
        rdfs:comment      "Information about on-line databases in which the disseminated data can be accessed."@en ;
        rdfs:isDefinedBy  <http://sdmx.org/wp-content/uploads/2009/01/01_sdmx_cog_annex_1_cdc_2009.pdf> ;
        rdfs:label        "Dissemination Format - online database"@en ;
        skos:broader      sdmx-concept:dissFormat ;
        skos:inScheme     sdmx-concept:cog ;
        skos:notation     "urn:sdmx:org.sdmx.infomodel.conceptscheme.Concept=SDMX:CROSS_DOMAIN_CONCEPTS[1.0].ONLINE_DB" .

sdmx:DimensionProperty
        a                 rdfs:Class , owl:Class ;
        rdfs:label        "Dimension property"@en ;
        rdfs:subClassOf   sdmx:ComponentProperty , sdmx:CodedProperty , sdmx:DimensionOrAttributeProperty ;
        owl:disjointWith  sdmx:MeasureProperty .

sdmx:childComponents  a  rdf:Property , owl:ObjectProperty ;
        rdfs:comment  "Used primarily in sdmx:MetadataStructureDefinitions to indicate a grouping of the metadata properties used for presentational purposes. The sub components should still be listed as sdmx:components of the structure but in the sdmx:componentOrder the group is represented by a single sdmx:ComponentSpecification which in turn lists the child components by means of this property"@en ;
        rdfs:domain   sdmx:ComponentSpecification ;
        rdfs:label    "child components"@en ;
        rdfs:range    rdf:List .

sdmx-metadata:contactName
        a                   sdmx:MetadataProperty , rdf:Property ;
        rdfs:comment        "The name of the contact points for the data or metadata."@en ;
        rdfs:isDefinedBy    <http://sdmx.org/wp-content/uploads/2009/01/01_sdmx_cog_annex_1_cdc_2009.pdf> ;
        rdfs:label          "Contact name"@en ;
        rdfs:subPropertyOf  vcard:fn ;
        qb:concept          sdmx-concept:contactName .

sdmx-concept:comparGeo
        a                 sdmx:Concept , skos:Concept ;
        rdfs:comment      "Extent to which statistics are comparable between geographical areas."@en ;
        rdfs:isDefinedBy  <http://sdmx.org/wp-content/uploads/2009/01/01_sdmx_cog_annex_1_cdc_2009.pdf> ;
        rdfs:label        "Comparability - geographical"@en ;
        skos:broader      sdmx-concept:comparability ;
        skos:inScheme     sdmx-concept:cog ;
        skos:notation     "urn:sdmx:org.sdmx.infomodel.conceptscheme.Concept=SDMX:CROSS_DOMAIN_CONCEPTS[1.0].COMPAR_GEO" .

sdmx-metadata:unitMeasDetail
        a                 sdmx:MetadataProperty , rdf:Property ;
        rdfs:comment      "Additional textual information on the unit of measure."@en ;
        rdfs:isDefinedBy  <http://sdmx.org/wp-content/uploads/2009/01/01_sdmx_cog_annex_1_cdc_2009.pdf> ;
        rdfs:label        "Unit of Measure Detail"@en ;
        qb:concept        sdmx-concept:unitMeasDetail .

sdmx-metadata:onlineDb
        a                 sdmx:MetadataProperty , rdf:Property ;
        rdfs:comment      "Information about on-line databases in which the disseminated data can be accessed."@en ;
        rdfs:isDefinedBy  <http://sdmx.org/wp-content/uploads/2009/01/01_sdmx_cog_annex_1_cdc_2009.pdf> ;
        rdfs:label        "Dissemination Format - online database"@en ;
        qb:concept        sdmx-concept:onlineDb .

sdmx-attribute:costBurden
        a                 qb:AttributeProperty , rdf:Property ;
        rdfs:comment      "Costs associated with the collection and production of a statistical product and burden on respondents."@en ;
        rdfs:isDefinedBy  <http://sdmx.org/wp-content/uploads/2009/01/01_sdmx_cog_annex_1_cdc_2009.pdf> ;
        rdfs:label        "Cost and Burden"@en ;
        qb:concept        sdmx-concept:costBurden .

sdmx:ComponentSpecification
        a             rdfs:Class , owl:Class ;
        rdfs:comment  "Used to define properties of a component (attribute, dimension etc) which are specific to its usage in a DSD or MSD. This is used by including instances of sdmx:ComponentSpecification in place of the sdmx:ComponentProperty in an sdmx:componentOrder list"@en ;
        rdfs:label    "Component specification"@en .

sdmx-subject:2.3  a      skos:Concept , sdmx:Concept , sdmx-subject:SubjectMatterDomain ;
        skos:broader     sdmx-subject:2 ;
        skos:definition  "Business statistics - economy wide statistics on the activities of enterprises, covers work on economic statistics across different sectors (as opposed to 2.4 that deals with specific individual sectors), deals with topics like statistics on economic activities of enterprises, business demography, business investment, business services, demand for services, industrial performance, enterprises by size class, industrial production, commodities, structure of sales and services, outputs of the service industries, non-profit institutions.\nExcludes:\n- business tendency surveys (2.1)\n- international trade (2.6)\n- prices (2.7)\n- labour cost (2.8)\n- science and technology (2.9)\n- ICT (3.3.3)\n- activities of foreign affiliates and multinational companies (3.3.4)"@en ;
        skos:notation    "2.3" ;
        skos:prefLabel   "Business statistics"@en .

sdmx-concept:freqDetail
        a                 sdmx:Concept , skos:Concept ;
        rdfs:comment      "A further specification of the frequency to include more detailed information about the type of frequency and frequencies not commonly used."@en ;
        rdfs:isDefinedBy  <http://sdmx.org/wp-content/uploads/2009/01/01_sdmx_cog_annex_1_cdc_2009.pdf> ;
        rdfs:label        "Frequency Detail"@en ;
        skos:broader      sdmx-concept:freq ;
        skos:inScheme     sdmx-concept:cog ;
        skos:notation     "urn:sdmx:org.sdmx.infomodel.conceptscheme.Concept=SDMX:CROSS_DOMAIN_CONCEPTS[1.0].FREQ_DETAIL" .

sdmx-metadata:organisationUnit
        a                   sdmx:MetadataProperty , rdf:Property ;
        rdfs:comment        "An addressable subdivision of an organization."@en ;
        rdfs:isDefinedBy    <http://sdmx.org/wp-content/uploads/2009/01/01_sdmx_cog_annex_1_cdc_2009.pdf> ;
        rdfs:label          "Contact organization unit"@en ;
        rdfs:subPropertyOf  vcard:organization-unit ;
        qb:concept          sdmx-concept:organisationUnit .

sdmx-concept:contactPhone
        a                 sdmx:Concept , skos:Concept ;
        rdfs:comment      "The telephone number of the contact points for the data or metadata."@en ;
        rdfs:isDefinedBy  <http://sdmx.org/wp-content/uploads/2009/01/01_sdmx_cog_annex_1_cdc_2009.pdf> ;
        rdfs:label        "Contact phone number"@en ;
        skos:broader      sdmx-concept:contact ;
        skos:inScheme     sdmx-concept:cog ;
        skos:notation     "urn:sdmx:org.sdmx.infomodel.conceptscheme.Concept=SDMX:CROSS_DOMAIN_CONCEPTS[1.0].CONTACT_PHONE" .

sdmx-metadata:area  a  qb:CodedProperty ;
        rdfs:range   sdmx-code:Area ;
        qb:codeList  sdmx-code:area .

sdmx-concept:freq  a      sdmx:Concept , skos:Concept , sdmx:FrequencyRole ;
        rdfs:comment      "The time interval at which observations occur over a given time period."@en ;
        rdfs:isDefinedBy  <http://sdmx.org/wp-content/uploads/2009/01/01_sdmx_cog_annex_1_cdc_2009.pdf> ;
        rdfs:label        "Frequency"@en ;
        skos:inScheme     sdmx-concept:cog ;
        skos:notation     "urn:sdmx:org.sdmx.infomodel.conceptscheme.Concept=SDMX:CROSS_DOMAIN_CONCEPTS[1.0].FREQ" .

sdmx-metadata:dataValSource
        a                 sdmx:MetadataProperty , rdf:Property ;
        rdfs:comment      "Assessment of discrepancies and other problems related to source data."@en ;
        rdfs:isDefinedBy  <http://sdmx.org/wp-content/uploads/2009/01/01_sdmx_cog_annex_1_cdc_2009.pdf> ;
        rdfs:label        "Data Validation - source"@en ;
        qb:concept        sdmx-concept:dataValSource .

sdmx-metadata:sex  a      sdmx:MetadataProperty , rdf:Property , qb:CodedProperty ;
        rdfs:comment      "The state of being male or female."@en ;
        rdfs:isDefinedBy  <http://sdmx.org/wp-content/uploads/2009/01/01_sdmx_cog_annex_1_cdc_2009.pdf> ;
        rdfs:label        "Sex"@en ;
        rdfs:range        sdmx-code:Sex ;
        qb:codeList       sdmx-code:sex ;
        qb:concept        sdmx-concept:sex .

sdmx-concept:costBurdenRes
        a                 sdmx:Concept , skos:Concept ;
        rdfs:comment      "Staff, facilities, computing resources, and financing to undertake statistical production."@en ;
        rdfs:isDefinedBy  <http://sdmx.org/wp-content/uploads/2009/01/01_sdmx_cog_annex_1_cdc_2009.pdf> ;
        rdfs:label        "Cost and Burden - resources"@en ;
        skos:broader      sdmx-concept:costBurden ;
        skos:inScheme     sdmx-concept:cog ;
        skos:notation     "urn:sdmx:org.sdmx.infomodel.conceptscheme.Concept=SDMX:CROSS_DOMAIN_CONCEPTS[1.0].COST_BURDEN_RES" .

sdmx-attribute:dissOrg
        a                 qb:AttributeProperty , rdf:Property ;
        rdfs:comment      "The organisation disseminating the data."@en ;
        rdfs:isDefinedBy  <http://sdmx.org/wp-content/uploads/2009/01/01_sdmx_cog_annex_1_cdc_2009.pdf> ;
        rdfs:label        "Data Dissemination Agency"@en ;
        qb:concept        sdmx-concept:dissOrg .

sdmx-code:decimals-7  a    skos:Concept , sdmx:Concept , sdmx-code:Decimals ;
        skos:inScheme      sdmx-code:decimals ;
        skos:notation      "7" ;
        skos:prefLabel     "Seven"@en ;
        skos:topConceptOf  sdmx-code:decimals .

sdmx-concept:refPeriod
        a                 sdmx:Concept , skos:Concept , sdmx:TimeRole ;
        rdfs:comment      "The period of time or point in time to which the measured observation is intended to refer."@en ;
        rdfs:isDefinedBy  <http://sdmx.org/wp-content/uploads/2009/01/01_sdmx_cog_annex_1_cdc_2009.pdf> ;
        rdfs:label        "Reference Period"@en ;
        skos:inScheme     sdmx-concept:cog ;
        skos:notation     "urn:sdmx:org.sdmx.infomodel.conceptscheme.Concept=SDMX:CROSS_DOMAIN_CONCEPTS[1.0].REF_PERIOD" .

sdmx-subject:3.4  a      skos:Concept , sdmx:Concept , sdmx-subject:SubjectMatterDomain ;
        skos:broader     sdmx-subject:3 ;
        skos:definition  "Yearbooks and similar compendia - multi-domain statistical publications, databases and other data products without specific thematic or issue-oriented focus.\nExcludes:\n- Multi-domain statistical products based on specific thematic approaches, like sustainable development, MDGs etc. (under 3.3.1 to 3.3.5)"@en ;
        skos:notation    "3.4" ;
        skos:prefLabel   "Yearbooks and similar compendia"@en .

sdmx-metadata:contactEmail
        a                   sdmx:MetadataProperty , rdf:Property ;
        rdfs:comment        "E-mail address of the contact points for the data or metadata."@en ;
        rdfs:isDefinedBy    <http://sdmx.org/wp-content/uploads/2009/01/01_sdmx_cog_annex_1_cdc_2009.pdf> ;
        rdfs:label          "Contact email address"@en ;
        rdfs:subPropertyOf  vcard:email ;
        qb:concept          sdmx-concept:contactEmail .

sdmx-attribute:contactEmail
        a                 qb:AttributeProperty , rdf:Property ;
        rdfs:comment      "E-mail address of the contact points for the data or metadata."@en ;
        rdfs:isDefinedBy  <http://sdmx.org/wp-content/uploads/2009/01/01_sdmx_cog_annex_1_cdc_2009.pdf> ;
        rdfs:label        "Contact email address"@en ;
        qb:concept        sdmx-concept:contactEmail .

sdmx-metadata:comparDomains
        a                 sdmx:MetadataProperty , rdf:Property ;
        rdfs:comment      "Extent to which statistics are comparable between different statistical domains."@en ;
        rdfs:isDefinedBy  <http://sdmx.org/wp-content/uploads/2009/01/01_sdmx_cog_annex_1_cdc_2009.pdf> ;
        rdfs:label        "Comparability - between domains"@en ;
        qb:concept        sdmx-concept:comparDomains .

sdmx:Structured  a    rdfs:Class , owl:Class ;
        rdfs:comment  "Abstract class for things whose Structure can be defined by an sdmx:Structure declaration, alternative name: StructureUsage"@en ;
        rdfs:label    "Structured"@en .

sdmx:TimeProperty  a      rdfs:Class , owl:Class ;
        rdfs:label        "Time property"@en ;
        rdfs:subClassOf   sdmx:ConceptRoleProperty , sdmx:DimensionProperty ;
        owl:disjointWith  sdmx:MeasureProperty , sdmx:AttributeProperty .

sdmx:nonObsTimeProperty
        a                   rdf:Property , owl:ObjectProperty ;
        rdfs:comment        "identifies the Concept that plays the role of a date/time identifier in the KeyFamily which is not related to the time of the observation"@en ;
        rdfs:label          "non-observational time property"@en ;
        rdfs:range          sdmx:DimensionOrAttributeProperty ;
        rdfs:subPropertyOf  sdmx:component .

sdmx-attribute:userNeeds
        a                 qb:AttributeProperty , rdf:Property ;
        rdfs:comment      "Description of users and their respective needs with respect to the statistical data."@en ;
        rdfs:isDefinedBy  <http://sdmx.org/wp-content/uploads/2009/01/01_sdmx_cog_annex_1_cdc_2009.pdf> ;
        rdfs:label        "Relevance - user needs"@en ;
        qb:concept        sdmx-concept:userNeeds .

eg:o62  a                  qb:Observation ;
        eg:lifeExpectancy  83.4 ;
        eg:refArea         ex-geo:cardiff_00pt ;
        qb:dataSet         eg:dataset-le3 .

sdmx-code:sex-U  a         skos:Concept , sdmx:Concept , sdmx-code:Sex ;
        skos:inScheme      sdmx-code:sex ;
        skos:notation      "U" ;
        skos:prefLabel     "Not specified or unknown"@en ;
        skos:topConceptOf  sdmx-code:sex .

sdmx-concept:dataValInter
        a                 sdmx:Concept , skos:Concept ;
        rdfs:comment      "Validation that intermediate calculations leading to statistical outputs have been correctly done."@en ;
        rdfs:isDefinedBy  <http://sdmx.org/wp-content/uploads/2009/01/01_sdmx_cog_annex_1_cdc_2009.pdf> ;
        rdfs:label        "Data Validation - intermediate"@en ;
        skos:broader      sdmx-concept:dataValidation ;
        skos:inScheme     sdmx-concept:cog ;
        skos:notation     "urn:sdmx:org.sdmx.infomodel.conceptscheme.Concept=SDMX:CROSS_DOMAIN_CONCEPTS[1.0].DATA_VAL_INTER" .

sdmx-attribute:coherence
        a                 qb:AttributeProperty , rdf:Property ;
        rdfs:comment      "Adequacy of statistics to be combined in different ways and for various uses."@en ;
        rdfs:isDefinedBy  <http://sdmx.org/wp-content/uploads/2009/01/01_sdmx_cog_annex_1_cdc_2009.pdf> ;
        rdfs:label        "Coherence"@en ;
        qb:concept        sdmx-concept:coherence .

sdmx-attribute:dataDescr
        a                 qb:AttributeProperty , rdf:Property ;
        rdfs:comment      "Main characteristics of the data set described in an easily understandable manner, referring to the data and indicators disseminated."@en ;
        rdfs:isDefinedBy  <http://sdmx.org/wp-content/uploads/2009/01/01_sdmx_cog_annex_1_cdc_2009.pdf> ;
        rdfs:label        "Data Presentation - data description"@en ;
        qb:concept        sdmx-concept:dataDescr .

sdmx:Report  a           owl:Class , rdfs:Class ;
        rdfs:comment     "Represents a collection of data sets or flows which aren't required to have the same structure"@en ;
        rdfs:label       "Report"@en ;
        rdfs:subClassOf  sdmx:ReportEntry .

sdmx-attribute:sourceType
        a                 qb:AttributeProperty , rdf:Property ;
        rdfs:comment      "Characteristics and components of the raw statistical data used for compiling statistical aggregates."@en ;
        rdfs:isDefinedBy  <http://sdmx.org/wp-content/uploads/2009/01/01_sdmx_cog_annex_1_cdc_2009.pdf> ;
        rdfs:label        "Source Data"@en ;
        qb:concept        sdmx-concept:sourceType .

sdmx-attribute:coverage
        a                 qb:AttributeProperty , rdf:Property ;
        rdfs:comment      "The definition of the population that statistics aim to cover."@en ;
        rdfs:isDefinedBy  <http://sdmx.org/wp-content/uploads/2009/01/01_sdmx_cog_annex_1_cdc_2009.pdf> ;
        rdfs:label        "Coverage"@en ;
        qb:concept        sdmx-concept:coverage .

sdmx-concept:freqColl
        a                 sdmx:Concept , skos:Concept ;
        rdfs:comment      "Frequency with which the source data are collected."@en ;
        rdfs:isDefinedBy  <http://sdmx.org/wp-content/uploads/2009/01/01_sdmx_cog_annex_1_cdc_2009.pdf> ;
        rdfs:label        "Frequency of data collection"@en ;
        skos:broader      sdmx-concept:freq ;
        skos:inScheme     sdmx-concept:cog ;
        skos:notation     "urn:sdmx:org.sdmx.infomodel.conceptscheme.Concept=SDMX:CROSS_DOMAIN_CONCEPTS[1.0].FREQ_COLL" .

sdmx-metadata:freqColl
        a                 sdmx:MetadataProperty , rdf:Property ;
        rdfs:comment      "Frequency with which the source data are collected."@en ;
        rdfs:isDefinedBy  <http://sdmx.org/wp-content/uploads/2009/01/01_sdmx_cog_annex_1_cdc_2009.pdf> ;
        rdfs:label        "Frequency of data collection"@en ;
        qb:concept        sdmx-concept:freqColl .

sdmx-measure:occupation
        a                 qb:MeasureProperty , rdf:Property ;
        rdfs:comment      "Job or position held by an individual who performs a set of tasks and duties."@en ;
        rdfs:isDefinedBy  <http://sdmx.org/wp-content/uploads/2009/01/01_sdmx_cog_annex_1_cdc_2009.pdf> ;
        rdfs:label        "Occupation"@en ;
        qb:concept        sdmx-concept:occupation .

sdmx:frequencyProperty
        a                   rdf:Property , owl:ObjectProperty , owl:FunctionalProperty ;
        rdfs:comment        "identifies the Concept that plays the role of frequency"@en ;
        rdfs:label          "frequency property"@en ;
        rdfs:range          sdmx:DimensionOrAttributeProperty ;
        rdfs:subPropertyOf  sdmx:component .

sdmx-metadata:dissFormat
        a                 sdmx:MetadataProperty , rdf:Property ;
        rdfs:comment      "Media by which statistical data and metadata are disseminated."@en ;
        rdfs:isDefinedBy  <http://sdmx.org/wp-content/uploads/2009/01/01_sdmx_cog_annex_1_cdc_2009.pdf> ;
        rdfs:label        "Dissemination Format"@en ;
        qb:concept        sdmx-concept:dissFormat .

sdmx:MetadataSet  a   rdfs:Class , owl:Class ;
        rdfs:comment  "A collection of metadata resports"@en ;
        rdfs:label    "Metadata set"@en .

sdmx-dimension:occupation
        a                 qb:DimensionProperty , rdf:Property ;
        rdfs:comment      "Job or position held by an individual who performs a set of tasks and duties."@en ;
        rdfs:isDefinedBy  <http://sdmx.org/wp-content/uploads/2009/01/01_sdmx_cog_annex_1_cdc_2009.pdf> ;
        rdfs:label        "Occupation"@en ;
        rdfs:range        rdfs:Resource ;
        qb:concept        sdmx-concept:occupation .

sdmx-subject:1.11  a     skos:Concept , sdmx:Concept , sdmx-subject:SubjectMatterDomain ;
        skos:broader     sdmx-subject:1 ;
        skos:definition  ""@en ;
        skos:notation    "1.11" ;
        skos:prefLabel   "Time use"@en .

sdmx-metadata:refPeriod
        a                 sdmx:MetadataProperty , rdf:Property ;
        rdfs:comment      "The period of time or point in time to which the measured observation is intended to refer."@en ;
        rdfs:isDefinedBy  <http://sdmx.org/wp-content/uploads/2009/01/01_sdmx_cog_annex_1_cdc_2009.pdf> ;
        rdfs:label        "Reference Period"@en ;
        qb:concept        sdmx-concept:refPeriod .

sdmx:MetadataFlow  a     rdfs:Class , owl:Class ;
        rdfs:comment     "A flow of Metadata sets"@en ;
        rdfs:label       "Metadata flow"@en ;
        rdfs:subClassOf  sdmx:Structured , sdmx:Flow .

sdmx-metadata:embargoTime
        a                 sdmx:MetadataProperty , rdf:Property ;
        rdfs:comment      "The exact time at which the data could be made available to the public."@en ;
        rdfs:isDefinedBy  <http://sdmx.org/wp-content/uploads/2009/01/01_sdmx_cog_annex_1_cdc_2009.pdf> ;
        rdfs:label        "Embargo Time"@en ;
        qb:concept        sdmx-concept:embargoTime .

sdmx-attribute:grossNet
        a                 qb:AttributeProperty , rdf:Property ;
        rdfs:comment      "Form of consolidation used in presenting the data."@en ;
        rdfs:isDefinedBy  <http://sdmx.org/wp-content/uploads/2009/01/01_sdmx_cog_annex_1_cdc_2009.pdf> ;
        rdfs:label        "Grossing/Netting"@en ;
        qb:concept        sdmx-concept:grossNet .

sdmx-attribute:revPolicy
        a                 qb:AttributeProperty , rdf:Property ;
        rdfs:comment      "Policy aimed at ensuring the transparency of disseminated data, whereby preliminary data are compiled that are later revised."@en ;
        rdfs:isDefinedBy  <http://sdmx.org/wp-content/uploads/2009/01/01_sdmx_cog_annex_1_cdc_2009.pdf> ;
        rdfs:label        "Data Revision - policy"@en ;
        qb:concept        sdmx-concept:revPolicy .

sdmx-concept:cog  a       skos:ConceptScheme ;
        rdfs:isDefinedBy  <http://sdmx.org/wp-content/uploads/2009/01/01_sdmx_cog_annex_1_cdc_2009.pdf> ;
        rdfs:label        "Content Oriented Guidelines concept scheme"@en .

sdmx-concept:dataValOutput
        a                 sdmx:Concept , skos:Concept ;
        rdfs:comment      "Assessment of discrepancies and other problems in statistical outputs."@en ;
        rdfs:isDefinedBy  <http://sdmx.org/wp-content/uploads/2009/01/01_sdmx_cog_annex_1_cdc_2009.pdf> ;
        rdfs:label        "Data Validation - output"@en ;
        skos:broader      sdmx-concept:dataValidation ;
        skos:inScheme     sdmx-concept:cog ;
        skos:notation     "urn:sdmx:org.sdmx.infomodel.conceptscheme.Concept=SDMX:CROSS_DOMAIN_CONCEPTS[1.0].DATA_VAL_OUTPUT" .

sdmx-concept:qualityMgmnt
        a                 sdmx:Concept , skos:Concept ;
        rdfs:comment      "Systems and frameworks in place within an organisation to manage the quality of statistical products and processes."@en ;
        rdfs:isDefinedBy  <http://sdmx.org/wp-content/uploads/2009/01/01_sdmx_cog_annex_1_cdc_2009.pdf> ;
        rdfs:label        "Quality Management"@en ;
        skos:inScheme     sdmx-concept:cog ;
        skos:notation     "urn:sdmx:org.sdmx.infomodel.conceptscheme.Concept=SDMX:CROSS_DOMAIN_CONCEPTS[1.0].QUALITY_MGMNT" .

sdmx-code:decimals-2  a    skos:Concept , sdmx:Concept , sdmx-code:Decimals ;
        skos:inScheme      sdmx-code:decimals ;
        skos:notation      "2" ;
        skos:prefLabel     "Two"@en ;
        skos:topConceptOf  sdmx-code:decimals .

sdmx-concept:dataValSource
        a                 sdmx:Concept , skos:Concept ;
        rdfs:comment      "Assessment of discrepancies and other problems related to source data."@en ;
        rdfs:isDefinedBy  <http://sdmx.org/wp-content/uploads/2009/01/01_sdmx_cog_annex_1_cdc_2009.pdf> ;
        rdfs:label        "Data Validation - source"@en ;
        skos:broader      sdmx-concept:dataValidation ;
        skos:inScheme     sdmx-concept:cog ;
        skos:notation     "urn:sdmx:org.sdmx.infomodel.conceptscheme.Concept=SDMX:CROSS_DOMAIN_CONCEPTS[1.0].DATA_VAL_SOURCE" .

sdmx-attribute:unitMeasure
        a                 qb:AttributeProperty , rdf:Property ;
        rdfs:comment      "The unit in which the data values are measured."@en ;
        rdfs:isDefinedBy  <http://sdmx.org/wp-content/uploads/2009/01/01_sdmx_cog_annex_1_cdc_2009.pdf> ;
        rdfs:label        "Unit of Measure"@en ;
        qb:concept        sdmx-concept:unitMeasure .

sdmx-metadata:metaUpdate
        a                 sdmx:MetadataProperty , rdf:Property ;
        rdfs:comment      "The date on which the metadata element was inserted or modified in the database."@en ;
        rdfs:isDefinedBy  <http://sdmx.org/wp-content/uploads/2009/01/01_sdmx_cog_annex_1_cdc_2009.pdf> ;
        rdfs:label        "Metadata Update"@en ;
        qb:concept        sdmx-concept:metaUpdate .

sdmx-code:unitMult  a       skos:ConceptScheme , sdmx:CodeList ;
        rdfs:label          "code list for the Unit Multiplier (UNIT_MULT) - codelist scheme"@en ;
        rdfs:seeAlso        sdmx-code:UnitMult ;
        skos:definition     <http://sdmx.org/wp-content/uploads/2009/01/02_sdmx_cog_annex_2_cl_2009.pdf> ;
        skos:hasTopConcept  sdmx-code:unitMult-2 , sdmx-code:unitMult-6 , sdmx-code:unitMult-3 , sdmx-code:unitMult-1 , sdmx-code:unitMult-0 , sdmx-code:unitMult-4 , sdmx-code:unitMult-12 , sdmx-code:unitMult-9 , sdmx-code:unitMult-15 ;
        skos:notation       "CL_UNIT_MULT" ;
        skos:note           "it provides code values for indicating the magnitude in the units of measurements."@en ;
        skos:prefLabel      "code list for the Unit Multiplier (UNIT_MULT) - codelist scheme"@en .

eg:o43  a                  qb:Observation ;
        eg:lifeExpectancy  81.5 ;
        eg:refArea         ex-geo:monmouthshire_00pp ;
        qb:dataSet         eg:dataset-le3 .

sdmx-metadata:conf  a     sdmx:MetadataProperty , rdf:Property ;
        rdfs:comment      "A property of data indicating the extent to which their unauthorised disclosure could be prejudicial or harmful to the interest of the source or other relevant parties."@en ;
        rdfs:isDefinedBy  <http://sdmx.org/wp-content/uploads/2009/01/01_sdmx_cog_annex_1_cdc_2009.pdf> ;
        rdfs:label        "Confidentiality"@en ;
        qb:concept        sdmx-concept:conf .

sdmx-concept:dissFormat
        a                 sdmx:Concept , skos:Concept ;
        rdfs:comment      "Media by which statistical data and metadata are disseminated."@en ;
        rdfs:isDefinedBy  <http://sdmx.org/wp-content/uploads/2009/01/01_sdmx_cog_annex_1_cdc_2009.pdf> ;
        rdfs:label        "Dissemination Format"@en ;
        skos:inScheme     sdmx-concept:cog ;
        skos:notation     "urn:sdmx:org.sdmx.infomodel.conceptscheme.Concept=SDMX:CROSS_DOMAIN_CONCEPTS[1.0].DISS_FORMAT" .

sdmx-code:unitMult-3  a    skos:Concept , sdmx:Concept , sdmx-code:UnitMult ;
        skos:inScheme      sdmx-code:unitMult ;
        skos:notation      "3" ;
        skos:prefLabel     "Thousands"@en ;
        skos:topConceptOf  sdmx-code:unitMult .

eg:o11  a                  qb:Observation ;
        eg:lifeExpectancy  76.7 ;
        eg:refArea         ex-geo:newport_00pr ;
        qb:dataSet         eg:dataset-le3 .

sdmx-metadata:adjustDetail
        a                 sdmx:MetadataProperty , rdf:Property ;
        rdfs:comment      "Textual description of the type of adjustment used."@en ;
        rdfs:isDefinedBy  <http://sdmx.org/wp-content/uploads/2009/01/01_sdmx_cog_annex_1_cdc_2009.pdf> ;
        rdfs:label        "Adjustment - detail"@en ;
        qb:concept        sdmx-concept:adjustDetail .

sdmx-code:obsStatus-P
        a                  skos:Concept , sdmx:Concept , sdmx-code:ObsStatus ;
        skos:definition    "An observation is characterised as \"provisional\" when the source agency - while it bases its calculations on its standard production methodology - considers that the data, almost certainly, are expected to be revised."@en ;
        skos:inScheme      sdmx-code:obsStatus ;
        skos:notation      "P" ;
        skos:prefLabel     "Provisional value"@en ;
        skos:topConceptOf  sdmx-code:obsStatus .

sdmx-metadata:dataEditing
        a                 sdmx:MetadataProperty , rdf:Property ;
        rdfs:comment      "Activity aimed at detecting and correcting errors, logical inconsistencies and suspicious data."@en ;
        rdfs:isDefinedBy  <http://sdmx.org/wp-content/uploads/2009/01/01_sdmx_cog_annex_1_cdc_2009.pdf> ;
        rdfs:label        "Data Editing"@en ;
        qb:concept        sdmx-concept:dataEditing .

sdmx-attribute:adjustDetail
        a                 qb:AttributeProperty , rdf:Property ;
        rdfs:comment      "Textual description of the type of adjustment used."@en ;
        rdfs:isDefinedBy  <http://sdmx.org/wp-content/uploads/2009/01/01_sdmx_cog_annex_1_cdc_2009.pdf> ;
        rdfs:label        "Adjustment - detail"@en ;
        qb:concept        sdmx-concept:adjustDetail .

sdmx-code:timeFormat  a     skos:ConceptScheme , sdmx:CodeList ;
        rdfs:label          "Code list for the Time Format as written in the SDMX-EDI and SDMX-ML messages - codelist scheme"@en ;
        rdfs:seeAlso        sdmx-code:TimeFormat ;
        skos:definition     <http://sdmx.org/wp-content/uploads/2009/01/02_sdmx_cog_annex_2_cl_2009.pdf> ;
        skos:hasTopConcept  sdmx-code:timeFormat-604 , sdmx-code:timeFormat-708 , sdmx-code:timeFormat-710 , sdmx-code:timeFormat-102 , sdmx-code:timeFormat-P3M , sdmx-code:timeFormat-719 , sdmx-code:timeFormat-PT1M , sdmx-code:timeFormat-602 , sdmx-code:timeFormat-610 , sdmx-code:timeFormat-608 , sdmx-code:timeFormat-P6M , sdmx-code:timeFormat-P1D , sdmx-code:timeFormat-716 , sdmx-code:timeFormat-P1M , sdmx-code:timeFormat-P1Y , sdmx-code:timeFormat-616 , sdmx-code:timeFormat-203 , sdmx-code:timeFormat-704 , sdmx-code:timeFormat-P7D , sdmx-code:timeFormat-711 , sdmx-code:timeFormat-702 ;
        skos:notation       "CL_TIME_FORMAT" ;
        skos:note           "These codes (based on the ISO 8601 standard) indicate the type of time references used in the data. The numeric codes below (203, 102,...,702) are used only in the SDMX-EDI messages; and the alphanumeric codes (P1D...PT1M) only in the SDMX-ML messages."@en ;
        skos:prefLabel      "Code list for the Time Format as written in the SDMX-EDI and SDMX-ML messages - codelist scheme"@en .

eg:slice6  a                qb:Slice ;
        eg:refPeriod        <http://reference.data.gov.uk/id/gregorian-interval/2006-01-01T00:00:00/P3Y> ;
        qb:observation      eg:o61 , eg:o62 , eg:o63 , eg:o64 ;
        qb:sliceStructure   eg:sliceByRegion ;
        sdmx-dimension:sex  sdmx-code:sex-F .

sdmx-code:freq  a           sdmx:CodeList , skos:ConceptScheme ;
        rdfs:label          "Code list for Frequency (FREQ) - codelist scheme"@en ;
        rdfs:seeAlso        sdmx-code:Freq ;
        skos:definition     <http://sdmx.org/wp-content/uploads/2009/01/02_sdmx_cog_annex_2_cl_2009.pdf> ;
        skos:hasTopConcept  sdmx-code:freq-D , sdmx-code:freq-W , sdmx-code:freq-M , sdmx-code:freq-B , sdmx-code:freq-Q , sdmx-code:freq-S , sdmx-code:freq-N , sdmx-code:freq-A ;
        skos:notation       "CL_FREQ" ;
        skos:note           "It provides a list of values indicating the \"frequency\" of the data (e.g. monthly) and, thus, indirectly, also implying the type of \"time reference\" that could be used for identifying the data with respect time."@en ;
        skos:prefLabel      "Code list for Frequency (FREQ) - codelist scheme"@en .

sdmx:coreType  a     rdf:Property , owl:ObjectProperty ;
        rdfs:domain  skos:Concept ;
        rdfs:label   "core type"@en ;
        rdfs:range   rdf:Datatype .

sdmx-subject:1.9  a      skos:Concept , sdmx:Concept , sdmx-subject:SubjectMatterDomain ;
        skos:broader     sdmx-subject:1 ;
        skos:definition  "Culture - statistics dealing with cultural activities in society, like theatre, cinemas, museums, libraries, mass media, book production, sports, etc., including expenditure and financing of culture."@en ;
        skos:notation    "1.9" ;
        skos:prefLabel   "Culture"@en .

sdmx-attribute:samplingErr
        a                 qb:AttributeProperty , rdf:Property ;
        rdfs:comment      "That part of the difference between a population value and an estimate thereof, derived from a random sample, which is due to the fact that only a subset of the population is enumerated."@en ;
        rdfs:isDefinedBy  <http://sdmx.org/wp-content/uploads/2009/01/01_sdmx_cog_annex_1_cdc_2009.pdf> ;
        rdfs:label        "Accuracy - sampling error"@en ;
        qb:concept        sdmx-concept:samplingErr .

sdmx:FrequencyRole  a    rdfs:Class , owl:Class ;
        rdfs:comment     "concept for a dimension or attribute that plays the role of frequency"@en ;
        rdfs:label       "Frequency property"@en ;
        rdfs:subClassOf  sdmx:ConceptRole .

eg:dataset-le3  a                   qb:DataSet ;
        rdfs:comment                "Life expectancy within Welsh Unitary authorities - extracted from Stats Wales"@en ;
        rdfs:label                  "Life expectancy"@en ;
        dct:description             "Life expectancy within Welsh Unitary authorities - extracted from Stats Wales"@en ;
        dct:issued                  "2010-08-11"^^xsd:date ;
        dct:publisher               eg:organization ;
        dct:subject                 ex-geo:wales , sdmx-subject:1.4 , sdmx-subject:3.2 ;
        dct:title                   "Life expectancy"@en ;
        qb:slice                    eg:slice1 , eg:slice6 , eg:slice4 , eg:slice5 , eg:slice2 , eg:slice3 ;
        qb:structure                eg:dsd-le3 ;
        sdmx-attribute:unitMeasure  <http://dbpedia.org/resource/Year> .

sdmx-concept:metaUpdate
        a                 sdmx:Concept , skos:Concept ;
        rdfs:comment      "The date on which the metadata element was inserted or modified in the database."@en ;
        rdfs:isDefinedBy  <http://sdmx.org/wp-content/uploads/2009/01/01_sdmx_cog_annex_1_cdc_2009.pdf> ;
        rdfs:label        "Metadata Update"@en ;
        skos:inScheme     sdmx-concept:cog ;
        skos:notation     "urn:sdmx:org.sdmx.infomodel.conceptscheme.Concept=SDMX:CROSS_DOMAIN_CONCEPTS[1.0].META_UPDATE" .

sdmx:DimensionOrAttributeProperty
        a             rdfs:Class , owl:class ;
        rdfs:comment  "union of the class of dimension or attribute properties, used to denote allowed range for some roles"@en ;
        rdfs:label    "dimension or attribute"@en ;
        owl:unionOf   ( sdmx:DimensionProperty sdmx:AttributeProperty ) .

sdmx-attribute:instMandate
        a                 qb:AttributeProperty , rdf:Property ;
        rdfs:comment      "Set of rules or other formal set of instructions assigning responsibility as well as the authority to an organisation for the collection, processing, and dissemination of statistics."@en ;
        rdfs:isDefinedBy  <http://sdmx.org/wp-content/uploads/2009/01/01_sdmx_cog_annex_1_cdc_2009.pdf> ;
        rdfs:label        "Institutional Mandate"@en ;
        qb:concept        sdmx-concept:instMandate .

sdmx-metadata:microDatAcc
        a                 sdmx:MetadataProperty , rdf:Property ;
        rdfs:comment      "Information on whether micro-data are also disseminated."@en ;
        rdfs:isDefinedBy  <http://sdmx.org/wp-content/uploads/2009/01/01_sdmx_cog_annex_1_cdc_2009.pdf> ;
        rdfs:label        "Dissemination Format - mirco-data access"@en ;
        qb:concept        sdmx-concept:microDatAcc .

sdmx-attribute:statConcDef
        a                 qb:AttributeProperty , rdf:Property ;
        rdfs:comment      "Statistical characteristics of statistical observations."@en ;
        rdfs:isDefinedBy  <http://sdmx.org/wp-content/uploads/2009/01/01_sdmx_cog_annex_1_cdc_2009.pdf> ;
        rdfs:label        "Statistical Concepts and Definitions"@en ;
        qb:concept        sdmx-concept:statConcDef .

sdmx-concept:accuracyOverall
        a                 sdmx:Concept , skos:Concept ;
        rdfs:comment      "Assessment of accuracy, linked to a certain data set or domain, which is summarising the various components into one single measure."@en ;
        rdfs:isDefinedBy  <http://sdmx.org/wp-content/uploads/2009/01/01_sdmx_cog_annex_1_cdc_2009.pdf> ;
        rdfs:label        "Accuracy - overall"@en ;
        skos:broader      sdmx-concept:accuracy ;
        skos:inScheme     sdmx-concept:cog ;
        skos:notation     "urn:sdmx:org.sdmx.infomodel.conceptscheme.Concept=SDMX:CROSS_DOMAIN_CONCEPTS[1.0].ACCURACY_OVERALL" .

sdmx:IdentityRole  a     rdfs:Class , owl:Class ;
        rdfs:comment     "concept for a dimension or attribute that plays the role of an identifier which is taken from a known scheme of identifiers."@en ;
        rdfs:label       "Identity property"@en ;
        rdfs:subClassOf  sdmx:ConceptRole .

sdmx-code:timeFormat-702
        a                  skos:Concept , sdmx:Concept , sdmx-code:TimeFormat ;
        skos:definition    "(for annual series)\nfrom year to year"@en ;
        skos:inScheme      sdmx-code:timeFormat ;
        skos:notation      "702" ;
        skos:prefLabel     "CCYYCCYY"@en ;
        skos:topConceptOf  sdmx-code:timeFormat .

sdmx-metadata:dataPres
        a                 sdmx:MetadataProperty , rdf:Property ;
        rdfs:comment      "Description of the disseminated data."@en ;
        rdfs:isDefinedBy  <http://sdmx.org/wp-content/uploads/2009/01/01_sdmx_cog_annex_1_cdc_2009.pdf> ;
        rdfs:label        "Data Presentation"@en ;
        qb:concept        sdmx-concept:dataPres .

sdmx-metadata:coverageTime
        a                 sdmx:MetadataProperty , rdf:Property ;
        rdfs:comment      "The length of time for which data are available."@en ;
        rdfs:isDefinedBy  <http://sdmx.org/wp-content/uploads/2009/01/01_sdmx_cog_annex_1_cdc_2009.pdf> ;
        rdfs:label        "Coverage- time"@en ;
        qb:concept        sdmx-concept:coverageTime .

eg:o24  a                  qb:Observation ;
        eg:lifeExpectancy  79.1 ;
        eg:refArea         ex-geo:merthyr_tdfil_00ph ;
        qb:dataSet         eg:dataset-le3 .

sdmx-attribute:coverageTime
        a                 qb:AttributeProperty , rdf:Property ;
        rdfs:comment      "The length of time for which data are available."@en ;
        rdfs:isDefinedBy  <http://sdmx.org/wp-content/uploads/2009/01/01_sdmx_cog_annex_1_cdc_2009.pdf> ;
        rdfs:label        "Coverage- time"@en ;
        qb:concept        sdmx-concept:coverageTime .

sdmx-subject:1  a          skos:Concept , sdmx:Concept , sdmx-subject:SubjectMatterDomain ;
        skos:definition    "Time-use - statistics on the use of time by individuals, often related to work-life balance (reconciling family responsibilities and paid work); unpaid work. \nExcludes \n- working time (1.2)"@en ;
        skos:notation      "1" ;
        skos:prefLabel     "Demographic and social statistics"@en ;
        skos:topConceptOf  sdmx-subject:subjectMatterDomain .

sdmx-concept:title  a     sdmx:Concept , skos:Concept ;
        rdfs:comment      "Textual label used as identification of a statistical object."@en ;
        rdfs:isDefinedBy  <http://sdmx.org/wp-content/uploads/2009/01/01_sdmx_cog_annex_1_cdc_2009.pdf> ;
        rdfs:label        "Title"@en ;
        skos:inScheme     sdmx-concept:cog ;
        skos:notation     "urn:sdmx:org.sdmx.infomodel.conceptscheme.Concept=SDMX:CROSS_DOMAIN_CONCEPTS[1.0].TITLE" .

sdmx-dimension:refArea
        a                 qb:DimensionProperty , rdf:Property ;
        rdfs:comment      "The country or geographic area to which the measured statistical phenomenon relates."@en ;
        rdfs:isDefinedBy  <http://sdmx.org/wp-content/uploads/2009/01/01_sdmx_cog_annex_1_cdc_2009.pdf> ;
        rdfs:label        "Reference Area"@en ;
        rdfs:range        rdfs:Resource ;
        qb:concept        sdmx-concept:refArea .

sdmx-metadata:coherXDom
        a                 sdmx:MetadataProperty , rdf:Property ;
        rdfs:comment      "Extent to which statistics are reconcilable with those obtained through other data sources or statistical domains."@en ;
        rdfs:isDefinedBy  <http://sdmx.org/wp-content/uploads/2009/01/01_sdmx_cog_annex_1_cdc_2009.pdf> ;
        rdfs:label        "Coherence - cross domain"@en ;
        qb:concept        sdmx-concept:coherXDom .

sdmx-metadata:confPolicy
        a                 sdmx:MetadataProperty , rdf:Property ;
        rdfs:comment      "Legislative measures or other formal procedures which prevent unauthorised disclosure of data that identify a person or economic entity either directly or indirectly."@en ;
        rdfs:isDefinedBy  <http://sdmx.org/wp-content/uploads/2009/01/01_sdmx_cog_annex_1_cdc_2009.pdf> ;
        rdfs:label        "Confidentiality - policy"@en ;
        qb:concept        sdmx-concept:confPolicy .

sdmx-concept:dissOrg  a   sdmx:Concept , skos:Concept ;
        rdfs:comment      "The organisation disseminating the data."@en ;
        rdfs:isDefinedBy  <http://sdmx.org/wp-content/uploads/2009/01/01_sdmx_cog_annex_1_cdc_2009.pdf> ;
        rdfs:label        "Data Dissemination Agency"@en ;
        skos:inScheme     sdmx-concept:cog ;
        skos:notation     "urn:sdmx:org.sdmx.infomodel.conceptscheme.Concept=SDMX:CROSS_DOMAIN_CONCEPTS[1.0].DISS_ORG" .

sdmx-metadata:accuracyOverall
        a                 sdmx:MetadataProperty , rdf:Property ;
        rdfs:comment      "Assessment of accuracy, linked to a certain data set or domain, which is summarising the various components into one single measure."@en ;
        rdfs:isDefinedBy  <http://sdmx.org/wp-content/uploads/2009/01/01_sdmx_cog_annex_1_cdc_2009.pdf> ;
        rdfs:label        "Accuracy - overall"@en ;
        qb:concept        sdmx-concept:accuracyOverall .

sdmx-code:confStatus-F
        a                  skos:Concept , sdmx:Concept , sdmx-code:ConfStatus ;
        skos:definition    "It is used for observations for observations for which there are no special sensitivity considerations and which can be freely shared. Please note:\nIn some institutional environments the term \"unclassified\" is used in a sense that still denotes implied restrictions in the circulation of information. If this is the case, this organisation may probably consider that \"free\" (value F) is not the appropriate corresponding tag for this kind of \"unclassified\" category and it may be that \"non-publishable / restricted\" (value N) may be more appropriate.\nThe focus of this code is not to describe and anticipate all potential permissible uses (e.g. permission to re-disseminate). Thus, the use of \"F\" does not allow safe assumptions with respect to the permission to \"re-disseminate\" (freely or at a price) the received or accessed information (e.g. on web or paper), especially on a massive and regular basis (legal and copyright constraints may apply). Usually, source organisations provide information and guidance on re-dissemination issues, either on their websites or on their paper publications."@en ;
        skos:inScheme      sdmx-code:confStatus ;
        skos:notation      "F" ;
        skos:prefLabel     "Free"@en ;
        skos:topConceptOf  sdmx-code:confStatus .

sdmx-subject:3.3.7  a    skos:Concept , sdmx:Concept , sdmx-subject:SubjectMatterDomain ;
        skos:broader     sdmx-subject:3.3 ;
        skos:definition  "Entrepreneurship - the measurement of the determinants, performance and impact of entrepreneurial activities of people and organisations."@en ;
        skos:notation    "3.3.7" ;
        skos:prefLabel   "Entrepreneurship"@en .

eg:slice1  a                qb:Slice ;
        eg:refPeriod        <http://reference.data.gov.uk/id/gregorian-interval/2004-01-01T00:00:00/P3Y> ;
        qb:observation      eg:o11 , eg:o12 , eg:o13 , eg:o14 ;
        qb:sliceStructure   eg:sliceByRegion ;
        sdmx-dimension:sex  sdmx-code:sex-M .

sdmx-metadata:costBurden
        a                 sdmx:MetadataProperty , rdf:Property ;
        rdfs:comment      "Costs associated with the collection and production of a statistical product and burden on respondents."@en ;
        rdfs:isDefinedBy  <http://sdmx.org/wp-content/uploads/2009/01/01_sdmx_cog_annex_1_cdc_2009.pdf> ;
        rdfs:label        "Cost and Burden"@en ;
        qb:concept        sdmx-concept:costBurden .

sdmx-concept:coverage
        a                 sdmx:Concept , skos:Concept ;
        rdfs:comment      "The definition of the population that statistics aim to cover."@en ;
        rdfs:isDefinedBy  <http://sdmx.org/wp-content/uploads/2009/01/01_sdmx_cog_annex_1_cdc_2009.pdf> ;
        rdfs:label        "Coverage"@en ;
        skos:inScheme     sdmx-concept:cog ;
        skos:notation     "urn:sdmx:org.sdmx.infomodel.conceptscheme.Concept=SDMX:CROSS_DOMAIN_CONCEPTS[1.0].COVERAGE" .

sdmx-attribute:metaLastUpdate
        a                 qb:AttributeProperty , rdf:Property ;
        rdfs:comment      "Date of last update of the content of the metadata."@en ;
        rdfs:isDefinedBy  <http://sdmx.org/wp-content/uploads/2009/01/01_sdmx_cog_annex_1_cdc_2009.pdf> ;
        rdfs:label        "Metadata Update - last update"@en ;
        qb:concept        sdmx-concept:metaLastUpdate .

sdmx-subject:2.4.3  a    skos:Concept , sdmx:Concept , sdmx-subject:SubjectMatterDomain ;
        skos:broader     sdmx-subject:2.4 ;
        skos:definition  "Mining, manufacturing, construction - statistics on specific industrial activities, e.g. steel, shipbuilding, and on construction, trade in specific products related to mining, manufacturing and construction.\nExcludes\n- prices of manufactured products (2.7)\n- construction prices (2.7)"@en ;
        skos:notation    "2.4.3" ;
        skos:prefLabel   "Mining, manufacturing, construction"@en .

sdmx:NonObsTimeProperty
        a                 rdfs:Class , owl:Class ;
        rdfs:label        "Non-observation time property"@en ;
        rdfs:subClassOf   sdmx:ConceptRoleProperty ;
        owl:disjointWith  sdmx:MeasureProperty .

sdmx-metadata:coverage
        a                 sdmx:MetadataProperty , rdf:Property ;
        rdfs:comment      "The definition of the population that statistics aim to cover."@en ;
        rdfs:isDefinedBy  <http://sdmx.org/wp-content/uploads/2009/01/01_sdmx_cog_annex_1_cdc_2009.pdf> ;
        rdfs:label        "Coverage"@en ;
        qb:concept        sdmx-concept:coverage .

sdmx-subject:1.4  a      skos:Concept , sdmx:Concept , sdmx-subject:SubjectMatterDomain ;
        skos:broader     sdmx-subject:1 ;
        skos:definition  "Health - covers the health and mortality related statistical activities, including topics like life expectancy, health status, health and safety, health determinants (including lifestyle, nutrition, smoking, alcohol abuse), health resources and expenditure, health care systems, morbidity and mortality (including infant and child mortality), hospital admission, causes of illness and death, specific diseases (e.g. AIDS), disabilities, pharmaceutical consumption and sales, health personnel, remuneration of health professions, environmental health status, health inequality, health accounts.\nExcludes \n- work related health and safety (1.2) \n- victimisation from criminal behaviour (1.8)\n- traffic accidents and injuries (2.4.4)"@en ;
        skos:notation    "1.4" ;
        skos:prefLabel   "Health"@en .

sdmx-metadata:comparability
        a                 sdmx:MetadataProperty , rdf:Property ;
        rdfs:comment      "The extent to which differences between statistics can be attributed to differences between the true values of the statistical characteristics."@en ;
        rdfs:isDefinedBy  <http://sdmx.org/wp-content/uploads/2009/01/01_sdmx_cog_annex_1_cdc_2009.pdf> ;
        rdfs:label        "Comparability"@en ;
        qb:concept        sdmx-concept:comparability .

sdmx-concept:confDataTr
        a                 sdmx:Concept , skos:Concept ;
        rdfs:comment      "Rules applied for treating the data set to ensure statistical confidentiality and prevent unauthorised disclosure."@en ;
        rdfs:isDefinedBy  <http://sdmx.org/wp-content/uploads/2009/01/01_sdmx_cog_annex_1_cdc_2009.pdf> ;
        rdfs:label        "Confidentiality - data treatment"@en ;
        skos:broader      sdmx-concept:conf ;
        skos:inScheme     sdmx-concept:cog ;
        skos:notation     "urn:sdmx:org.sdmx.infomodel.conceptscheme.Concept=SDMX:CROSS_DOMAIN_CONCEPTS[1.0].CONF_DATA_TR" .

sdmx-concept:qualityDoc
        a                 sdmx:Concept , skos:Concept ;
        rdfs:comment      "Documentation on procedures applied for quality management and quality assessment."@en ;
        rdfs:isDefinedBy  <http://sdmx.org/wp-content/uploads/2009/01/01_sdmx_cog_annex_1_cdc_2009.pdf> ;
        rdfs:label        "Quality Management - documentation"@en ;
        skos:broader      sdmx-concept:qualityMgmnt ;
        skos:inScheme     sdmx-concept:cog ;
        skos:notation     "urn:sdmx:org.sdmx.infomodel.conceptscheme.Concept=SDMX:CROSS_DOMAIN_CONCEPTS[1.0].QUALITY_DOC" .

sdmx-concept:timeOutput
        a                 sdmx:Concept , skos:Concept ;
        rdfs:comment      "The lapse of time between the end of a reference period and dissemination of the data."@en ;
        rdfs:isDefinedBy  <http://sdmx.org/wp-content/uploads/2009/01/01_sdmx_cog_annex_1_cdc_2009.pdf> ;
        rdfs:label        "Timeliness - output"@en ;
        skos:broader      sdmx-concept:timeliness ;
        skos:inScheme     sdmx-concept:cog ;
        skos:notation     "urn:sdmx:org.sdmx.infomodel.conceptscheme.Concept=SDMX:CROSS_DOMAIN_CONCEPTS[1.0].TIME_OUTPUT" .

sdmx-concept:unitMeasure
        a                 sdmx:Concept , skos:Concept ;
        rdfs:comment      "The unit in which the data values are measured."@en ;
        rdfs:isDefinedBy  <http://sdmx.org/wp-content/uploads/2009/01/01_sdmx_cog_annex_1_cdc_2009.pdf> ;
        rdfs:label        "Unit of Measure"@en ;
        skos:inScheme     sdmx-concept:cog ;
        skos:notation     "urn:sdmx:org.sdmx.infomodel.conceptscheme.Concept=SDMX:CROSS_DOMAIN_CONCEPTS[1.0].UNIT_MEASURE" .

sdmx-metadata:punctuality
        a                 sdmx:MetadataProperty , rdf:Property ;
        rdfs:comment      "Time lag between the actual delivery of the data and the target date when it should have been delivered."@en ;
        rdfs:isDefinedBy  <http://sdmx.org/wp-content/uploads/2009/01/01_sdmx_cog_annex_1_cdc_2009.pdf> ;
        rdfs:label        "Punctuality"@en ;
        qb:concept        sdmx-concept:punctuality .

sdmx-concept:grossNet
        a                 sdmx:Concept , skos:Concept ;
        rdfs:comment      "Form of consolidation used in presenting the data."@en ;
        rdfs:isDefinedBy  <http://sdmx.org/wp-content/uploads/2009/01/01_sdmx_cog_annex_1_cdc_2009.pdf> ;
        rdfs:label        "Grossing/Netting"@en ;
        skos:inScheme     sdmx-concept:cog ;
        skos:notation     "urn:sdmx:org.sdmx.infomodel.conceptscheme.Concept=SDMX:CROSS_DOMAIN_CONCEPTS[1.0].GROSS_NET" .

sdmx-concept:timeSource
        a                 sdmx:Concept , skos:Concept ;
        rdfs:comment      "The time between the end of a reference period and actual receipt of the data by the compiling agency."@en ;
        rdfs:isDefinedBy  <http://sdmx.org/wp-content/uploads/2009/01/01_sdmx_cog_annex_1_cdc_2009.pdf> ;
        rdfs:label        "Timeliness - source data"@en ;
        skos:broader      sdmx-concept:timeliness ;
        skos:inScheme     sdmx-concept:cog ;
        skos:notation     "urn:sdmx:org.sdmx.infomodel.conceptscheme.Concept=SDMX:CROSS_DOMAIN_CONCEPTS[1.0].TIME_SOURCE" .

sdmx-concept:prof  a      sdmx:Concept , skos:Concept ;
        rdfs:comment      "The standard, skill and ability suitable for producing statistics of good quality."@en ;
        rdfs:isDefinedBy  <http://sdmx.org/wp-content/uploads/2009/01/01_sdmx_cog_annex_1_cdc_2009.pdf> ;
        rdfs:label        "Professionalism"@en ;
        skos:inScheme     sdmx-concept:cog ;
        skos:notation     "urn:sdmx:org.sdmx.infomodel.conceptscheme.Concept=SDMX:CROSS_DOMAIN_CONCEPTS[1.0].PROF" .

sdmx:ConceptRoleProperty
        a                rdfs:Class , owl:Class ;
        rdfs:comment     "Abstract superclass for all properties representing ConceptRoleTypes"@en ;
        rdfs:label       "Concept role property (abstract)"@en ;
        rdfs:subClassOf  sdmx:ComponentProperty .

sdmx-metadata:grossNet
        a                 sdmx:MetadataProperty , rdf:Property ;
        rdfs:comment      "Form of consolidation used in presenting the data."@en ;
        rdfs:isDefinedBy  <http://sdmx.org/wp-content/uploads/2009/01/01_sdmx_cog_annex_1_cdc_2009.pdf> ;
        rdfs:label        "Grossing/Netting"@en ;
        qb:concept        sdmx-concept:grossNet .

sdmx:ConditionalAttributeProperty
        a                rdfs:Class , owl:Class ;
        rdfs:label       "Conditional attribute property"@en ;
        rdfs:subClassOf  sdmx:AttributeProperty .

sdmx-attribute:collMethod
        a                 qb:AttributeProperty , rdf:Property ;
        rdfs:comment      "Systematic process of gathering data for official statistics."@en ;
        rdfs:isDefinedBy  <http://sdmx.org/wp-content/uploads/2009/01/01_sdmx_cog_annex_1_cdc_2009.pdf> ;
        rdfs:label        "Data Collection Method"@en ;
        qb:concept        sdmx-concept:collMethod .

sdmx-code:sex  a            sdmx:CodeList , skos:ConceptScheme ;
        rdfs:label          "Code list for Sex (SEX) - codelist scheme"@en ;
        rdfs:seeAlso        sdmx-code:Sex ;
        skos:definition     <http://sdmx.org/wp-content/uploads/2009/01/02_sdmx_cog_annex_2_cl_2009.pdf> ;
        skos:hasTopConcept  sdmx-code:sex-U , sdmx-code:sex-M , sdmx-code:sex-F , sdmx-code:sex-N , sdmx-code:sex-T ;
        skos:notation       "CL_SEX" ;
        skos:note           "This  code list provides the gender."@en ;
        skos:prefLabel      "Code list for Sex (SEX) - codelist scheme"@en .

sdmx-attribute:contactMail
        a                 qb:AttributeProperty , rdf:Property ;
        rdfs:comment      "The postal address of the contact points for the data or metadata."@en ;
        rdfs:isDefinedBy  <http://sdmx.org/wp-content/uploads/2009/01/01_sdmx_cog_annex_1_cdc_2009.pdf> ;
        rdfs:label        "Contact mail address"@en ;
        qb:concept        sdmx-concept:contactMail .

sdmx-concept:costBurden
        a                 sdmx:Concept , skos:Concept ;
        rdfs:comment      "Costs associated with the collection and production of a statistical product and burden on respondents."@en ;
        rdfs:isDefinedBy  <http://sdmx.org/wp-content/uploads/2009/01/01_sdmx_cog_annex_1_cdc_2009.pdf> ;
        rdfs:label        "Cost and Burden"@en ;
        skos:inScheme     sdmx-concept:cog ;
        skos:notation     "urn:sdmx:org.sdmx.infomodel.conceptscheme.Concept=SDMX:CROSS_DOMAIN_CONCEPTS[1.0].COST_BURDEN" .

sdmx-subject:2.5  a      skos:Concept , sdmx:Concept , sdmx-subject:SubjectMatterDomain ;
        skos:broader     sdmx-subject:2 ;
        skos:definition  "Government finance, fiscal and public sector statistics - all statistics related to the government sector, including debt and deficit, revenue and expenditure, accounts of the government sector, central government, tax rates and revenues, tax and benefit systems, financing of state pension and other state social security schemes, public sector employment.\nExcludes \n- government expenditure in specific areas, like health (1.4), education (1.3), research and development (2.9), etc."@en ;
        skos:notation    "2.5" ;
        skos:prefLabel   "Government finance, fiscal and public sector statistics"@en .

sdmx-concept:classSystem
        a                 sdmx:Concept , skos:Concept ;
        rdfs:comment      "Arrangement or division of objects into groups based on characteristics which the objects have in common."@en ;
        rdfs:isDefinedBy  <http://sdmx.org/wp-content/uploads/2009/01/01_sdmx_cog_annex_1_cdc_2009.pdf> ;
        rdfs:label        "Classification systems"@en ;
        skos:inScheme     sdmx-concept:cog ;
        skos:notation     "urn:sdmx:org.sdmx.infomodel.conceptscheme.Concept=SDMX:CROSS_DOMAIN_CONCEPTS[1.0].CLASS_SYSTEM" .

eg:o51  a                  qb:Observation ;
        eg:lifeExpectancy  77.0 ;
        eg:refArea         ex-geo:newport_00pr ;
        qb:dataSet         eg:dataset-le3 .

sdmx-metadata:profCond
        a                 sdmx:MetadataProperty , rdf:Property ;
        rdfs:comment      "Provision for assuring the qualifications of staff and allowing staff to perform their functions without intervention motivated by non-statistical objectives."@en ;
        rdfs:isDefinedBy  <http://sdmx.org/wp-content/uploads/2009/01/01_sdmx_cog_annex_1_cdc_2009.pdf> ;
        rdfs:label        "Professionalism - code of conduct"@en ;
        qb:concept        sdmx-concept:profCond .

sdmx-concept:docMethod
        a                 sdmx:Concept , skos:Concept ;
        rdfs:comment      "Descriptive text and references to methodological documents available."@en ;
        rdfs:isDefinedBy  <http://sdmx.org/wp-content/uploads/2009/01/01_sdmx_cog_annex_1_cdc_2009.pdf> ;
        rdfs:label        "Documentation on methodology"@en ;
        skos:inScheme     sdmx-concept:cog ;
        skos:notation     "urn:sdmx:org.sdmx.infomodel.conceptscheme.Concept=SDMX:CROSS_DOMAIN_CONCEPTS[1.0].DOC_METHOD" .

sdmx:primaryMeasureProperty
        a                   rdf:Property , owl:ObjectProperty , owl:FunctionalProperty ;
        rdfs:comment        "identifies the Concept that plays the role of the observation in a time series"@en ;
        rdfs:label          "primary measure property"@en ;
        rdfs:range          sdmx:MeasureProperty ;
        rdfs:subPropertyOf  sdmx:component .

sdmx:Slice  a         rdfs:Class , owl:Class ;
        rdfs:comment  "Denotes an subset of a DataSet such as a Group, Section or TimeSeries"@en ;
        rdfs:label    "Slice"@en .

sdmx-attribute:userSat
        a                 qb:AttributeProperty , rdf:Property ;
        rdfs:comment      "Measure to determine user satisfaction."@en ;
        rdfs:isDefinedBy  <http://sdmx.org/wp-content/uploads/2009/01/01_sdmx_cog_annex_1_cdc_2009.pdf> ;
        rdfs:label        "Relevance - user satisifaction"@en ;
        qb:concept        sdmx-concept:userSat .

sdmx-metadata:comment
        a                   sdmx:MetadataProperty , rdf:Property ;
        rdfs:comment        "Supplementary descriptive text which can be attached to data or metadata."@en ;
        rdfs:isDefinedBy    <http://sdmx.org/wp-content/uploads/2009/01/01_sdmx_cog_annex_1_cdc_2009.pdf> ;
        rdfs:label          "Comment"@en ;
        rdfs:subPropertyOf  rdfs:comment ;
        qb:concept          sdmx-concept:comment .

sdmx-metadata:contactFunct
        a                   sdmx:MetadataProperty , rdf:Property ;
        rdfs:comment        "The area of technical responsibility of the contact, such as \"methodology\", \"database management\" or \"dissemination\"."@en ;
        rdfs:isDefinedBy    <http://sdmx.org/wp-content/uploads/2009/01/01_sdmx_cog_annex_1_cdc_2009.pdf> ;
        rdfs:label          "Contact person job title"@en ;
        rdfs:subPropertyOf  vcard:role ;
        qb:concept          sdmx-concept:contactFunct .

sdmx-code:timeFormat-P1M
        a                  skos:Concept , sdmx:Concept , sdmx-code:TimeFormat ;
        skos:inScheme      sdmx-code:timeFormat ;
        skos:notation      "P1M" ;
        skos:prefLabel     "Monthly"@en ;
        skos:topConceptOf  sdmx-code:timeFormat .

sdmx-attribute:valuation
        a                 qb:AttributeProperty , rdf:Property ;
        rdfs:comment      "The definition of the price per unit, for goods and services flows and asset stocks."@en ;
        rdfs:isDefinedBy  <http://sdmx.org/wp-content/uploads/2009/01/01_sdmx_cog_annex_1_cdc_2009.pdf> ;
        rdfs:label        "Valuation"@en ;
        qb:concept        sdmx-concept:valuation .

sdmx-code:freq-Q  a        skos:Concept , sdmx:Concept , sdmx-code:Freq ;
        skos:inScheme      sdmx-code:freq ;
        skos:notation      "Q" ;
        skos:prefLabel     "Quarterly"@en ;
        skos:topConceptOf  sdmx-code:freq .

sdmx-code:confStatus  a     sdmx:CodeList , skos:ConceptScheme ;
        rdfs:label          "code list for Confidentiality Status (CONF_STATUS) - codelist scheme"@en ;
        rdfs:seeAlso        sdmx-code:ConfStatus ;
        skos:definition     <http://sdmx.org/wp-content/uploads/2009/01/02_sdmx_cog_annex_2_cl_2009.pdf> ;
        skos:hasTopConcept  sdmx-code:confStatus-F , sdmx-code:confStatus-S , sdmx-code:confStatus-D , sdmx-code:confStatus-C , sdmx-code:confStatus-N ;
        skos:notation       "CL_CONF_STATUS" ;
        skos:note           "this code list provides coded information about the sensitivity and confidentiality status of the data."@en ;
        skos:prefLabel      "code list for Confidentiality Status (CONF_STATUS) - codelist scheme"@en .

sdmx-code:obsStatus-F
        a                  skos:Concept , sdmx:Concept , sdmx-code:ObsStatus ;
        skos:inScheme      sdmx-code:obsStatus ;
        skos:notation      "F" ;
        skos:prefLabel     "Forecast value"@en ;
        skos:topConceptOf  sdmx-code:obsStatus .

sdmx-subject:3.3.2  a    skos:Concept , sdmx:Concept , sdmx-subject:SubjectMatterDomain ;
        skos:broader     sdmx-subject:3.3 ;
        skos:definition  "Gender and special population groups - their living conditions and role in the society: comparisons men/women and situation of special population groups like children, youth, women, elderly, disabled, minority groups, etc."@en ;
        skos:notation    "3.3.2" ;
        skos:prefLabel   "Gender and special population groups"@en .

sdmx-code:sex-F  a         skos:Concept , sdmx:Concept , sdmx-code:Sex ;
        skos:inScheme      sdmx-code:sex ;
        skos:notation      "F" ;
        skos:prefLabel     "Female"@en ;
        skos:topConceptOf  sdmx-code:sex .

sdmx-concept:contactOrganisation
        a                 sdmx:Concept , skos:Concept ;
        rdfs:comment      "The name of the organisation of the contact points for the data or metadata."@en ;
        rdfs:isDefinedBy  <http://sdmx.org/wp-content/uploads/2009/01/01_sdmx_cog_annex_1_cdc_2009.pdf> ;
        rdfs:label        "Contact organisation"@en ;
        skos:broader      sdmx-concept:contact ;
        skos:inScheme     sdmx-concept:cog ;
        skos:notation     "urn:sdmx:org.sdmx.infomodel.conceptscheme.Concept=SDMX:CROSS_DOMAIN_CONCEPTS[1.0].CONTACT_ORGANISATION" .

sdmx:MeasureTypeRole  a  rdfs:Class , owl:Class ;
        rdfs:comment     "concept for a dimension that plays the role of identifying a type of measure"@en ;
        rdfs:label       "Measure type property"@en ;
        rdfs:subClassOf  sdmx:ConceptRole .

sdmx-code:decimals-9  a    skos:Concept , sdmx:Concept , sdmx-code:Decimals ;
        skos:inScheme      sdmx-code:decimals ;
        skos:notation      "9" ;
        skos:prefLabel     "Nine"@en ;
        skos:topConceptOf  sdmx-code:decimals .

sdmx-concept:conf  a      sdmx:Concept , skos:Concept ;
        rdfs:comment      "A property of data indicating the extent to which their unauthorised disclosure could be prejudicial or harmful to the interest of the source or other relevant parties."@en ;
        rdfs:isDefinedBy  <http://sdmx.org/wp-content/uploads/2009/01/01_sdmx_cog_annex_1_cdc_2009.pdf> ;
        rdfs:label        "Confidentiality"@en ;
        skos:inScheme     sdmx-concept:cog ;
        skos:notation     "urn:sdmx:org.sdmx.infomodel.conceptscheme.Concept=SDMX:CROSS_DOMAIN_CONCEPTS[1.0].CONF" .

sdmx-concept:instMandate
        a                 sdmx:Concept , skos:Concept ;
        rdfs:comment      "Set of rules or other formal set of instructions assigning responsibility as well as the authority to an organisation for the collection, processing, and dissemination of statistics."@en ;
        rdfs:isDefinedBy  <http://sdmx.org/wp-content/uploads/2009/01/01_sdmx_cog_annex_1_cdc_2009.pdf> ;
        rdfs:label        "Institutional Mandate"@en ;
        skos:inScheme     sdmx-concept:cog ;
        skos:notation     "urn:sdmx:org.sdmx.infomodel.conceptscheme.Concept=SDMX:CROSS_DOMAIN_CONCEPTS[1.0].INST_MANDATE" .

eg:sliceByRegion  a           qb:SliceKey ;
        rdfs:comment          "Slice by grouping regions together, fixing sex and time values"@en ;
        rdfs:label            "slice by region"@en ;
        qb:componentProperty  eg:refPeriod , sdmx-dimension:sex .

sdmx-concept:statConcDef
        a                 sdmx:Concept , skos:Concept ;
        rdfs:comment      "Statistical characteristics of statistical observations."@en ;
        rdfs:isDefinedBy  <http://sdmx.org/wp-content/uploads/2009/01/01_sdmx_cog_annex_1_cdc_2009.pdf> ;
        rdfs:label        "Statistical Concepts and Definitions"@en ;
        skos:inScheme     sdmx-concept:cog ;
        skos:notation     "urn:sdmx:org.sdmx.infomodel.conceptscheme.Concept=SDMX:CROSS_DOMAIN_CONCEPTS[1.0].STAT_CONC_DEF" .

sdmx-metadata:sourceType
        a                 sdmx:MetadataProperty , rdf:Property ;
        rdfs:comment      "Characteristics and components of the raw statistical data used for compiling statistical aggregates."@en ;
        rdfs:isDefinedBy  <http://sdmx.org/wp-content/uploads/2009/01/01_sdmx_cog_annex_1_cdc_2009.pdf> ;
        rdfs:label        "Source Data"@en ;
        qb:concept        sdmx-concept:sourceType .

sdmx-concept:coherence
        a                 sdmx:Concept , skos:Concept ;
        rdfs:comment      "Adequacy of statistics to be combined in different ways and for various uses."@en ;
        rdfs:isDefinedBy  <http://sdmx.org/wp-content/uploads/2009/01/01_sdmx_cog_annex_1_cdc_2009.pdf> ;
        rdfs:label        "Coherence"@en ;
        skos:inScheme     sdmx-concept:cog ;
        skos:notation     "urn:sdmx:org.sdmx.infomodel.conceptscheme.Concept=SDMX:CROSS_DOMAIN_CONCEPTS[1.0].COHERENCE" .

sdmx-code:area  a        skos:ConceptScheme , sdmx:CodeList ;
        rdfs:label       "Code list for providing values to concepts such as 'Reference area' and/or 'Counterpart area' - codelist scheme"@en ;
        rdfs:seeAlso     sdmx-code:Area ;
        skos:definition  <http://sdmx.org/wp-content/uploads/2009/01/02_sdmx_cog_annex_2_cl_2009.pdf> ;
        skos:notation    "CL_AREA" ;
        skos:note        ": This code list provides code values for geographical areas, defined as areas included within the borders of a country, region, group of countries, etc."@en ;
        skos:prefLabel   "Code list for providing values to concepts such as 'Reference area' and/or 'Counterpart area' - codelist scheme"@en .

sdmx-concept:dataDescr
        a                 sdmx:Concept , skos:Concept ;
        rdfs:comment      "Main characteristics of the data set described in an easily understandable manner, referring to the data and indicators disseminated."@en ;
        rdfs:isDefinedBy  <http://sdmx.org/wp-content/uploads/2009/01/01_sdmx_cog_annex_1_cdc_2009.pdf> ;
        rdfs:label        "Data Presentation - data description"@en ;
        skos:broader      sdmx-concept:dataPres ;
        skos:inScheme     sdmx-concept:cog ;
        skos:notation     "urn:sdmx:org.sdmx.infomodel.conceptscheme.Concept=SDMX:CROSS_DOMAIN_CONCEPTS[1.0].DATA_DESCR" .

sdmx-attribute:advNotice
        a                 qb:AttributeProperty , rdf:Property ;
        rdfs:comment      "Policy on notifying the public of changes in methodology, indicating whether the public is notified before a methodological change affects disseminated data and, if so, how long before."@en ;
        rdfs:isDefinedBy  <http://sdmx.org/wp-content/uploads/2009/01/01_sdmx_cog_annex_1_cdc_2009.pdf> ;
        rdfs:label        "Documentation on methodology - advance notice"@en ;
        qb:concept        sdmx-concept:advNotice .

sdmx-code:unitMult-12
        a                  skos:Concept , sdmx:Concept , sdmx-code:UnitMult ;
        skos:inScheme      sdmx-code:unitMult ;
        skos:notation      "12" ;
        skos:prefLabel     "Trillions"@en ;
        skos:topConceptOf  sdmx-code:unitMult .

sdmx-code:timeFormat-710
        a                  skos:Concept , sdmx:Concept , sdmx-code:TimeFormat ;
        skos:definition    "(for monthly series)\nfrom year/month to year/month"@en ;
        skos:inScheme      sdmx-code:timeFormat ;
        skos:notation      "710" ;
        skos:prefLabel     "CCYYMMCCYYMM"@en ;
        skos:topConceptOf  sdmx-code:timeFormat .

eg:o64  a                  qb:Observation ;
        eg:lifeExpectancy  79.6 ;
        eg:refArea         ex-geo:merthyr_tdfil_00ph ;
        qb:dataSet         eg:dataset-le3 .

eg:o32  a                  qb:Observation ;
        eg:lifeExpectancy  78.6 ;
        eg:refArea         ex-geo:cardiff_00pt ;
        qb:dataSet         eg:dataset-le3 .

sdmx-metadata:dissDet
        a                 sdmx:MetadataProperty , rdf:Property ;
        rdfs:comment      "Disseminated domain, measure, and time period breakdowns of statistics in the dataset."@en ;
        rdfs:isDefinedBy  <http://sdmx.org/wp-content/uploads/2009/01/01_sdmx_cog_annex_1_cdc_2009.pdf> ;
        rdfs:label        "Data Presentation - disseminated detail"@en ;
        qb:concept        sdmx-concept:dissDet .

sdmx-code:timeFormat-608
        a                  skos:Concept , sdmx:Concept , sdmx-code:TimeFormat ;
        skos:definition    "(for quarterly series)\nyear/quarter"@en ;
        skos:inScheme      sdmx-code:timeFormat ;
        skos:notation      "608" ;
        skos:prefLabel     "CCYYQ"@en ;
        skos:topConceptOf  sdmx-code:timeFormat .

sdmx-metadata:mAgency
        a                 sdmx:MetadataProperty , rdf:Property ;
        rdfs:comment      "The organisation or other expert body that maintains a domain-specific data or metadata structure definition."@en ;
        rdfs:isDefinedBy  <http://sdmx.org/wp-content/uploads/2009/01/01_sdmx_cog_annex_1_cdc_2009.pdf> ;
        rdfs:label        "Maintenance Agency"@en ;
        qb:concept        sdmx-concept:mAgency .

sdmx-metadata:occupation
        a                 sdmx:MetadataProperty , rdf:Property ;
        rdfs:comment      "Job or position held by an individual who performs a set of tasks and duties."@en ;
        rdfs:isDefinedBy  <http://sdmx.org/wp-content/uploads/2009/01/01_sdmx_cog_annex_1_cdc_2009.pdf> ;
        rdfs:label        "Occupation"@en ;
        qb:concept        sdmx-concept:occupation .

sdmx-attribute:unitMult
        a                 qb:AttributeProperty , rdf:Property , qb:CodedProperty ;
        rdfs:comment      "Exponent in base 10 specified so that multiplying the observation numeric values by 10^UNIT_MULT gives a value expressed in the UNIT."@en ;
        rdfs:isDefinedBy  <http://sdmx.org/wp-content/uploads/2009/01/01_sdmx_cog_annex_1_cdc_2009.pdf> ;
        rdfs:label        "Unit Multiplier"@en ;
        rdfs:range        sdmx-code:UnitMult ;
        qb:codeList       sdmx-code:unitMult ;
        qb:concept        sdmx-concept:unitMult .

sdmx-attribute:metaPosted
        a                 qb:AttributeProperty , rdf:Property ;
        rdfs:comment      "Date of the latest dissemination of the metadata."@en ;
        rdfs:isDefinedBy  <http://sdmx.org/wp-content/uploads/2009/01/01_sdmx_cog_annex_1_cdc_2009.pdf> ;
        rdfs:label        "Metadata Update - last posted"@en ;
        qb:concept        sdmx-concept:metaPosted .

sdmx:FrequencyProperty
        a                 rdfs:Class , owl:Class ;
        rdfs:label        "Frequency property"@en ;
        rdfs:subClassOf   sdmx:ConceptRoleProperty ;
        owl:disjointWith  sdmx:MeasureProperty .

sdmx-concept:sourceType
        a                 sdmx:Concept , skos:Concept ;
        rdfs:comment      "Characteristics and components of the raw statistical data used for compiling statistical aggregates."@en ;
        rdfs:isDefinedBy  <http://sdmx.org/wp-content/uploads/2009/01/01_sdmx_cog_annex_1_cdc_2009.pdf> ;
        rdfs:label        "Source Data"@en ;
        skos:inScheme     sdmx-concept:cog ;
        skos:notation     "urn:sdmx:org.sdmx.infomodel.conceptscheme.Concept=SDMX:CROSS_DOMAIN_CONCEPTS[1.0].SOURCE_TYPE" .

sdmx-attribute:accessibility
        a                 qb:AttributeProperty , rdf:Property ;
        rdfs:comment      "The ease and the conditions under which statistical information can be obtained."@en ;
        rdfs:isDefinedBy  <http://sdmx.org/wp-content/uploads/2009/01/01_sdmx_cog_annex_1_cdc_2009.pdf> ;
        rdfs:label        "Accessibility"@en ;
        qb:concept        sdmx-concept:accessibility .

sdmx-metadata:userNeeds
        a                 sdmx:MetadataProperty , rdf:Property ;
        rdfs:comment      "Description of users and their respective needs with respect to the statistical data."@en ;
        rdfs:isDefinedBy  <http://sdmx.org/wp-content/uploads/2009/01/01_sdmx_cog_annex_1_cdc_2009.pdf> ;
        rdfs:label        "Relevance - user needs"@en ;
        qb:concept        sdmx-concept:userNeeds .

sdmx-attribute:freqDetail
        a                 qb:AttributeProperty , rdf:Property ;
        rdfs:comment      "A further specification of the frequency to include more detailed information about the type of frequency and frequencies not commonly used."@en ;
        rdfs:isDefinedBy  <http://sdmx.org/wp-content/uploads/2009/01/01_sdmx_cog_annex_1_cdc_2009.pdf> ;
        rdfs:label        "Frequency Detail"@en ;
        qb:concept        sdmx-concept:freqDetail .

sdmx-concept:relPolLegActs
        a                 sdmx:Concept , skos:Concept ;
        rdfs:comment      "Legal acts and other agreements pertaining to data access."@en ;
        rdfs:isDefinedBy  <http://sdmx.org/wp-content/uploads/2009/01/01_sdmx_cog_annex_1_cdc_2009.pdf> ;
        rdfs:label        "Release Policy - legal acts and other agreements"@en ;
        skos:broader      sdmx-concept:relPolicy ;
        skos:inScheme     sdmx-concept:cog ;
        skos:notation     "urn:sdmx:org.sdmx.infomodel.conceptscheme.Concept=SDMX:CROSS_DOMAIN_CONCEPTS[1.0].REL_POL_LEG_ACTS" .

sdmx:DataFlow  a         rdfs:Class , owl:Class ;
        rdfs:label       "Data flow"@en ;
        rdfs:subClassOf  sdmx:DataSetOrFlow , sdmx:ReportEntry , sdmx:Structured , sdmx:Flow .

sdmx-code:Sex  a         rdfs:Class , owl:Class ;
        rdfs:comment     "This  code list provides the gender."@en ;
        rdfs:label       "Code list for Sex (SEX) - codelist class"@en ;
        rdfs:seeAlso     sdmx-code:sex ;
        rdfs:subClassOf  skos:Concept .

sdmx-dimension:currency
        a                 qb:CodedProperty , qb:DimensionProperty , rdf:Property ;
        rdfs:comment      "Monetary denomination of the object being measured."@en ;
        rdfs:isDefinedBy  <http://sdmx.org/wp-content/uploads/2009/01/01_sdmx_cog_annex_1_cdc_2009.pdf> ;
        rdfs:label        "Currency"@en ;
        rdfs:range        sdmx-code:Currency , rdfs:Resource ;
        qb:codeList       sdmx-code:currency ;
        qb:concept        sdmx-concept:currency .

sdmx-metadata:coherence
        a                 sdmx:MetadataProperty , rdf:Property ;
        rdfs:comment      "Adequacy of statistics to be combined in different ways and for various uses."@en ;
        rdfs:isDefinedBy  <http://sdmx.org/wp-content/uploads/2009/01/01_sdmx_cog_annex_1_cdc_2009.pdf> ;
        rdfs:label        "Coherence"@en ;
        qb:concept        sdmx-concept:coherence .

sdmx-metadata:dataDescr
        a                 sdmx:MetadataProperty , rdf:Property ;
        rdfs:comment      "Main characteristics of the data set described in an easily understandable manner, referring to the data and indicators disseminated."@en ;
        rdfs:isDefinedBy  <http://sdmx.org/wp-content/uploads/2009/01/01_sdmx_cog_annex_1_cdc_2009.pdf> ;
        rdfs:label        "Data Presentation - data description"@en ;
        qb:concept        sdmx-concept:dataDescr .

sdmx-code:obsStatus-A
        a                  skos:Concept , sdmx:Concept , sdmx-code:ObsStatus ;
        skos:definition    "Normal is the default value (if no value is provided) and is used when no special coded qualification is assumed. Usually, in this case, it can be assumed that the source agency assigns sufficient confidence to the provided observation and/or the value is not expected to be dramatically revised."@en ;
        skos:inScheme      sdmx-code:obsStatus ;
        skos:notation      "A" ;
        skos:prefLabel     "Normal"@en ;
        skos:topConceptOf  sdmx-code:obsStatus .

sdmx-code:currency  a    skos:ConceptScheme , sdmx:CodeList ;
        rdfs:label       "code list for Currency (CURRENCY) - codelist scheme"@en ;
        rdfs:seeAlso     sdmx-code:Currency ;
        skos:definition  <http://sdmx.org/wp-content/uploads/2009/01/02_sdmx_cog_annex_2_cl_2009.pdf> ;
        skos:notation    "CL_CURRENCY" ;
        skos:note        "This code list provides code values for currencies."@en ;
        skos:prefLabel   "code list for Currency (CURRENCY) - codelist scheme"@en .

sdmx-measure:obsValue
        a                 qb:MeasureProperty , rdf:Property ;
        rdfs:comment      "The value of a particular variable at a particular period."@en ;
        rdfs:isDefinedBy  <http://sdmx.org/wp-content/uploads/2009/01/01_sdmx_cog_annex_1_cdc_2009.pdf> ;
        rdfs:label        "Observation"@en ;
        qb:concept        sdmx-concept:obsValue .

sdmx-code:decimals  a       sdmx:CodeList , skos:ConceptScheme ;
        rdfs:label          "Code list for Decimals (DECIMALS) - codelist scheme"@en ;
        rdfs:seeAlso        sdmx-code:Decimals ;
        skos:definition     <http://sdmx.org/wp-content/uploads/2009/01/02_sdmx_cog_annex_2_cl_2009.pdf> ;
        skos:hasTopConcept  sdmx-code:decimals-5 , sdmx-code:decimals-3 , sdmx-code:decimals-8 , sdmx-code:decimals-6 , sdmx-code:decimals-1 , sdmx-code:decimals-4 , sdmx-code:decimals-2 , sdmx-code:decimals-9 , sdmx-code:decimals-0 , sdmx-code:decimals-7 ;
        skos:notation       "CL_DECIMALS" ;
        skos:note           "It provides a list of values showing the number of decimal digits used in the data."@en ;
        skos:prefLabel      "Code list for Decimals (DECIMALS) - codelist scheme"@en .

sdmx-concept:metaLastUpdate
        a                 sdmx:Concept , skos:Concept ;
        rdfs:comment      "Date of last update of the content of the metadata."@en ;
        rdfs:isDefinedBy  <http://sdmx.org/wp-content/uploads/2009/01/01_sdmx_cog_annex_1_cdc_2009.pdf> ;
        rdfs:label        "Metadata Update - last update"@en ;
        skos:broader      sdmx-concept:metaUpdate ;
        skos:inScheme     sdmx-concept:cog ;
        skos:notation     "urn:sdmx:org.sdmx.infomodel.conceptscheme.Concept=SDMX:CROSS_DOMAIN_CONCEPTS[1.0].META_LAST_UPD" .

sdmx-attribute:nonsamplingErr
        a                 qb:AttributeProperty , rdf:Property ;
        rdfs:comment      "Error in sample estimates which cannot be attributed to sampling fluctuations."@en ;
        rdfs:isDefinedBy  <http://sdmx.org/wp-content/uploads/2009/01/01_sdmx_cog_annex_1_cdc_2009.pdf> ;
        rdfs:label        "Accuracy - nonsampling error"@en ;
        qb:concept        sdmx-concept:nonsamplingErr .

sdmx-code:decimals-4  a    skos:Concept , sdmx:Concept , sdmx-code:Decimals ;
        skos:inScheme      sdmx-code:decimals ;
        skos:notation      "4" ;
        skos:prefLabel     "Four"@en ;
        skos:topConceptOf  sdmx-code:decimals .

sdmx-subject:3.1  a      skos:Concept , sdmx:Concept , sdmx-subject:SubjectMatterDomain ;
        skos:broader     sdmx-subject:3 ;
        skos:definition  "Environment - includes topics like climate, climate change, biodiversity, environment and health, natural resources, soil, water, air, landscape, waste, environmental expenditure, expenditure for the protection of the environment, environmental accounts, agri-environmental indicators, environmental pressure, environmental impact of industry, transport, energy etc., environmental monitoring, material flow analysis, environmental decoupling indicators, pollution, ecosystems, land use and cover, environmental protection, nationally protected areas.\nExcludes\n- environment as part of sustainable development (3.3.6)"@en ;
        skos:notation    "3.1" ;
        skos:prefLabel   "Environment"@en .

sdmx-concept:occupation
        a                 sdmx:Concept , skos:Concept ;
        rdfs:comment      "Job or position held by an individual who performs a set of tasks and duties."@en ;
        rdfs:isDefinedBy  <http://sdmx.org/wp-content/uploads/2009/01/01_sdmx_cog_annex_1_cdc_2009.pdf> ;
        rdfs:label        "Occupation"@en ;
        skos:inScheme     sdmx-concept:cog ;
        skos:notation     "urn:sdmx:org.sdmx.infomodel.conceptscheme.Concept=SDMX:CROSS_DOMAIN_CONCEPTS[1.0].OCCUPATION" .

sdmx-metadata:clarity
        a                 sdmx:MetadataProperty , rdf:Property ;
        rdfs:comment      "The extent to which easily comprehensible metadata are available, where these metadata are necessary to give a full understanding of statistical data."@en ;
        rdfs:isDefinedBy  <http://sdmx.org/wp-content/uploads/2009/01/01_sdmx_cog_annex_1_cdc_2009.pdf> ;
        rdfs:label        "Clarity"@en ;
        qb:concept        sdmx-concept:clarity .

sdmx-metadata:instManLaOa
        a                 sdmx:MetadataProperty , rdf:Property ;
        rdfs:comment      "Legal acts or other formal or informal agreements that assign responsibility as well as the authority to an agency for the collection, processing, and dissemination of statistics."@en ;
        rdfs:isDefinedBy  <http://sdmx.org/wp-content/uploads/2009/01/01_sdmx_cog_annex_1_cdc_2009.pdf> ;
        rdfs:label        "Institutional Mandate - legal acts and other agreements."@en ;
        qb:concept        sdmx-concept:instManLaOa .

sdmx-metadata:completeness
        a                 sdmx:MetadataProperty , rdf:Property ;
        rdfs:comment      "The extent to which all statistics that are needed are available."@en ;
        rdfs:isDefinedBy  <http://sdmx.org/wp-content/uploads/2009/01/01_sdmx_cog_annex_1_cdc_2009.pdf> ;
        rdfs:label        "Relevance - Completeness"@en ;
        qb:concept        sdmx-concept:completeness .

sdmx-code:TimeFormat  a  rdfs:Class , owl:Class ;
        rdfs:comment     "These codes (based on the ISO 8601 standard) indicate the type of time references used in the data. The numeric codes below (203, 102,...,702) are used only in the SDMX-EDI messages; and the alphanumeric codes (P1D...PT1M) only in the SDMX-ML messages."@en ;
        rdfs:label       "Code list for the Time Format as written in the SDMX-EDI and SDMX-ML messages - codelist class"@en ;
        rdfs:seeAlso     sdmx-code:timeFormat ;
        rdfs:subClassOf  skos:Concept .

sdmx-code:timeFormat-P1Y
        a                  skos:Concept , sdmx:Concept , sdmx-code:TimeFormat ;
        skos:inScheme      sdmx-code:timeFormat ;
        skos:notation      "P1Y" ;
        skos:prefLabel     "Annual"@en ;
        skos:topConceptOf  sdmx-code:timeFormat .

sdmx-metadata:civilStatus
        a                 sdmx:MetadataProperty , rdf:Property ;
        rdfs:comment      "Legal, conjugal status of each individual in relation to the marriage laws or customs of the country."@en ;
        rdfs:isDefinedBy  <http://sdmx.org/wp-content/uploads/2009/01/01_sdmx_cog_annex_1_cdc_2009.pdf> ;
        rdfs:label        "Civil Status"@en ;
        qb:concept        sdmx-concept:civilStatus .

sdmx-attribute:completeness
        a                 qb:AttributeProperty , rdf:Property ;
        rdfs:comment      "The extent to which all statistics that are needed are available."@en ;
        rdfs:isDefinedBy  <http://sdmx.org/wp-content/uploads/2009/01/01_sdmx_cog_annex_1_cdc_2009.pdf> ;
        rdfs:label        "Relevance - Completeness"@en ;
        qb:concept        sdmx-concept:completeness .

eg:o13  a                  qb:Observation ;
        eg:lifeExpectancy  76.6 ;
        eg:refArea         ex-geo:monmouthshire_00pp ;
        qb:dataSet         eg:dataset-le3 .

sdmx:entityProperty  a      rdf:Property , owl:ObjectProperty , owl:FunctionalProperty ;
        rdfs:comment        "identifies the Concept that plays the role of the subject to whom the data refers (e.g. the reporting agent for primary reporting, the country for secondary reporting)"@en ;
        rdfs:label          "entity property"@en ;
        rdfs:range          sdmx:DimensionOrAttributeProperty ;
        rdfs:subPropertyOf  sdmx:component .

sdmx-measure:civilStatus
        a                 qb:MeasureProperty , rdf:Property ;
        rdfs:comment      "Legal, conjugal status of each individual in relation to the marriage laws or customs of the country."@en ;
        rdfs:isDefinedBy  <http://sdmx.org/wp-content/uploads/2009/01/01_sdmx_cog_annex_1_cdc_2009.pdf> ;
        rdfs:label        "Civil Status"@en ;
        qb:concept        sdmx-concept:civilStatus .

sdmx-metadata:revPolicy
        a                 sdmx:MetadataProperty , rdf:Property ;
        rdfs:comment      "Policy aimed at ensuring the transparency of disseminated data, whereby preliminary data are compiled that are later revised."@en ;
        rdfs:isDefinedBy  <http://sdmx.org/wp-content/uploads/2009/01/01_sdmx_cog_annex_1_cdc_2009.pdf> ;
        rdfs:label        "Data Revision - policy"@en ;
        qb:concept        sdmx-concept:revPolicy .

sdmx-dimension:timePeriod
        a                 qb:DimensionProperty , rdf:Property ;
        rdfs:comment      "The period of time or point in time to which the measured observation refers."@en ;
        rdfs:isDefinedBy  <http://sdmx.org/wp-content/uploads/2009/01/01_sdmx_cog_annex_1_cdc_2009.pdf> ;
        rdfs:label        "Time Period"@en ;
        rdfs:range        rdfs:Resource ;
        qb:concept        sdmx-concept:timePeriod .

sdmx:measureTypeProperty
        a                   rdf:Property , owl:ObjectProperty ;
        rdfs:comment        "identifies the Concept that plays the role of identifying a type of measure"@en ;
        rdfs:label          "measure type property"@en ;
        rdfs:range          sdmx:DimensionProperty ;
        rdfs:subPropertyOf  sdmx:component .

sdmx-attribute:embargoTime
        a                 qb:AttributeProperty , rdf:Property ;
        rdfs:comment      "The exact time at which the data could be made available to the public."@en ;
        rdfs:isDefinedBy  <http://sdmx.org/wp-content/uploads/2009/01/01_sdmx_cog_annex_1_cdc_2009.pdf> ;
        rdfs:label        "Embargo Time"@en ;
        qb:concept        sdmx-concept:embargoTime .

sdmx:IdentityProperty
        a                 rdfs:Class , owl:Class ;
        rdfs:label        "Identity property"@en ;
        rdfs:subClassOf   sdmx:ConceptRoleProperty ;
        owl:disjointWith  sdmx:MeasureProperty .

sdmx-metadata:refArea
        a                 sdmx:MetadataProperty , rdf:Property ;
        rdfs:comment      "The country or geographic area to which the measured statistical phenomenon relates."@en ;
        rdfs:isDefinedBy  <http://sdmx.org/wp-content/uploads/2009/01/01_sdmx_cog_annex_1_cdc_2009.pdf> ;
        rdfs:label        "Reference Area"@en ;
        qb:concept        sdmx-concept:refArea .

sdmx-metadata:educationLev
        a                 sdmx:MetadataProperty , rdf:Property ;
        rdfs:comment      "The highest level of an educational programme the person has successfully completed."@en ;
        rdfs:isDefinedBy  <http://sdmx.org/wp-content/uploads/2009/01/01_sdmx_cog_annex_1_cdc_2009.pdf> ;
        rdfs:label        "Education Level"@en ;
        qb:concept        sdmx-concept:educationLev .

eg:dsd-le3  a         qb:DataStructureDefinition ;
        qb:component  [ qb:dimension  eg:refArea ;
                        qb:order      1
                      ] ;
        qb:component  [ qb:componentAttachment  qb:Slice ;
                        qb:dimension            eg:refPeriod ;
                        qb:order                2
                      ] ;
        qb:component  [ qb:componentAttachment  qb:Slice ;
                        qb:dimension            sdmx-dimension:sex ;
                        qb:order                3
                      ] ;
        qb:component  [ qb:measure  eg:lifeExpectancy ] ;
        qb:component  [ qb:attribute            sdmx-attribute:unitMeasure ;
                        qb:componentAttachment  qb:DataSet ;
                        qb:componentRequired    true
                      ] ;
        qb:sliceKey   eg:sliceByRegion .

sdmx-concept:contactName
        a                 sdmx:Concept , skos:Concept ;
        rdfs:comment      "The name of the contact points for the data or metadata."@en ;
        rdfs:isDefinedBy  <http://sdmx.org/wp-content/uploads/2009/01/01_sdmx_cog_annex_1_cdc_2009.pdf> ;
        rdfs:label        "Contact name"@en ;
        skos:broader      sdmx-concept:contact ;
        skos:inScheme     sdmx-concept:cog ;
        skos:notation     "urn:sdmx:org.sdmx.infomodel.conceptscheme.Concept=SDMX:CROSS_DOMAIN_CONCEPTS[1.0].CONTACT_NAME" .

eg:refArea  a               rdf:Property , qb:DimensionProperty ;
        rdfs:label          "reference area"@en ;
        rdfs:range          admingeo:UnitaryAuthority ;
        rdfs:subPropertyOf  sdmx-dimension:refArea ;
        qb:concept          sdmx-concept:refArea .

sdmx-concept:relevance
        a                 sdmx:Concept , skos:Concept ;
        rdfs:comment      "The degree to which statistical information meets the real or perceived needs of clients."@en ;
        rdfs:isDefinedBy  <http://sdmx.org/wp-content/uploads/2009/01/01_sdmx_cog_annex_1_cdc_2009.pdf> ;
        rdfs:label        "Relevance"@en ;
        skos:inScheme     sdmx-concept:cog ;
        skos:notation     "urn:sdmx:org.sdmx.infomodel.conceptscheme.Concept=SDMX:CROSS_DOMAIN_CONCEPTS[1.0].RELEVANCE" .

sdmx-attribute:relPolUsAc
        a                 qb:AttributeProperty , rdf:Property ;
        rdfs:comment      "The policy for release of the data to users, the scope of dissemination (eg, to the public, to selected users), how users are informed that the data are being released, and whether the policy provides determines the dissemination of statistical data to all users."@en ;
        rdfs:isDefinedBy  <http://sdmx.org/wp-content/uploads/2009/01/01_sdmx_cog_annex_1_cdc_2009.pdf> ;
        rdfs:label        "Release Policy - user access"@en ;
        qb:concept        sdmx-concept:relPolUsAc .

sdmx-code:timeFormat-704
        a                  skos:Concept , sdmx:Concept , sdmx-code:TimeFormat ;
        skos:definition    "(for half yearly series)\nfrom half-year to half-year"@en ;
        skos:inScheme      sdmx-code:timeFormat ;
        skos:notation      "704" ;
        skos:prefLabel     "CCYYSCCYYS"@en ;
        skos:topConceptOf  sdmx-code:timeFormat .

sdmx-attribute:instManShar
        a                 qb:AttributeProperty , rdf:Property ;
        rdfs:comment      "Arrangements or procedures for data sharing and coordination between data producing agencies."@en ;
        rdfs:isDefinedBy  <http://sdmx.org/wp-content/uploads/2009/01/01_sdmx_cog_annex_1_cdc_2009.pdf> ;
        rdfs:label        "Institutional Mandate - data sharing"@en ;
        qb:concept        sdmx-concept:instManShar .

sdmx-attribute:costBurdenEff
        a                 qb:AttributeProperty , rdf:Property ;
        rdfs:comment      "Cost benefit analysis, effectiveness of execution of medium term statistical programs, and ensuring efficient use of resources."@en ;
        rdfs:isDefinedBy  <http://sdmx.org/wp-content/uploads/2009/01/01_sdmx_cog_annex_1_cdc_2009.pdf> ;
        rdfs:label        "Cost and Burden - efficiency management"@en ;
        qb:concept        sdmx-concept:costBurdenEff .

sdmx-attribute:dsi  a     qb:AttributeProperty , rdf:Property ;
        rdfs:comment      "Sequence of characters identifying the data set with which it is associated."@en ;
        rdfs:isDefinedBy  <http://sdmx.org/wp-content/uploads/2009/01/01_sdmx_cog_annex_1_cdc_2009.pdf> ;
        rdfs:label        "Data Set Identifier"@en ;
        qb:concept        sdmx-concept:dsi .

sdmx-attribute:dataEditing
        a                 qb:AttributeProperty , rdf:Property ;
        rdfs:comment      "Activity aimed at detecting and correcting errors, logical inconsistencies and suspicious data."@en ;
        rdfs:isDefinedBy  <http://sdmx.org/wp-content/uploads/2009/01/01_sdmx_cog_annex_1_cdc_2009.pdf> ;
        rdfs:label        "Data Editing"@en ;
        qb:concept        sdmx-concept:dataEditing .

sdmx-subject:3  a          skos:Concept , sdmx:Concept , sdmx-subject:SubjectMatterDomain ;
        skos:definition    ""@en ;
        skos:notation      "3" ;
        skos:prefLabel     "Environment and multi-domain statistics"@en ;
        skos:topConceptOf  sdmx-subject:subjectMatterDomain .

sdmx-metadata:revPractice
        a                 sdmx:MetadataProperty , rdf:Property ;
        rdfs:comment      "Information on the data revision practice."@en ;
        rdfs:isDefinedBy  <http://sdmx.org/wp-content/uploads/2009/01/01_sdmx_cog_annex_1_cdc_2009.pdf> ;
        rdfs:label        "Data Revision - practice"@en ;
        qb:concept        sdmx-concept:revPractice .

sdmx-code:timeFormat-616
        a                  skos:Concept , sdmx:Concept , sdmx-code:TimeFormat ;
        skos:definition    "(for weekly series)\nyear/ week"@en ;
        skos:inScheme      sdmx-code:timeFormat ;
        skos:notation      "616" ;
        skos:prefLabel     "CCYYWW"@en ;
        skos:topConceptOf  sdmx-code:timeFormat .

sdmx-metadata:basePer
        a                 sdmx:MetadataProperty , rdf:Property ;
        rdfs:comment      "The period of time used as the base of an index number, or to which a constant price series refers."@en ;
        rdfs:isDefinedBy  <http://sdmx.org/wp-content/uploads/2009/01/01_sdmx_cog_annex_1_cdc_2009.pdf> ;
        rdfs:label        "Base Period"@en ;
        qb:concept        sdmx-concept:basePer .

sdmx-code:unitMult-0  a    skos:Concept , sdmx:Concept , sdmx-code:UnitMult ;
        skos:inScheme      sdmx-code:unitMult ;
        skos:notation      "0" ;
        skos:prefLabel     "Units"@en ;
        skos:topConceptOf  sdmx-code:unitMult .

sdmx-attribute:dataComp
        a                 qb:AttributeProperty , rdf:Property ;
        rdfs:comment      "Operations performed on data to derive new information according to a given set of rules."@en ;
        rdfs:isDefinedBy  <http://sdmx.org/wp-content/uploads/2009/01/01_sdmx_cog_annex_1_cdc_2009.pdf> ;
        rdfs:label        "Data Compilation"@en ;
        qb:concept        sdmx-concept:dataComp .

sdmx-code:obsStatus-M
        a                  skos:Concept , sdmx:Concept , sdmx-code:ObsStatus ;
        skos:definition    "Data can be missing due to various reasons:  data do not exist, are insignificant (or not collected because they are below a certain threshold), are unreliable, are not relevant for the period, or other reason not elsewhere specified."@en ;
        skos:inScheme      sdmx-code:obsStatus ;
        skos:notation      "M" ;
        skos:prefLabel     "Missing value"@en ;
        skos:topConceptOf  sdmx-code:obsStatus .

sdmx-attribute:conf  a    qb:AttributeProperty , rdf:Property ;
        rdfs:comment      "A property of data indicating the extent to which their unauthorised disclosure could be prejudicial or harmful to the interest of the source or other relevant parties."@en ;
        rdfs:isDefinedBy  <http://sdmx.org/wp-content/uploads/2009/01/01_sdmx_cog_annex_1_cdc_2009.pdf> ;
        rdfs:label        "Confidentiality"@en ;
        qb:concept        sdmx-concept:conf .

sdmx-code:sex-M  a         skos:Concept , sdmx:Concept , sdmx-code:Sex ;
        skos:inScheme      sdmx-code:sex ;
        skos:notation      "M" ;
        skos:prefLabel     "Male"@en ;
        skos:topConceptOf  sdmx-code:sex .

eg:slice3  a                qb:Slice ;
        eg:refPeriod        <http://reference.data.gov.uk/id/gregorian-interval/2005-01-01T00:00:00/P3Y> ;
        qb:observation      eg:o31 , eg:o32 , eg:o33 , eg:o34 ;
        qb:sliceStructure   eg:sliceByRegion ;
        sdmx-dimension:sex  sdmx-code:sex-M .

sdmx-metadata:collMethod
        a                 sdmx:MetadataProperty , rdf:Property ;
        rdfs:comment      "Systematic process of gathering data for official statistics."@en ;
        rdfs:isDefinedBy  <http://sdmx.org/wp-content/uploads/2009/01/01_sdmx_cog_annex_1_cdc_2009.pdf> ;
        rdfs:label        "Data Collection Method"@en ;
        qb:concept        sdmx-concept:collMethod .

sdmx-concept:unitMult
        a                 sdmx:Concept , skos:Concept ;
        rdfs:comment      "Exponent in base 10 specified so that multiplying the observation numeric values by 10^UNIT_MULT gives a value expressed in the UNIT."@en ;
        rdfs:isDefinedBy  <http://sdmx.org/wp-content/uploads/2009/01/01_sdmx_cog_annex_1_cdc_2009.pdf> ;
        rdfs:label        "Unit Multiplier"@en ;
        skos:inScheme     sdmx-concept:cog ;
        skos:notation     "urn:sdmx:org.sdmx.infomodel.conceptscheme.Concept=SDMX:CROSS_DOMAIN_CONCEPTS[1.0].UNIT_MULT" .

sdmx:Observation  a          rdfs:Class , owl:Class ;
        rdfs:label           "Observation"@en ;
        rdfs:subClassOf      sdmx:Attachable ;
        owl:equivalentClass  scovo:Item .

sdmx:MetadataReport  a  rdfs:Class , owl:Class ;
        rdfs:comment  "A metadata report (within an overall Metadata set) containing metadata via attached MetadataProperties"@en ;
        rdfs:label    "Metadata report"@en .

sdmx-subject:2.4.5  a    skos:Concept , sdmx:Concept , sdmx-subject:SubjectMatterDomain ;
        skos:broader     sdmx-subject:2.4 ;
        skos:definition  "Tourism - covers statistics regarding visitor activity (such as arrivals/departures, overnight stays, expenditures, purpose of the visit, etc.) associated to different forms of tourism (inbound, domestic and outbound), tourism industries activity and infrastructure, employment and tourism satellite accounts. \nExcludes\n- prices for tourist services (2.7)\n- environmental impacts (3.1)"@en ;
        skos:notation    "2.4.5" ;
        skos:prefLabel   "Tourism"@en .

sdmx-metadata:unitMult
        a                 sdmx:MetadataProperty , rdf:Property , qb:CodedProperty ;
        rdfs:comment      "Exponent in base 10 specified so that multiplying the observation numeric values by 10^UNIT_MULT gives a value expressed in the UNIT."@en ;
        rdfs:isDefinedBy  <http://sdmx.org/wp-content/uploads/2009/01/01_sdmx_cog_annex_1_cdc_2009.pdf> ;
        rdfs:label        "Unit Multiplier"@en ;
        rdfs:range        sdmx-code:UnitMult ;
        qb:codeList       sdmx-code:unitMult ;
        qb:concept        sdmx-concept:unitMult .

sdmx-metadata:costBurdenEff
        a                 sdmx:MetadataProperty , rdf:Property ;
        rdfs:comment      "Cost benefit analysis, effectiveness of execution of medium term statistical programs, and ensuring efficient use of resources."@en ;
        rdfs:isDefinedBy  <http://sdmx.org/wp-content/uploads/2009/01/01_sdmx_cog_annex_1_cdc_2009.pdf> ;
        rdfs:label        "Cost and Burden - efficiency management"@en ;
        qb:concept        sdmx-concept:costBurdenEff .

sdmx-dimension:freq  a    rdf:Property , qb:CodedProperty , qb:DimensionProperty ;
        rdfs:comment      "The time interval at which observations occur over a given time period."@en ;
        rdfs:isDefinedBy  <http://sdmx.org/wp-content/uploads/2009/01/01_sdmx_cog_annex_1_cdc_2009.pdf> ;
        rdfs:label        "Frequency"@en ;
        rdfs:range        rdfs:Resource , sdmx-code:Freq ;
        qb:codeList       sdmx-code:freq ;
        qb:concept        sdmx-concept:freq .

sdmx-concept:sex  a       sdmx:Concept , skos:Concept ;
        rdfs:comment      "The state of being male or female."@en ;
        rdfs:isDefinedBy  <http://sdmx.org/wp-content/uploads/2009/01/01_sdmx_cog_annex_1_cdc_2009.pdf> ;
        rdfs:label        "Sex"@en ;
        skos:inScheme     sdmx-concept:cog ;
        skos:notation     "urn:sdmx:org.sdmx.infomodel.conceptscheme.Concept=SDMX:CROSS_DOMAIN_CONCEPTS[1.0].SEX" .

sdmx-subject:1.6  a      skos:Concept , sdmx:Concept , sdmx-subject:SubjectMatterDomain ;
        skos:broader     sdmx-subject:1 ;
        skos:definition  "Social protection - deals with statistics on measures to protect people against the risks of inadequate incomes associated with unemployment, ill health, invalidity, old age, parental responsibilities, or inadequate income following the loss of a spouse or parent, etc., includes statistics on pension beneficiaries, social security schemes, social protection expenditure, etc.\nExcludes \n- insurance companies as economic actors (2.4.6)\n- pension funds as actors in financial markets(2.4.6)"@en ;
        skos:notation    "1.6" ;
        skos:prefLabel   "Social protection"@en .

sdmx:annotation  a          rdf:Property , owl:ObjectProperty ;
        rdfs:comment        "Attaches an annotation to an observation" ;
        rdfs:label          "has annotation"@en ;
        rdfs:range          sdmx:Annotation ;
        rdfs:subPropertyOf  skos:note .

sdmx-attribute:microDatAcc
        a                 qb:AttributeProperty , rdf:Property ;
        rdfs:comment      "Information on whether micro-data are also disseminated."@en ;
        rdfs:isDefinedBy  <http://sdmx.org/wp-content/uploads/2009/01/01_sdmx_cog_annex_1_cdc_2009.pdf> ;
        rdfs:label        "Dissemination Format - mirco-data access"@en ;
        qb:concept        sdmx-concept:microDatAcc .

sdmx-concept:relCalPolicy
        a                 sdmx:Concept , skos:Concept ;
        rdfs:comment      "The schedule of statistical release dates."@en ;
        rdfs:isDefinedBy  <http://sdmx.org/wp-content/uploads/2009/01/01_sdmx_cog_annex_1_cdc_2009.pdf> ;
        rdfs:label        "Release Policy - release calendar"@en ;
        skos:broader      sdmx-concept:relPolicy ;
        skos:inScheme     sdmx-concept:cog ;
        skos:notation     "urn:sdmx:org.sdmx.infomodel.conceptscheme.Concept=SDMX:CROSS_DOMAIN_CONCEPTS[1.0].REL_CAL_POLICY" .

eg:organization  a  org:Organization , foaf:Agent ;
        rdfs:label  "Example org"@en .

sdmx:DataSetOrFlow  a    rdfs:Class , owl:Class ;
        rdfs:comment     "Abstract superclass of DataSet and DataFlow"@en ;
        rdfs:label       "Data set or Data flow (abstract)"@en ;
        rdfs:subClassOf  void:Dataset .

sdmx:MetadataStructureDefinition
        a                rdfs:Class , owl:Class ;
        rdfs:comment     "Defines the structure of a MetadataSet"@en ;
        rdfs:label       "Metadata structure definition"@en ;
        rdfs:subClassOf  sdmx:Structure .

sdmx-metadata:dataProvider
        a                 sdmx:MetadataProperty , rdf:Property ;
        rdfs:comment      "Organisation which produces data or metadata"@en ;
        rdfs:isDefinedBy  <http://sdmx.org/wp-content/uploads/2009/01/01_sdmx_cog_annex_1_cdc_2009.pdf> ;
        rdfs:label        "Data Provider"@en ;
        qb:concept        sdmx-concept:dataProvider .

sdmx-attribute:costBurdenRes
        a                 qb:AttributeProperty , rdf:Property ;
        rdfs:comment      "Staff, facilities, computing resources, and financing to undertake statistical production."@en ;
        rdfs:isDefinedBy  <http://sdmx.org/wp-content/uploads/2009/01/01_sdmx_cog_annex_1_cdc_2009.pdf> ;
        rdfs:label        "Cost and Burden - resources"@en ;
        qb:concept        sdmx-concept:costBurdenRes .

sdmx-metadata:dataRev
        a                 sdmx:MetadataProperty , rdf:Property ;
        rdfs:comment      "Any change in a value of a statistic released to the public."@en ;
        rdfs:isDefinedBy  <http://sdmx.org/wp-content/uploads/2009/01/01_sdmx_cog_annex_1_cdc_2009.pdf> ;
        rdfs:label        "Data Revision"@en ;
        qb:concept        sdmx-concept:dataRev .

sdmx-attribute:dataProvider
        a                 qb:AttributeProperty , rdf:Property ;
        rdfs:comment      "Organisation which produces data or metadata"@en ;
        rdfs:isDefinedBy  <http://sdmx.org/wp-content/uploads/2009/01/01_sdmx_cog_annex_1_cdc_2009.pdf> ;
        rdfs:label        "Data Provider"@en ;
        qb:concept        sdmx-concept:dataProvider .

sdmx-code:freq-B  a        skos:Concept , sdmx:Concept , sdmx-code:Freq ;
        skos:definition    "Similar to \"daily\", however there are no observations for Saturday and Sunday (so, neither \"missing values\" nor \"numeric values\" should be provided for Saturday and Sunday). This treatment (\"business\") is one way to deal with such cases, but it is not the only option. Such a time series could alternatively be considered daily (\"D\"), thus, with missing values in the weekend."@en ;
        skos:inScheme      sdmx-code:freq ;
        skos:notation      "B" ;
        skos:prefLabel     "Daily - business week"@en ;
        skos:topConceptOf  sdmx-code:freq .

sdmx-concept:collMethod
        a                 sdmx:Concept , skos:Concept ;
        rdfs:comment      "Systematic process of gathering data for official statistics."@en ;
        rdfs:isDefinedBy  <http://sdmx.org/wp-content/uploads/2009/01/01_sdmx_cog_annex_1_cdc_2009.pdf> ;
        rdfs:label        "Data Collection Method"@en ;
        skos:inScheme     sdmx-concept:cog ;
        skos:notation     "urn:sdmx:org.sdmx.infomodel.conceptscheme.Concept=SDMX:CROSS_DOMAIN_CONCEPTS[1.0].COLL_METHOD" .

sdmx-concept:qualityAssure
        a                 sdmx:Concept , skos:Concept ;
        rdfs:comment      "Guidelines focusing on quality in general and dealing with quality of statistical programmes, including measures for ensuring the efficient use of resources."@en ;
        rdfs:isDefinedBy  <http://sdmx.org/wp-content/uploads/2009/01/01_sdmx_cog_annex_1_cdc_2009.pdf> ;
        rdfs:label        "Quality Management - assurance"@en ;
        skos:broader      sdmx-concept:qualityMgmnt ;
        skos:inScheme     sdmx-concept:cog ;
        skos:notation     "urn:sdmx:org.sdmx.infomodel.conceptscheme.Concept=SDMX:CROSS_DOMAIN_CONCEPTS[1.0].QUALITY_ASSURE" .

sdmx-concept:nonsamplingErr
        a                 sdmx:Concept , skos:Concept ;
        rdfs:comment      "Error in sample estimates which cannot be attributed to sampling fluctuations."@en ;
        rdfs:isDefinedBy  <http://sdmx.org/wp-content/uploads/2009/01/01_sdmx_cog_annex_1_cdc_2009.pdf> ;
        rdfs:label        "Accuracy - nonsampling error"@en ;
        skos:broader      sdmx-concept:accuracy ;
        skos:inScheme     sdmx-concept:cog ;
        skos:notation     "urn:sdmx:org.sdmx.infomodel.conceptscheme.Concept=SDMX:CROSS_DOMAIN_CONCEPTS[1.0].NONSAMPLING_ERR" .

sdmx-subject:2.7  a      skos:Concept , sdmx:Concept , sdmx-subject:SubjectMatterDomain ;
        skos:broader     sdmx-subject:2 ;
        skos:definition  "Prices - covers any statistical activity dealing with prices, including Purchasing Power Parities (PPPs) and international comparisons of GDP, covers topics like Consumer Price Indices (CPI), inflation, Producer Price Indices (PPI), price indexes for specific products and services (e.g. Information and Communication Technology products). \nExcludes \n- interest rates (2.4.6)\n- wages (2.8"@en ;
        skos:notation    "2.7" ;
        skos:prefLabel   "Prices"@en .

eg:o53  a                  qb:Observation ;
        eg:lifeExpectancy  76.6 ;
        eg:refArea         ex-geo:monmouthshire_00pp ;
        qb:dataSet         eg:dataset-le3 .

sdmx-metadata:relCalAccess
        a                 sdmx:MetadataProperty , rdf:Property ;
        rdfs:comment      "Access to the release calendar information."@en ;
        rdfs:isDefinedBy  <http://sdmx.org/wp-content/uploads/2009/01/01_sdmx_cog_annex_1_cdc_2009.pdf> ;
        rdfs:label        "Release Policy - release calendar access"@en ;
        qb:concept        sdmx-concept:relCalAccess .

sdmx-concept:valuation
        a                 sdmx:Concept , skos:Concept ;
        rdfs:comment      "The definition of the price per unit, for goods and services flows and asset stocks."@en ;
        rdfs:isDefinedBy  <http://sdmx.org/wp-content/uploads/2009/01/01_sdmx_cog_annex_1_cdc_2009.pdf> ;
        rdfs:label        "Valuation"@en ;
        skos:inScheme     sdmx-concept:cog ;
        skos:notation     "urn:sdmx:org.sdmx.infomodel.conceptscheme.Concept=SDMX:CROSS_DOMAIN_CONCEPTS[1.0].VALUATION" .

sdmx-attribute:dissDet
        a                 qb:AttributeProperty , rdf:Property ;
        rdfs:comment      "Disseminated domain, measure, and time period breakdowns of statistics in the dataset."@en ;
        rdfs:isDefinedBy  <http://sdmx.org/wp-content/uploads/2009/01/01_sdmx_cog_annex_1_cdc_2009.pdf> ;
        rdfs:label        "Data Presentation - disseminated detail"@en ;
        qb:concept        sdmx-concept:dissDet .

sdmx-concept:refPerWgts
        a                 sdmx:Concept , skos:Concept ;
        rdfs:comment      "Dates or periods to which the observations used to compile the weights refer."@en ;
        rdfs:isDefinedBy  <http://sdmx.org/wp-content/uploads/2009/01/01_sdmx_cog_annex_1_cdc_2009.pdf> ;
        rdfs:label        "Reference Period - weights"@en ;
        skos:broader      sdmx-concept:refPeriod ;
        skos:inScheme     sdmx-concept:cog ;
        skos:notation     "urn:sdmx:org.sdmx.infomodel.conceptscheme.Concept=SDMX:CROSS_DOMAIN_CONCEPTS[1.0].REF_PER_WGTS" .

sdmx-concept:revStudy
        a                 sdmx:Concept , skos:Concept ;
        rdfs:comment      "Information about data revision studies and analyses."@en ;
        rdfs:isDefinedBy  <http://sdmx.org/wp-content/uploads/2009/01/01_sdmx_cog_annex_1_cdc_2009.pdf> ;
        rdfs:label        "Data Revision - studies"@en ;
        skos:broader      sdmx-concept:dataRev ;
        skos:inScheme     sdmx-concept:cog ;
        skos:notation     "urn:sdmx:org.sdmx.infomodel.conceptscheme.Concept=SDMX:CROSS_DOMAIN_CONCEPTS[1.0].REV_STUDY" .

sdmx-concept:obsStatus
        a                 sdmx:Concept , skos:Concept ;
        rdfs:comment      "Information on the quality of a value or an unusual or missing value."@en ;
        rdfs:isDefinedBy  <http://sdmx.org/wp-content/uploads/2009/01/01_sdmx_cog_annex_1_cdc_2009.pdf> ;
        rdfs:label        "Observation Status"@en ;
        skos:inScheme     sdmx-concept:cog ;
        skos:notation     "urn:sdmx:org.sdmx.infomodel.conceptscheme.Concept=SDMX:CROSS_DOMAIN_CONCEPTS[1.0].OBS_STATUS" .

sdmx-attribute:relCalAccess
        a                 qb:AttributeProperty , rdf:Property ;
        rdfs:comment      "Access to the release calendar information."@en ;
        rdfs:isDefinedBy  <http://sdmx.org/wp-content/uploads/2009/01/01_sdmx_cog_annex_1_cdc_2009.pdf> ;
        rdfs:label        "Release Policy - release calendar access"@en ;
        qb:concept        sdmx-concept:relCalAccess .

sdmx-attribute:mAgency
        a                 qb:AttributeProperty , rdf:Property ;
        rdfs:comment      "The organisation or other expert body that maintains a domain-specific data or metadata structure definition."@en ;
        rdfs:isDefinedBy  <http://sdmx.org/wp-content/uploads/2009/01/01_sdmx_cog_annex_1_cdc_2009.pdf> ;
        rdfs:label        "Maintenance Agency"@en ;
        qb:concept        sdmx-concept:mAgency .

eg:o21  a                  qb:Observation ;
        eg:lifeExpectancy  80.7 ;
        eg:refArea         ex-geo:newport_00pr ;
        qb:dataSet         eg:dataset-le3 .

sdmx-code:ConfStatus  a  rdfs:Class , owl:Class ;
        rdfs:comment     "this code list provides coded information about the sensitivity and confidentiality status of the data."@en ;
        rdfs:label       "code list for Confidentiality Status (CONF_STATUS) - codelist class"@en ;
        rdfs:seeAlso     sdmx-code:confStatus ;
        rdfs:subClassOf  skos:Concept .

sdmx-metadata:title  a    sdmx:MetadataProperty , rdf:Property ;
        rdfs:comment      "Textual label used as identification of a statistical object."@en ;
        rdfs:isDefinedBy  <http://sdmx.org/wp-content/uploads/2009/01/01_sdmx_cog_annex_1_cdc_2009.pdf> ;
        rdfs:label        "Title"@en ;
        qb:concept        sdmx-concept:title .

sdmx-concept:embargoTime
        a                 sdmx:Concept , skos:Concept ;
        rdfs:comment      "The exact time at which the data could be made available to the public."@en ;
        rdfs:isDefinedBy  <http://sdmx.org/wp-content/uploads/2009/01/01_sdmx_cog_annex_1_cdc_2009.pdf> ;
        rdfs:label        "Embargo Time"@en ;
        skos:inScheme     sdmx-concept:cog ;
        skos:notation     "urn:sdmx:org.sdmx.infomodel.conceptscheme.Concept=SDMX:CROSS_DOMAIN_CONCEPTS[1.0].EMBARGO_TIME" .

sdmx-attribute:unitMeasDetail
        a                 qb:AttributeProperty , rdf:Property ;
        rdfs:comment      "Additional textual information on the unit of measure."@en ;
        rdfs:isDefinedBy  <http://sdmx.org/wp-content/uploads/2009/01/01_sdmx_cog_annex_1_cdc_2009.pdf> ;
        rdfs:label        "Unit of Measure Detail"@en ;
        qb:concept        sdmx-concept:unitMeasDetail .

sdmx-code:freq-S  a        skos:Concept , sdmx:Concept , sdmx-code:Freq ;
        skos:inScheme      sdmx-code:freq ;
        skos:notation      "S" ;
        skos:prefLabel     "Half Yearly, semester"@en ;
        skos:topConceptOf  sdmx-code:freq .

sdmx-code:confStatus-C
        a                  skos:Concept , sdmx:Concept , sdmx-code:ConfStatus ;
        skos:definition    "Confidential statistical information (primary confidentiality) due to identifiable respondents.  Measures also should be taken to prevent not only direct access, but also indirect deduction or calculation by other users and parties, probably by considering and treating additional observations as \"confidential\" (secondary confidentiality management)."@en ;
        skos:inScheme      sdmx-code:confStatus ;
        skos:notation      "C" ;
        skos:prefLabel     "Confidential statistical information"@en ;
        skos:topConceptOf  sdmx-code:confStatus .

sdmx:dataExtractionDate
        a            rdf:Property , owl:ObjectProperty ;
        rdfs:domain  sdmx:DataSet ;
        rdfs:label   "data extraction date"@en .

sdmx-attribute:relPolTra
        a                 qb:AttributeProperty , rdf:Property ;
        rdfs:comment      "Dissemination of the release policy to the public."@en ;
        rdfs:isDefinedBy  <http://sdmx.org/wp-content/uploads/2009/01/01_sdmx_cog_annex_1_cdc_2009.pdf> ;
        rdfs:label        "Release Policy - transparency"@en ;
        qb:concept        sdmx-concept:relPolTra .

sdmx-subject:3.3.4  a    skos:Concept , sdmx:Concept , sdmx-subject:SubjectMatterDomain ;
        skos:broader     sdmx-subject:3.3 ;
        skos:definition  "Globalisation - deals with measuring the economic activities of multinational companies, as well as with attempts to measure globalisation through a variety of components from other subject areas."@en ;
        skos:notation    "3.3.4" ;
        skos:prefLabel   "Globalisation"@en .

sdmx-metadata:costBurdenRes
        a                 sdmx:MetadataProperty , rdf:Property ;
        rdfs:comment      "Staff, facilities, computing resources, and financing to undertake statistical production."@en ;
        rdfs:isDefinedBy  <http://sdmx.org/wp-content/uploads/2009/01/01_sdmx_cog_annex_1_cdc_2009.pdf> ;
        rdfs:label        "Cost and Burden - resources"@en ;
        qb:concept        sdmx-concept:costBurdenRes .

sdmx-attribute:punctuality
        a                 qb:AttributeProperty , rdf:Property ;
        rdfs:comment      "Time lag between the actual delivery of the data and the target date when it should have been delivered."@en ;
        rdfs:isDefinedBy  <http://sdmx.org/wp-content/uploads/2009/01/01_sdmx_cog_annex_1_cdc_2009.pdf> ;
        rdfs:label        "Punctuality"@en ;
        qb:concept        sdmx-concept:punctuality .

sdmx-subject:1.1  a      skos:Concept , sdmx:Concept , sdmx-subject:SubjectMatterDomain ;
        skos:broader     sdmx-subject:1 ;
        skos:definition  "Population and migration - covers work in population and demographic statistics, topics like demography, vital statistics, population structures and growth, demographic projections, families and households (marriages, divorces, household size), migration, refugees and asylum seekers. \nExcludes\n- causes of death (1.4)"@en ;
        skos:notation    "1.1" ;
        skos:prefLabel   "Population and migration"@en .

sdmx-dimension:sex  a     qb:DimensionProperty , qb:CodedProperty , rdf:Property ;
        rdfs:comment      "The state of being male or female."@en ;
        rdfs:isDefinedBy  <http://sdmx.org/wp-content/uploads/2009/01/01_sdmx_cog_annex_1_cdc_2009.pdf> ;
        rdfs:label        "Sex"@en ;
        rdfs:range        sdmx-code:Sex , rdfs:Resource ;
        qb:codeList       sdmx-code:sex ;
        qb:concept        sdmx-concept:sex .

sdmx-metadata:metaPosted
        a                 sdmx:MetadataProperty , rdf:Property ;
        rdfs:comment      "Date of the latest dissemination of the metadata."@en ;
        rdfs:isDefinedBy  <http://sdmx.org/wp-content/uploads/2009/01/01_sdmx_cog_annex_1_cdc_2009.pdf> ;
        rdfs:label        "Metadata Update - last posted"@en ;
        qb:concept        sdmx-concept:metaPosted .

sdmx-concept:publications
        a                 sdmx:Concept , skos:Concept ;
        rdfs:comment      "Regular or ad-hoc publications in which the data are made available to the public."@en ;
        rdfs:isDefinedBy  <http://sdmx.org/wp-content/uploads/2009/01/01_sdmx_cog_annex_1_cdc_2009.pdf> ;
        rdfs:label        "Dissemination Format - publications"@en ;
        skos:broader      sdmx-concept:dissFormat ;
        skos:inScheme     sdmx-concept:cog ;
        skos:notation     "urn:sdmx:org.sdmx.infomodel.conceptscheme.Concept=SDMX:CROSS_DOMAIN_CONCEPTS[1.0].PUBLICATIONS" .

sdmx:countProperty  a       rdf:Property , owl:ObjectProperty ;
        rdfs:comment        "identifies the Concept that plays the role of an identifier where the identifier is taken from a known system of counts"@en ;
        rdfs:label          "count property"@en ;
        rdfs:range          sdmx:DimensionOrAttributeProperty ;
        rdfs:subPropertyOf  sdmx:component .

sdmx-attribute:clarity
        a                 qb:AttributeProperty , rdf:Property ;
        rdfs:comment      "The extent to which easily comprehensible metadata are available, where these metadata are necessary to give a full understanding of statistical data."@en ;
        rdfs:isDefinedBy  <http://sdmx.org/wp-content/uploads/2009/01/01_sdmx_cog_annex_1_cdc_2009.pdf> ;
        rdfs:label        "Clarity"@en ;
        qb:concept        sdmx-concept:clarity .

sdmx-attribute:confDataTr
        a                 qb:AttributeProperty , rdf:Property ;
        rdfs:comment      "Rules applied for treating the data set to ensure statistical confidentiality and prevent unauthorised disclosure."@en ;
        rdfs:isDefinedBy  <http://sdmx.org/wp-content/uploads/2009/01/01_sdmx_cog_annex_1_cdc_2009.pdf> ;
        rdfs:label        "Confidentiality - data treatment"@en ;
        qb:concept        sdmx-concept:confDataTr .

sdmx-metadata:freqDetail
        a                 sdmx:MetadataProperty , rdf:Property ;
        rdfs:comment      "A further specification of the frequency to include more detailed information about the type of frequency and frequencies not commonly used."@en ;
        rdfs:isDefinedBy  <http://sdmx.org/wp-content/uploads/2009/01/01_sdmx_cog_annex_1_cdc_2009.pdf> ;
        rdfs:label        "Frequency Detail"@en ;
        qb:concept        sdmx-concept:freqDetail .

sdmx-attribute:qualityDoc
        a                 qb:AttributeProperty , rdf:Property ;
        rdfs:comment      "Documentation on procedures applied for quality management and quality assessment."@en ;
        rdfs:isDefinedBy  <http://sdmx.org/wp-content/uploads/2009/01/01_sdmx_cog_annex_1_cdc_2009.pdf> ;
        rdfs:label        "Quality Management - documentation"@en ;
        qb:concept        sdmx-concept:qualityDoc .

sdmx-concept:dataEditing
        a                 sdmx:Concept , skos:Concept ;
        rdfs:comment      "Activity aimed at detecting and correcting errors, logical inconsistencies and suspicious data."@en ;
        rdfs:isDefinedBy  <http://sdmx.org/wp-content/uploads/2009/01/01_sdmx_cog_annex_1_cdc_2009.pdf> ;
        rdfs:label        "Data Editing"@en ;
        skos:inScheme     sdmx-concept:cog ;
        skos:notation     "urn:sdmx:org.sdmx.infomodel.conceptscheme.Concept=SDMX:CROSS_DOMAIN_CONCEPTS[1.0].DATA_EDITING" .

sdmx-attribute:currency
        a                 qb:AttributeProperty , rdf:Property , qb:CodedProperty ;
        rdfs:comment      "Monetary denomination of the object being measured."@en ;
        rdfs:isDefinedBy  <http://sdmx.org/wp-content/uploads/2009/01/01_sdmx_cog_annex_1_cdc_2009.pdf> ;
        rdfs:label        "Currency"@en ;
        rdfs:range        sdmx-code:Currency ;
        qb:codeList       sdmx-code:currency ;
        qb:concept        sdmx-concept:currency .

sdmx-attribute:timeOutput
        a                 qb:AttributeProperty , rdf:Property ;
        rdfs:comment      "The lapse of time between the end of a reference period and dissemination of the data."@en ;
        rdfs:isDefinedBy  <http://sdmx.org/wp-content/uploads/2009/01/01_sdmx_cog_annex_1_cdc_2009.pdf> ;
        rdfs:label        "Timeliness - output"@en ;
        qb:concept        sdmx-concept:timeOutput .

sdmx-attribute:decimals
        a                 qb:AttributeProperty , rdf:Property , qb:CodedProperty ;
        rdfs:comment      "The number of digits of an observation to the right of a decimal point."@en ;
        rdfs:isDefinedBy  <http://sdmx.org/wp-content/uploads/2009/01/01_sdmx_cog_annex_1_cdc_2009.pdf> ;
        rdfs:label        "Decimals"@en ;
        rdfs:range        sdmx-code:Decimals ;
        qb:codeList       sdmx-code:decimals ;
        qb:concept        sdmx-concept:decimals .

sdmx-code:ObsStatus  a   rdfs:Class , owl:Class ;
        rdfs:comment     "This code list provides coded information about the \"status\" of an observation (with respect events such as the ones reflected in the codes composing the code list)."@en ;
        rdfs:label       "Observation status - codelist class"@en ;
        rdfs:seeAlso     sdmx-code:obsStatus ;
        rdfs:subClassOf  skos:Concept .

sdmx-attribute:dissOther
        a                 qb:AttributeProperty , rdf:Property ;
        rdfs:comment      "References to the most important other data dissemination done."@en ;
        rdfs:isDefinedBy  <http://sdmx.org/wp-content/uploads/2009/01/01_sdmx_cog_annex_1_cdc_2009.pdf> ;
        rdfs:label        "Dissemination Format - other"@en ;
        qb:concept        sdmx-concept:dissOther .

eg:o34  a                  qb:Observation ;
        eg:lifeExpectancy  75.5 ;
        eg:refArea         ex-geo:merthyr_tdfil_00ph ;
        qb:dataSet         eg:dataset-le3 .

sdmx-attribute:dataValOutput
        a                 qb:AttributeProperty , rdf:Property ;
        rdfs:comment      "Assessment of discrepancies and other problems in statistical outputs."@en ;
        rdfs:isDefinedBy  <http://sdmx.org/wp-content/uploads/2009/01/01_sdmx_cog_annex_1_cdc_2009.pdf> ;
        rdfs:label        "Data Validation - output"@en ;
        qb:concept        sdmx-concept:dataValOutput .

sdmx-attribute:timeSource
        a                 qb:AttributeProperty , rdf:Property ;
        rdfs:comment      "The time between the end of a reference period and actual receipt of the data by the compiling agency."@en ;
        rdfs:isDefinedBy  <http://sdmx.org/wp-content/uploads/2009/01/01_sdmx_cog_annex_1_cdc_2009.pdf> ;
        rdfs:label        "Timeliness - source data"@en ;
        qb:concept        sdmx-concept:timeSource .

sdmx-attribute:accuracyOverall
        a                 qb:AttributeProperty , rdf:Property ;
        rdfs:comment      "Assessment of accuracy, linked to a certain data set or domain, which is summarising the various components into one single measure."@en ;
        rdfs:isDefinedBy  <http://sdmx.org/wp-content/uploads/2009/01/01_sdmx_cog_annex_1_cdc_2009.pdf> ;
        rdfs:label        "Accuracy - overall"@en ;
        qb:concept        sdmx-concept:accuracyOverall .

sdmx-attribute:dataValSource
        a                 qb:AttributeProperty , rdf:Property ;
        rdfs:comment      "Assessment of discrepancies and other problems related to source data."@en ;
        rdfs:isDefinedBy  <http://sdmx.org/wp-content/uploads/2009/01/01_sdmx_cog_annex_1_cdc_2009.pdf> ;
        rdfs:label        "Data Validation - source"@en ;
        qb:concept        sdmx-concept:dataValSource .

sdmx-attribute:comparGeo
        a                 qb:AttributeProperty , rdf:Property ;
        rdfs:comment      "Extent to which statistics are comparable between geographical areas."@en ;
        rdfs:isDefinedBy  <http://sdmx.org/wp-content/uploads/2009/01/01_sdmx_cog_annex_1_cdc_2009.pdf> ;
        rdfs:label        "Comparability - geographical"@en ;
        qb:concept        sdmx-concept:comparGeo .

sdmx-subject:2.2  a      skos:Concept , sdmx:Concept , sdmx-subject:SubjectMatterDomain ;
        skos:broader     sdmx-subject:2 ;
        skos:definition  "Economic accounts - covers work on National Accounts in both current and constant prices, dealing with topics like implementation of the 1993 System National Accounts (1993 SNA), update of the 1993 SNA, European System of Accounts (ESA95), Gross Domestic Product (GDP), Gross National Income (GNI), non-observed and informal economy, measurement of capital, input-output tables, balance sheets, etc.\nExcludes \n- agricultural economic accounts (in 2.4.1)\n- tourism satellite accounts (in 2.4.5)\n- detailed general government accounts (2.5)\n- financial accounts(2.5)\n- price statistics(2.7)\n- environmental accounts (3.1)"@en ;
        skos:notation    "2.2" ;
        skos:prefLabel   "Economic accounts"@en .

sdmx-metadata:advNotice
        a                 sdmx:MetadataProperty , rdf:Property ;
        rdfs:comment      "Policy on notifying the public of changes in methodology, indicating whether the public is notified before a methodological change affects disseminated data and, if so, how long before."@en ;
        rdfs:isDefinedBy  <http://sdmx.org/wp-content/uploads/2009/01/01_sdmx_cog_annex_1_cdc_2009.pdf> ;
        rdfs:label        "Documentation on methodology - advance notice"@en ;
        qb:concept        sdmx-concept:advNotice .

sdmx-concept:metaPosted
        a                 sdmx:Concept , skos:Concept ;
        rdfs:comment      "Date of the latest dissemination of the metadata."@en ;
        rdfs:isDefinedBy  <http://sdmx.org/wp-content/uploads/2009/01/01_sdmx_cog_annex_1_cdc_2009.pdf> ;
        rdfs:label        "Metadata Update - last posted"@en ;
        skos:broader      sdmx-concept:metaUpdate ;
        skos:inScheme     sdmx-concept:cog ;
        skos:notation     "urn:sdmx:org.sdmx.infomodel.conceptscheme.Concept=SDMX:CROSS_DOMAIN_CONCEPTS[1.0].META_POSTED" .

sdmx:reportStructure  a  rdf:Property , owl:ObjectProperty ;
        rdfs:comment  "Links an individual metadata report to the report structure it corresponds to"@en ;
        rdfs:domain   sdmx:MetadataReport ;
        rdfs:label    "report structure"@en ;
        rdfs:range    sdmx:MetadataReportStructure .

sdmx-concept:dataComp
        a                 sdmx:Concept , skos:Concept ;
        rdfs:comment      "Operations performed on data to derive new information according to a given set of rules."@en ;
        rdfs:isDefinedBy  <http://sdmx.org/wp-content/uploads/2009/01/01_sdmx_cog_annex_1_cdc_2009.pdf> ;
        rdfs:label        "Data Compilation"@en ;
        skos:inScheme     sdmx-concept:cog ;
        skos:notation     "urn:sdmx:org.sdmx.infomodel.conceptscheme.Concept=SDMX:CROSS_DOMAIN_CONCEPTS[1.0].DATA_COMP" .

sdmx-metadata:coverageSector
        a                 sdmx:MetadataProperty , rdf:Property ;
        rdfs:comment      "Main economic or other sectors covered by the statistics."@en ;
        rdfs:isDefinedBy  <http://sdmx.org/wp-content/uploads/2009/01/01_sdmx_cog_annex_1_cdc_2009.pdf> ;
        rdfs:label        "Coverage - sector"@en ;
        qb:concept        sdmx-concept:coverageSector .

sdmx-concept:microDatAcc
        a                 sdmx:Concept , skos:Concept ;
        rdfs:comment      "Information on whether micro-data are also disseminated."@en ;
        rdfs:isDefinedBy  <http://sdmx.org/wp-content/uploads/2009/01/01_sdmx_cog_annex_1_cdc_2009.pdf> ;
        rdfs:label        "Dissemination Format - mirco-data access"@en ;
        skos:broader      sdmx-concept:dissFormat ;
        skos:inScheme     sdmx-concept:cog ;
        skos:notation     "urn:sdmx:org.sdmx.infomodel.conceptscheme.Concept=SDMX:CROSS_DOMAIN_CONCEPTS[1.0].MICRO_DAT_ACC" .

sdmx-metadata:dataComp
        a                 sdmx:MetadataProperty , rdf:Property ;
        rdfs:comment      "Operations performed on data to derive new information according to a given set of rules."@en ;
        rdfs:isDefinedBy  <http://sdmx.org/wp-content/uploads/2009/01/01_sdmx_cog_annex_1_cdc_2009.pdf> ;
        rdfs:label        "Data Compilation"@en ;
        qb:concept        sdmx-concept:dataComp .

sdmx-attribute:comparDomains
        a                 qb:AttributeProperty , rdf:Property ;
        rdfs:comment      "Extent to which statistics are comparable between different statistical domains."@en ;
        rdfs:isDefinedBy  <http://sdmx.org/wp-content/uploads/2009/01/01_sdmx_cog_annex_1_cdc_2009.pdf> ;
        rdfs:label        "Comparability - between domains"@en ;
        qb:concept        sdmx-concept:comparDomains .

sdmx:ComponentProperty
        a                rdfs:Class , owl:Class ;
        rdfs:comment     "Abstract super-property of all properties representing dimensions, attributes or measures"@en ;
        rdfs:label       "Component property (abstract)"@en ;
        rdfs:subClassOf  rdf:Property .

sdmx-code:freq-N  a        skos:Concept , sdmx:Concept , sdmx-code:Freq ;
        skos:definition    "While N denotes \"minutely\", usually, there may be no observations every minute (for several series the frequency is usually \"irregular\" within a day/days). And though observations may be sparse (not collected every minute), missing values do not need to be given for the minutes when no observations exist: in any case the time stamp determines when an observation is observed."@en ;
        skos:inScheme      sdmx-code:freq ;
        skos:notation      "N" ;
        skos:prefLabel     "Minutely"@en ;
        skos:topConceptOf  sdmx-code:freq .

sdmx-measure:sex  a       qb:MeasureProperty , rdf:Property , qb:CodedProperty ;
        rdfs:comment      "The state of being male or female."@en ;
        rdfs:isDefinedBy  <http://sdmx.org/wp-content/uploads/2009/01/01_sdmx_cog_annex_1_cdc_2009.pdf> ;
        rdfs:label        "Sex"@en ;
        rdfs:range        sdmx-code:Sex ;
        qb:codeList       sdmx-code:sex ;
        qb:concept        sdmx-concept:sex .

sdmx-metadata:adjustCoded
        a                 sdmx:MetadataProperty , rdf:Property ;
        rdfs:comment      "Type of adjustment used, represented by a code."@en ;
        rdfs:isDefinedBy  <http://sdmx.org/wp-content/uploads/2009/01/01_sdmx_cog_annex_1_cdc_2009.pdf> ;
        rdfs:label        "Adjustment - coded"@en ;
        qb:concept        sdmx-concept:adjustCoded .

sdmx-metadata:contactPhone
        a                   sdmx:MetadataProperty , rdf:Property ;
        rdfs:comment        "The telephone number of the contact points for the data or metadata."@en ;
        rdfs:isDefinedBy    <http://sdmx.org/wp-content/uploads/2009/01/01_sdmx_cog_annex_1_cdc_2009.pdf> ;
        rdfs:label          "Contact phone number"@en ;
        rdfs:subPropertyOf  vcard:tel ;
        qb:concept          sdmx-concept:contactPhone .

sdmx-metadata:dataValOutput
        a                 sdmx:MetadataProperty , rdf:Property ;
        rdfs:comment      "Assessment of discrepancies and other problems in statistical outputs."@en ;
        rdfs:isDefinedBy  <http://sdmx.org/wp-content/uploads/2009/01/01_sdmx_cog_annex_1_cdc_2009.pdf> ;
        rdfs:label        "Data Validation - output"@en ;
        qb:concept        sdmx-concept:dataValOutput .

sdmx-attribute:contactPhone
        a                 qb:AttributeProperty , rdf:Property ;
        rdfs:comment      "The telephone number of the contact points for the data or metadata."@en ;
        rdfs:isDefinedBy  <http://sdmx.org/wp-content/uploads/2009/01/01_sdmx_cog_annex_1_cdc_2009.pdf> ;
        rdfs:label        "Contact phone number"@en ;
        qb:concept        sdmx-concept:contactPhone .

sdmx-code:decimals-6  a    skos:Concept , sdmx:Concept , sdmx-code:Decimals ;
        skos:inScheme      sdmx-code:decimals ;
        skos:notation      "6" ;
        skos:prefLabel     "Six"@en ;
        skos:topConceptOf  sdmx-code:decimals .

sdmx-attribute:origDataId
        a                 qb:AttributeProperty , rdf:Property ;
        rdfs:comment      "The data identifier as found in the originating database."@en ;
        rdfs:isDefinedBy  <http://sdmx.org/wp-content/uploads/2009/01/01_sdmx_cog_annex_1_cdc_2009.pdf> ;
        rdfs:label        "Original Data Identifier"@en ;
        qb:concept        sdmx-concept:origDataId .

sdmx-attribute:organisationUnit
        a                 qb:AttributeProperty , rdf:Property ;
        rdfs:comment      "An addressable subdivision of an organization."@en ;
        rdfs:isDefinedBy  <http://sdmx.org/wp-content/uploads/2009/01/01_sdmx_cog_annex_1_cdc_2009.pdf> ;
        rdfs:label        "Contact organization unit"@en ;
        qb:concept        sdmx-concept:organisationUnit .

sdmx-subject:3.3  a      skos:Concept , sdmx:Concept , sdmx-subject:SubjectMatterDomain ;
        skos:broader     sdmx-subject:3 ;
        skos:definition  "Multi-domain statistics and indicators - deals with conceptual or data work based on a specific thematic approach to outputs that cut across several economic, social or environmental subject areas; the two-digit-level of the classification covers activities dealing with such type of issues that are not explicitly mentioned at the three-digit level.\nExcludes: \n- multi-domain statistics based on a regional approach (3.2)\n- yearbook type of compendia or similar products by international organisations not following a specific thematic approach (3.4)"@en ;
        skos:notation    "3.3" ;
        skos:prefLabel   "Multi-domain statistics and indicators"@en .

sdmx-code:obsStatus  a      skos:ConceptScheme , sdmx:CodeList ;
        rdfs:label          "Observation status - codelist scheme"@en ;
        rdfs:seeAlso        sdmx-code:ObsStatus ;
        skos:definition     <http://sdmx.org/wp-content/uploads/2009/01/02_sdmx_cog_annex_2_cl_2009.pdf> ;
        skos:hasTopConcept  sdmx-code:obsStatus-A , sdmx-code:obsStatus-M , sdmx-code:obsStatus-F , sdmx-code:obsStatus-E , sdmx-code:obsStatus-B , sdmx-code:obsStatus-I , sdmx-code:obsStatus-P , sdmx-code:obsStatus-S ;
        skos:notation       "CL_OBS_STATUS" ;
        skos:note           "This code list provides coded information about the \"status\" of an observation (with respect events such as the ones reflected in the codes composing the code list)."@en ;
        skos:prefLabel      "Observation status - codelist scheme"@en .

sdmx-metadata:timePeriod
        a                 sdmx:MetadataProperty , rdf:Property ;
        rdfs:comment      "The period of time or point in time to which the measured observation refers."@en ;
        rdfs:isDefinedBy  <http://sdmx.org/wp-content/uploads/2009/01/01_sdmx_cog_annex_1_cdc_2009.pdf> ;
        rdfs:label        "Time Period"@en ;
        qb:concept        sdmx-concept:timePeriod .

sdmx-concept:coherInternal
        a                 sdmx:Concept , skos:Concept ;
        rdfs:comment      "Extent to which statistics are consistent within a given data set."@en ;
        rdfs:isDefinedBy  <http://sdmx.org/wp-content/uploads/2009/01/01_sdmx_cog_annex_1_cdc_2009.pdf> ;
        rdfs:label        "Coherence - Internal"@en ;
        skos:broader      sdmx-concept:coherence ;
        skos:inScheme     sdmx-concept:cog ;
        skos:notation     "urn:sdmx:org.sdmx.infomodel.conceptscheme.Concept=SDMX:CROSS_DOMAIN_CONCEPTS[1.0].COHER_INTERNAL" .

sdmx-attribute:title  a   qb:AttributeProperty , rdf:Property ;
        rdfs:comment      "Textual label used as identification of a statistical object."@en ;
        rdfs:isDefinedBy  <http://sdmx.org/wp-content/uploads/2009/01/01_sdmx_cog_annex_1_cdc_2009.pdf> ;
        rdfs:label        "Title"@en ;
        qb:concept        sdmx-concept:title .

sdmx:timeProperty  a        rdf:Property , owl:ObjectProperty , owl:FunctionalProperty ;
        rdfs:comment        "identifies the Concept that specifies the time of the observation of the primaryMeasure"@en ;
        rdfs:label          "time property"@en ;
        rdfs:range          sdmx:DimensionProperty ;
        rdfs:subPropertyOf  sdmx:component .

sdmx:specifiedComponent
        a             rdf:Property , owl:ObjectProperty ;
        rdfs:comment  "Links a component specification to the component property that is being qualified"@en ;
        rdfs:domain   sdmx:ComponentSpecification ;
        rdfs:label    "specified component"@en ;
        rdfs:range    sdmx:ComponentProperty .

sdmx:codeList  a     rdf:Property , owl:ObjectProperty ;
        rdfs:domain  sdmx:CodedProperty ;
        rdfs:label   "code list"@en ;
        rdfs:range   skos:ConceptScheme .

eg:o61  a                  qb:Observation ;
        eg:lifeExpectancy  81.5 ;
        eg:refArea         ex-geo:newport_00pr ;
        qb:dataSet         eg:dataset-le3 .

sdmx-code:sex-T  a         skos:Concept , sdmx:Concept , sdmx-code:Sex ;
        skos:inScheme      sdmx-code:sex ;
        skos:notation      "T" ;
        skos:prefLabel     "Total"@en ;
        skos:topConceptOf  sdmx-code:sex .

sdmx-concept:comparTime
        a                 sdmx:Concept , skos:Concept ;
        rdfs:comment      "Extent to which statistics are comparable or reconcilable over time."@en ;
        rdfs:isDefinedBy  <http://sdmx.org/wp-content/uploads/2009/01/01_sdmx_cog_annex_1_cdc_2009.pdf> ;
        rdfs:label        "Comparability - over time"@en ;
        skos:broader      sdmx-concept:comparability ;
        skos:inScheme     sdmx-concept:cog ;
        skos:notation     "urn:sdmx:org.sdmx.infomodel.conceptscheme.Concept=SDMX:CROSS_DOMAIN_CONCEPTS[1.0].COMPAR_TIME" .

sdmx-metadata:relPolUsAc
        a                 sdmx:MetadataProperty , rdf:Property ;
        rdfs:comment      "The policy for release of the data to users, the scope of dissemination (eg, to the public, to selected users), how users are informed that the data are being released, and whether the policy provides determines the dissemination of statistical data to all users."@en ;
        rdfs:isDefinedBy  <http://sdmx.org/wp-content/uploads/2009/01/01_sdmx_cog_annex_1_cdc_2009.pdf> ;
        rdfs:label        "Release Policy - user access"@en ;
        qb:concept        sdmx-concept:relPolUsAc .

sdmx-metadata:dsi  a      sdmx:MetadataProperty , rdf:Property ;
        rdfs:comment      "Sequence of characters identifying the data set with which it is associated."@en ;
        rdfs:isDefinedBy  <http://sdmx.org/wp-content/uploads/2009/01/01_sdmx_cog_annex_1_cdc_2009.pdf> ;
        rdfs:label        "Data Set Identifier"@en ;
        qb:concept        sdmx-concept:dsi .

sdmx-concept:compilingOrg
        a                 sdmx:Concept , skos:Concept ;
        rdfs:comment      "The organisation compiling the data being reported."@en ;
        rdfs:isDefinedBy  <http://sdmx.org/wp-content/uploads/2009/01/01_sdmx_cog_annex_1_cdc_2009.pdf> ;
        rdfs:label        "Compiling agency"@en ;
        skos:inScheme     sdmx-concept:cog ;
        skos:notation     "urn:sdmx:org.sdmx.infomodel.conceptscheme.Concept=SDMX:CROSS_DOMAIN_CONCEPTS[1.0].COMPILING_ORG" .

sdmx-metadata:dataValInter
        a                 sdmx:MetadataProperty , rdf:Property ;
        rdfs:comment      "Validation that intermediate calculations leading to statistical outputs have been correctly done."@en ;
        rdfs:isDefinedBy  <http://sdmx.org/wp-content/uploads/2009/01/01_sdmx_cog_annex_1_cdc_2009.pdf> ;
        rdfs:label        "Data Validation - intermediate"@en ;
        qb:concept        sdmx-concept:dataValInter .

sdmx-metadata:samplingErr
        a                 sdmx:MetadataProperty , rdf:Property ;
        rdfs:comment      "That part of the difference between a population value and an estimate thereof, derived from a random sample, which is due to the fact that only a subset of the population is enumerated."@en ;
        rdfs:isDefinedBy  <http://sdmx.org/wp-content/uploads/2009/01/01_sdmx_cog_annex_1_cdc_2009.pdf> ;
        rdfs:label        "Accuracy - sampling error"@en ;
        qb:concept        sdmx-concept:samplingErr .

sdmx-metadata:profStatCom
        a                 sdmx:MetadataProperty , rdf:Property ;
        rdfs:comment      "Describes the elements providing assurances that the statistical entity is entitled to comment on erroneous interpretation and misuse of statistics."@en ;
        rdfs:isDefinedBy  <http://sdmx.org/wp-content/uploads/2009/01/01_sdmx_cog_annex_1_cdc_2009.pdf> ;
        rdfs:label        "Professionalism - statistical commentary"@en ;
        qb:concept        sdmx-concept:profStatCom .

sdmx-attribute:dataValInter
        a                 qb:AttributeProperty , rdf:Property ;
        rdfs:comment      "Validation that intermediate calculations leading to statistical outputs have been correctly done."@en ;
        rdfs:isDefinedBy  <http://sdmx.org/wp-content/uploads/2009/01/01_sdmx_cog_annex_1_cdc_2009.pdf> ;
        rdfs:label        "Data Validation - intermediate"@en ;
        qb:concept        sdmx-concept:dataValInter .

sdmx-attribute:iMResRel
        a                 qb:AttributeProperty , rdf:Property ;
        rdfs:comment      "Measures to encourage statistical reporting and/or to sanction non-reporting."@en ;
        rdfs:isDefinedBy  <http://sdmx.org/wp-content/uploads/2009/01/01_sdmx_cog_annex_1_cdc_2009.pdf> ;
        rdfs:label        "Institutional Mandate - respondent relations."@en ;
        qb:concept        sdmx-concept:iMResRel .

sdmx-attribute:accuracy
        a                 qb:AttributeProperty , rdf:Property ;
        rdfs:comment      "Closeness of computations or estimates to the exact or true values that the statistics were intended to measure."@en ;
        rdfs:isDefinedBy  <http://sdmx.org/wp-content/uploads/2009/01/01_sdmx_cog_annex_1_cdc_2009.pdf> ;
        rdfs:label        "Accuracy"@en ;
        qb:concept        sdmx-concept:accuracy .

sdmx-concept:punctuality
        a                 sdmx:Concept , skos:Concept ;
        rdfs:comment      "Time lag between the actual delivery of the data and the target date when it should have been delivered."@en ;
        rdfs:isDefinedBy  <http://sdmx.org/wp-content/uploads/2009/01/01_sdmx_cog_annex_1_cdc_2009.pdf> ;
        rdfs:label        "Punctuality"@en ;
        skos:inScheme     sdmx-concept:cog ;
        skos:notation     "urn:sdmx:org.sdmx.infomodel.conceptscheme.Concept=SDMX:CROSS_DOMAIN_CONCEPTS[1.0].PUNCTUALITY" .

sdmx-concept:timePeriod
        a                 sdmx:Concept , skos:Concept , sdmx:TimeRole ;
        rdfs:comment      "The period of time or point in time to which the measured observation refers."@en ;
        rdfs:isDefinedBy  <http://sdmx.org/wp-content/uploads/2009/01/01_sdmx_cog_annex_1_cdc_2009.pdf> ;
        rdfs:label        "Time Period"@en ;
        skos:inScheme     sdmx-concept:cog ;
        skos:notation     "urn:sdmx:org.sdmx.infomodel.conceptscheme.Concept=SDMX:CROSS_DOMAIN_CONCEPTS[1.0].TIME_PERIOD" .

sdmx-attribute:visArea
        a                 qb:AttributeProperty , rdf:Property ;
        rdfs:comment      "The secondary area, as opposed to reference area, to which the measured data is in relation."@en ;
        rdfs:isDefinedBy  <http://sdmx.org/wp-content/uploads/2009/01/01_sdmx_cog_annex_1_cdc_2009.pdf> ;
        rdfs:label        "Counterpart Reference Area"@en ;
        qb:concept        sdmx-concept:visArea .

sdmx-metadata:prof  a     sdmx:MetadataProperty , rdf:Property ;
        rdfs:comment      "The standard, skill and ability suitable for producing statistics of good quality."@en ;
        rdfs:isDefinedBy  <http://sdmx.org/wp-content/uploads/2009/01/01_sdmx_cog_annex_1_cdc_2009.pdf> ;
        rdfs:label        "Professionalism"@en ;
        qb:concept        sdmx-concept:prof .

sdmx-subject:1.10  a     skos:Concept , sdmx:Concept , sdmx-subject:SubjectMatterDomain ;
        skos:broader     sdmx-subject:1 ;
        skos:definition  "Political and other community activities - statistics on voting turnout, participation in political and other community activities, trade union membership, social dialogue, civil society, social capital, etc."@en ;
        skos:notation    "1.10" ;
        skos:prefLabel   "Political and other community activities"@en .

sdmx-concept:unitMeasDetail
        a                 sdmx:Concept , skos:Concept ;
        rdfs:comment      "Additional textual information on the unit of measure."@en ;
        rdfs:isDefinedBy  <http://sdmx.org/wp-content/uploads/2009/01/01_sdmx_cog_annex_1_cdc_2009.pdf> ;
        rdfs:label        "Unit of Measure Detail"@en ;
        skos:broader      sdmx-concept:unitMeasure ;
        skos:inScheme     sdmx-concept:cog ;
        skos:notation     "urn:sdmx:org.sdmx.infomodel.conceptscheme.Concept=SDMX:CROSS_DOMAIN_CONCEPTS[1.0].UNIT_MEAS_DETAIL" .

sdmx:metadataFlow  a  rdf:Property , owl:ObjectProperty ;
        rdfs:comment  "gives the metadata flow associated with a metadata set"@en ;
        rdfs:domain   sdmx:MetadataSet ;
        rdfs:label    "metadata flow"@en ;
        rdfs:range    sdmx:MetadataFlow .

sdmx-attribute:instManLaOa
        a                 qb:AttributeProperty , rdf:Property ;
        rdfs:comment      "Legal acts or other formal or informal agreements that assign responsibility as well as the authority to an agency for the collection, processing, and dissemination of statistics."@en ;
        rdfs:isDefinedBy  <http://sdmx.org/wp-content/uploads/2009/01/01_sdmx_cog_annex_1_cdc_2009.pdf> ;
        rdfs:label        "Institutional Mandate - legal acts and other agreements."@en ;
        qb:concept        sdmx-concept:instManLaOa .

sdmx-concept:dissDet  a   sdmx:Concept , skos:Concept ;
        rdfs:comment      "Disseminated domain, measure, and time period breakdowns of statistics in the dataset."@en ;
        rdfs:isDefinedBy  <http://sdmx.org/wp-content/uploads/2009/01/01_sdmx_cog_annex_1_cdc_2009.pdf> ;
        rdfs:label        "Data Presentation - disseminated detail"@en ;
        skos:broader      sdmx-concept:dataPres ;
        skos:inScheme     sdmx-concept:cog ;
        skos:notation     "urn:sdmx:org.sdmx.infomodel.conceptscheme.Concept=SDMX:CROSS_DOMAIN_CONCEPTS[1.0].DISS_DET" .

sdmx-concept:accessibility
        a                 sdmx:Concept , skos:Concept ;
        rdfs:comment      "The ease and the conditions under which statistical information can be obtained."@en ;
        rdfs:isDefinedBy  <http://sdmx.org/wp-content/uploads/2009/01/01_sdmx_cog_annex_1_cdc_2009.pdf> ;
        rdfs:label        "Accessibility"@en ;
        skos:inScheme     sdmx-concept:cog ;
        skos:notation     "urn:sdmx:org.sdmx.infomodel.conceptscheme.Concept=SDMX:CROSS_DOMAIN_CONCEPTS[1.0].ACCESSIBILITY" .

sdmx-concept:mAgency  a   sdmx:Concept , skos:Concept ;
        rdfs:comment      "The organisation or other expert body that maintains a domain-specific data or metadata structure definition."@en ;
        rdfs:isDefinedBy  <http://sdmx.org/wp-content/uploads/2009/01/01_sdmx_cog_annex_1_cdc_2009.pdf> ;
        rdfs:label        "Maintenance Agency"@en ;
        skos:inScheme     sdmx-concept:cog ;
        skos:notation     "urn:sdmx:org.sdmx.infomodel.conceptscheme.Concept=SDMX:CROSS_DOMAIN_CONCEPTS[1.0].M_AGENCY" .

sdmx-concept:relPolUsAc
        a                 sdmx:Concept , skos:Concept ;
        rdfs:comment      "The policy for release of the data to users, the scope of dissemination (eg, to the public, to selected users), how users are informed that the data are being released, and whether the policy provides determines the dissemination of statistical data to all users."@en ;
        rdfs:isDefinedBy  <http://sdmx.org/wp-content/uploads/2009/01/01_sdmx_cog_annex_1_cdc_2009.pdf> ;
        rdfs:label        "Release Policy - user access"@en ;
        skos:broader      sdmx-concept:relPolicy ;
        skos:inScheme     sdmx-concept:cog ;
        skos:notation     "urn:sdmx:org.sdmx.infomodel.conceptscheme.Concept=SDMX:CROSS_DOMAIN_CONCEPTS[1.0].REL_POL_US_AC" .

sdmx-code:decimals-1  a    skos:Concept , sdmx:Concept , sdmx-code:Decimals ;
        skos:inScheme      sdmx-code:decimals ;
        skos:notation      "1" ;
        skos:prefLabel     "One"@en ;
        skos:topConceptOf  sdmx-code:decimals .

sdmx:CodedProperty  a    rdfs:Class , owl:Class ;
        rdfs:comment     "Superclass of all coded ComponentProperties"@en ;
        rdfs:label       "Coded property"@en ;
        rdfs:subClassOf  sdmx:ComponentProperty .

sdmx-attribute:dataRev
        a                 qb:AttributeProperty , rdf:Property ;
        rdfs:comment      "Any change in a value of a statistic released to the public."@en ;
        rdfs:isDefinedBy  <http://sdmx.org/wp-content/uploads/2009/01/01_sdmx_cog_annex_1_cdc_2009.pdf> ;
        rdfs:label        "Data Revision"@en ;
        qb:concept        sdmx-concept:dataRev .

sdmx-metadata:qualityMgmnt
        a                 sdmx:MetadataProperty , rdf:Property ;
        rdfs:comment      "Systems and frameworks in place within an organisation to manage the quality of statistical products and processes."@en ;
        rdfs:isDefinedBy  <http://sdmx.org/wp-content/uploads/2009/01/01_sdmx_cog_annex_1_cdc_2009.pdf> ;
        rdfs:label        "Quality Management"@en ;
        qb:concept        sdmx-concept:qualityMgmnt .

eg:lifeExpectancy  a        rdf:Property , qb:MeasureProperty ;
        rdfs:label          "life expectancy"@en ;
        rdfs:range          xsd:decimal ;
        rdfs:subPropertyOf  sdmx-measure:obsValue .

sdmx-attribute:qualityMgmnt
        a                 qb:AttributeProperty , rdf:Property ;
        rdfs:comment      "Systems and frameworks in place within an organisation to manage the quality of statistical products and processes."@en ;
        rdfs:isDefinedBy  <http://sdmx.org/wp-content/uploads/2009/01/01_sdmx_cog_annex_1_cdc_2009.pdf> ;
        rdfs:label        "Quality Management"@en ;
        qb:concept        sdmx-concept:qualityMgmnt .

sdmx:Attachable  a    rdfs:Class , owl:Class ;
        rdfs:comment  "Abstract superclass for everything that can have attributes and dimensions"@en ;
        rdfs:label    "Attachable (abstract)"@en .

sdmx-concept:currency
        a                 sdmx:Concept , skos:Concept ;
        rdfs:comment      "Monetary denomination of the object being measured."@en ;
        rdfs:isDefinedBy  <http://sdmx.org/wp-content/uploads/2009/01/01_sdmx_cog_annex_1_cdc_2009.pdf> ;
        rdfs:label        "Currency"@en ;
        skos:inScheme     sdmx-concept:cog ;
        skos:notation     "urn:sdmx:org.sdmx.infomodel.conceptscheme.Concept=SDMX:CROSS_DOMAIN_CONCEPTS[1.0].CURRENCY" .

sdmx:TimeRole  a         rdfs:Class , owl:Class ;
        rdfs:comment     "concept for a dimension that specifies the time of the observation of the primaryMeasure"@en ;
        rdfs:label       "Time property"@en ;
        rdfs:subClassOf  sdmx:ConceptRole .

eg:o42  a                  qb:Observation ;
        eg:lifeExpectancy  83.7 ;
        eg:refArea         ex-geo:cardiff_00pt ;
        qb:dataSet         eg:dataset-le3 .

sdmx-concept:decimals
        a                 sdmx:Concept , skos:Concept ;
        rdfs:comment      "The number of digits of an observation to the right of a decimal point."@en ;
        rdfs:isDefinedBy  <http://sdmx.org/wp-content/uploads/2009/01/01_sdmx_cog_annex_1_cdc_2009.pdf> ;
        rdfs:label        "Decimals"@en ;
        skos:inScheme     sdmx-concept:cog ;
        skos:notation     "urn:sdmx:org.sdmx.infomodel.conceptscheme.Concept=SDMX:CROSS_DOMAIN_CONCEPTS[1.0].DECIMALS" .

sdmx-metadata:currency
        a                 sdmx:MetadataProperty , rdf:Property , qb:CodedProperty ;
        rdfs:comment      "Monetary denomination of the object being measured."@en ;
        rdfs:isDefinedBy  <http://sdmx.org/wp-content/uploads/2009/01/01_sdmx_cog_annex_1_cdc_2009.pdf> ;
        rdfs:label        "Currency"@en ;
        rdfs:range        sdmx-code:Currency ;
        qb:codeList       sdmx-code:currency ;
        qb:concept        sdmx-concept:currency .

sdmx-code:unitMult-2  a    skos:Concept , sdmx:Concept , sdmx-code:UnitMult ;
        skos:inScheme      sdmx-code:unitMult ;
        skos:notation      "2" ;
        skos:prefLabel     "Hundreds"@en ;
        skos:topConceptOf  sdmx-code:unitMult .

sdmx-metadata:decimals
        a                 sdmx:MetadataProperty , rdf:Property , qb:CodedProperty ;
        rdfs:comment      "The number of digits of an observation to the right of a decimal point."@en ;
        rdfs:isDefinedBy  <http://sdmx.org/wp-content/uploads/2009/01/01_sdmx_cog_annex_1_cdc_2009.pdf> ;
        rdfs:label        "Decimals"@en ;
        rdfs:range        sdmx-code:Decimals ;
        qb:codeList       sdmx-code:decimals ;
        qb:concept        sdmx-concept:decimals .

eg:slice5  a                qb:Slice ;
        eg:refPeriod        <http://reference.data.gov.uk/id/gregorian-interval/2006-01-01T00:00:00/P3Y> ;
        qb:observation      eg:o51 , eg:o52 , eg:o53 , eg:o54 ;
        qb:sliceStructure   eg:sliceByRegion ;
        sdmx-dimension:sex  sdmx-code:sex-M .

sdmx-subject:1.8  a      skos:Concept , sdmx:Concept , sdmx-subject:SubjectMatterDomain ;
        skos:broader     sdmx-subject:1 ;
        skos:definition  "Justice and crime - activities including crime, convictions, operation of criminal justice systems, justice, safety, victims, clear-up rates, prison population, illicit drug production, trafficking and use, etc."@en ;
        skos:notation    "1.8" ;
        skos:prefLabel   "Justice and crime"@en .

sdmx-code:timeFormat-102
        a                  skos:Concept , sdmx:Concept , sdmx-code:TimeFormat ;
        skos:definition    "(for daily and business series)\nyear/month/day"@en ;
        skos:inScheme      sdmx-code:timeFormat ;
        skos:notation      "102" ;
        skos:prefLabel     "CCYYMMDD"@en ;
        skos:topConceptOf  sdmx-code:timeFormat .

sdmx-measure:educationLev
        a                 qb:MeasureProperty , rdf:Property ;
        rdfs:comment      "The highest level of an educational programme the person has successfully completed."@en ;
        rdfs:isDefinedBy  <http://sdmx.org/wp-content/uploads/2009/01/01_sdmx_cog_annex_1_cdc_2009.pdf> ;
        rdfs:label        "Education Level"@en ;
        qb:concept        sdmx-concept:educationLev .

sdmx-attribute:contactOrganisation
        a                 qb:AttributeProperty , rdf:Property ;
        rdfs:comment      "The name of the organisation of the contact points for the data or metadata."@en ;
        rdfs:isDefinedBy  <http://sdmx.org/wp-content/uploads/2009/01/01_sdmx_cog_annex_1_cdc_2009.pdf> ;
        rdfs:label        "Contact organisation"@en ;
        qb:concept        sdmx-concept:contactOrganisation .

sdmx-attribute:classSystem
        a                 qb:AttributeProperty , rdf:Property ;
        rdfs:comment      "Arrangement or division of objects into groups based on characteristics which the objects have in common."@en ;
        rdfs:isDefinedBy  <http://sdmx.org/wp-content/uploads/2009/01/01_sdmx_cog_annex_1_cdc_2009.pdf> ;
        rdfs:label        "Classification systems"@en ;
        qb:concept        sdmx-concept:classSystem .

sdmx-concept:clarity  a   sdmx:Concept , skos:Concept ;
        rdfs:comment      "The extent to which easily comprehensible metadata are available, where these metadata are necessary to give a full understanding of statistical data."@en ;
        rdfs:isDefinedBy  <http://sdmx.org/wp-content/uploads/2009/01/01_sdmx_cog_annex_1_cdc_2009.pdf> ;
        rdfs:label        "Clarity"@en ;
        skos:inScheme     sdmx-concept:cog ;
        skos:notation     "urn:sdmx:org.sdmx.infomodel.conceptscheme.Concept=SDMX:CROSS_DOMAIN_CONCEPTS[1.0].CLARITY" .

sdmx-code:timeFormat-P7D
        a                  skos:Concept , sdmx:Concept , sdmx-code:TimeFormat ;
        skos:inScheme      sdmx-code:timeFormat ;
        skos:notation      "P7D" ;
        skos:prefLabel     "Weekly"@en ;
        skos:topConceptOf  sdmx-code:timeFormat .

sdmx-attribute:contact
        a                 qb:AttributeProperty , rdf:Property ;
        rdfs:comment      "Individual or organisational contact points for the data or metadata, including information on how to reach the contact points."@en ;
        rdfs:isDefinedBy  <http://sdmx.org/wp-content/uploads/2009/01/01_sdmx_cog_annex_1_cdc_2009.pdf> ;
        rdfs:label        "Contact"@en ;
        qb:concept        sdmx-concept:contact .

sdmx-code:timeFormat-719
        a                  skos:Concept , sdmx:Concept , sdmx-code:TimeFormat ;
        skos:definition    "(for series with freq. higher than daily)\nyear/month/day/hours/minutes to year/month/day/hours/minutes."@en ;
        skos:inScheme      sdmx-code:timeFormat ;
        skos:notation      "719" ;
        skos:prefLabel     "CCYYMMDDhhmmmCCYYMMDDhhmmm"@en ;
        skos:topConceptOf  sdmx-code:timeFormat .

sdmx-concept:coherXDom
        a                 sdmx:Concept , skos:Concept ;
        rdfs:comment      "Extent to which statistics are reconcilable with those obtained through other data sources or statistical domains."@en ;
        rdfs:isDefinedBy  <http://sdmx.org/wp-content/uploads/2009/01/01_sdmx_cog_annex_1_cdc_2009.pdf> ;
        rdfs:label        "Coherence - cross domain"@en ;
        skos:broader      sdmx-concept:coherence ;
        skos:inScheme     sdmx-concept:cog ;
        skos:notation     "urn:sdmx:org.sdmx.infomodel.conceptscheme.Concept=SDMX:CROSS_DOMAIN_CONCEPTS[1.0].COHER_X_DOM" .

sdmx:Concept  a          rdfs:Class , owl:Class ;
        rdfs:comment     "Denotes an SDMX concept, used in the particular SDMX terminological sense, which is in principle narrower than skos:Concept" ;
        rdfs:label       "concept"@en ;
        rdfs:subClassOf  skos:Concept .

sdmx:concept  a      rdf:Property , owl:ObjectProperty ;
        rdfs:domain  sdmx:ComponentProperty ;
        rdfs:label   "concept"@en ;
        rdfs:range   sdmx:Concept .

sdmx:structure  a    rdf:Property , owl:ObjectProperty ;
        rdfs:domain  sdmx:DataSetOrFlow , sdmx:Structured ;
        rdfs:label   "structure"@en ;
        rdfs:range   sdmx:DataStructureDefinition , sdmx:Structure .

sdmx-attribute:repAgency
        a                 qb:AttributeProperty , rdf:Property ;
        rdfs:comment      "The organisation that supplies the data for a given  instance of the statistics."@en ;
        rdfs:isDefinedBy  <http://sdmx.org/wp-content/uploads/2009/01/01_sdmx_cog_annex_1_cdc_2009.pdf> ;
        rdfs:label        "Reporting Agency"@en ;
        qb:concept        sdmx-concept:repAgency .

sdmx-metadata:age  a      sdmx:MetadataProperty , rdf:Property ;
        rdfs:comment      "The length of time that a person has lived or a thing has existed."@en ;
        rdfs:isDefinedBy  <http://sdmx.org/wp-content/uploads/2009/01/01_sdmx_cog_annex_1_cdc_2009.pdf> ;
        rdfs:label        "Age"@en ;
        qb:concept        sdmx-concept:age .

sdmx-code:freq-D  a        skos:Concept , sdmx:Concept , sdmx-code:Freq ;
        skos:inScheme      sdmx-code:freq ;
        skos:notation      "D" ;
        skos:prefLabel     "Daily"@en ;
        skos:topConceptOf  sdmx-code:freq .

sdmx:commponentRequired
        a             rdf:Property , owl:DatatypeProperty ;
        rdfs:comment  "Indicates whether a component property is required (true) or optional (false) in the context of a DSD or MSD"@en ;
        rdfs:domain   sdmx:ComponentSpecifition ;
        rdfs:label    "component required"@en ;
        rdfs:range    xsd:boolean .

sdmx-attribute:dataUpdate
        a                 qb:AttributeProperty , rdf:Property ;
        rdfs:comment      "The date on which the data element was inserted or modified in the database."@en ;
        rdfs:isDefinedBy  <http://sdmx.org/wp-content/uploads/2009/01/01_sdmx_cog_annex_1_cdc_2009.pdf> ;
        rdfs:label        "Data Update"@en ;
        qb:concept        sdmx-concept:dataUpdate .

sdmx-metadata:contactMail
        a                   sdmx:MetadataProperty , rdf:Property ;
        rdfs:comment        "The postal address of the contact points for the data or metadata."@en ;
        rdfs:isDefinedBy    <http://sdmx.org/wp-content/uploads/2009/01/01_sdmx_cog_annex_1_cdc_2009.pdf> ;
        rdfs:label          "Contact mail address"@en ;
        rdfs:subPropertyOf  vcard:adr ;
        qb:concept          sdmx-concept:contactMail .

sdmx-subject:2.9  a      skos:Concept , sdmx:Concept , sdmx-subject:SubjectMatterDomain ;
        skos:broader     sdmx-subject:2 ;
        skos:definition  "Science, technology and innovation - includes Research and Development (R&D), innovation, patents, human resources (in science, technology and innovation), high tech industries and knowledge based services, biotechnology, financing of R&D and innovation. \nExcludes: \n- information and communication technologies (ICTs) (3.3.3)"@en ;
        skos:notation    "2.9" ;
        skos:prefLabel   "Science, technology and innovation"@en .

sdmx-attribute:newsRel
        a                 qb:AttributeProperty , rdf:Property ;
        rdfs:comment      "Regular or ad-hoc press releases linked to the data."@en ;
        rdfs:isDefinedBy  <http://sdmx.org/wp-content/uploads/2009/01/01_sdmx_cog_annex_1_cdc_2009.pdf> ;
        rdfs:label        "Dissemination Format - news release"@en ;
        qb:concept        sdmx-concept:newsRel .

sdmx-code:timeFormat-203
        a                  skos:Concept , sdmx:Concept , sdmx-code:TimeFormat ;
        skos:definition    "(for series with freq. higher than daily)\nyear/month/day/hours/minutes"@en ;
        skos:inScheme      sdmx-code:timeFormat ;
        skos:notation      "203" ;
        skos:prefLabel     "CCYYMMDDhhmm"@en ;
        skos:topConceptOf  sdmx-code:timeFormat .

sdmx-concept:relPolTra
        a                 sdmx:Concept , skos:Concept ;
        rdfs:comment      "Dissemination of the release policy to the public."@en ;
        rdfs:isDefinedBy  <http://sdmx.org/wp-content/uploads/2009/01/01_sdmx_cog_annex_1_cdc_2009.pdf> ;
        rdfs:label        "Release Policy - transparency"@en ;
        skos:broader      sdmx-concept:relPolicy ;
        skos:inScheme     sdmx-concept:cog ;
        skos:notation     "urn:sdmx:org.sdmx.infomodel.conceptscheme.Concept=SDMX:CROSS_DOMAIN_CONCEPTS[1.0].REL_POL_TRA" .

eg:o23  a                  qb:Observation ;
        eg:lifeExpectancy  81.3 ;
        eg:refArea         ex-geo:monmouthshire_00pp ;
        qb:dataSet         eg:dataset-le3 .

sdmx-attribute:comparability
        a                 qb:AttributeProperty , rdf:Property ;
        rdfs:comment      "The extent to which differences between statistics can be attributed to differences between the true values of the statistical characteristics."@en ;
        rdfs:isDefinedBy  <http://sdmx.org/wp-content/uploads/2009/01/01_sdmx_cog_annex_1_cdc_2009.pdf> ;
        rdfs:label        "Comparability"@en ;
        qb:concept        sdmx-concept:comparability .

sdmx-metadata:confDataTr
        a                 sdmx:MetadataProperty , rdf:Property ;
        rdfs:comment      "Rules applied for treating the data set to ensure statistical confidentiality and prevent unauthorised disclosure."@en ;
        rdfs:isDefinedBy  <http://sdmx.org/wp-content/uploads/2009/01/01_sdmx_cog_annex_1_cdc_2009.pdf> ;
        rdfs:label        "Confidentiality - data treatment"@en ;
        qb:concept        sdmx-concept:confDataTr .

sdmx-concept:organisationUnit
        a                 sdmx:Concept , skos:Concept ;
        rdfs:comment      "An addressable subdivision of an organization."@en ;
        rdfs:isDefinedBy  <http://sdmx.org/wp-content/uploads/2009/01/01_sdmx_cog_annex_1_cdc_2009.pdf> ;
        rdfs:label        "Contact organization unit"@en ;
        skos:broader      sdmx-concept:contact ;
        skos:inScheme     sdmx-concept:cog ;
        skos:notation     "urn:sdmx:org.sdmx.infomodel.conceptscheme.Concept=SDMX:CROSS_DOMAIN_CONCEPTS[1.0].ORGANISATION_UNIT" .

sdmx-metadata:qualityDoc
        a                 sdmx:MetadataProperty , rdf:Property ;
        rdfs:comment      "Documentation on procedures applied for quality management and quality assessment."@en ;
        rdfs:isDefinedBy  <http://sdmx.org/wp-content/uploads/2009/01/01_sdmx_cog_annex_1_cdc_2009.pdf> ;
        rdfs:label        "Quality Management - documentation"@en ;
        qb:concept        sdmx-concept:qualityDoc .

sdmx-code:timeFormat-P6M
        a                  skos:Concept , sdmx:Concept , sdmx-code:TimeFormat ;
        skos:inScheme      sdmx-code:timeFormat ;
        skos:notation      "P6M" ;
        skos:prefLabel     "Half-yearly"@en ;
        skos:topConceptOf  sdmx-code:timeFormat .

sdmx-metadata:timeOutput
        a                 sdmx:MetadataProperty , rdf:Property ;
        rdfs:comment      "The lapse of time between the end of a reference period and dissemination of the data."@en ;
        rdfs:isDefinedBy  <http://sdmx.org/wp-content/uploads/2009/01/01_sdmx_cog_annex_1_cdc_2009.pdf> ;
        rdfs:label        "Timeliness - output"@en ;
        qb:concept        sdmx-concept:timeOutput .

sdmx-attribute:statUnit
        a                 qb:AttributeProperty , rdf:Property ;
        rdfs:comment      "Entity for which information is sought and for which statistics are ultimately compiled."@en ;
        rdfs:isDefinedBy  <http://sdmx.org/wp-content/uploads/2009/01/01_sdmx_cog_annex_1_cdc_2009.pdf> ;
        rdfs:label        "Statistical Unit"@en ;
        qb:concept        sdmx-concept:statUnit .

sdmx-metadata:profImp
        a                 sdmx:MetadataProperty , rdf:Property ;
        rdfs:comment      "Description of the elements providing assurances that statistics are produced on an impartial basis."@en ;
        rdfs:isDefinedBy  <http://sdmx.org/wp-content/uploads/2009/01/01_sdmx_cog_annex_1_cdc_2009.pdf> ;
        rdfs:label        "Professionalism - impartiality"@en ;
        qb:concept        sdmx-concept:profImp .

sdmx:controllingAgreement
        a            rdf:Property , owl:ObjectProperty ;
        rdfs:domain  sdmx:DataFlow , sdmx:Flow ;
        rdfs:label   "controlling agreement"@en ;
        rdfs:range   sdmx:ProvisionAgreement .

sdmx-subject:3.3.6  a    skos:Concept , sdmx:Concept , sdmx-subject:SubjectMatterDomain ;
        skos:broader     sdmx-subject:3.3 ;
        skos:definition  "Sustainable development - work on indicators and frameworks to monitor the economic, social and environmental dimensions of sustainable development."@en ;
        skos:notation    "3.3.6" ;
        skos:prefLabel   "Sustainable development"@en .

sdmx-metadata:timeSource
        a                 sdmx:MetadataProperty , rdf:Property ;
        rdfs:comment      "The time between the end of a reference period and actual receipt of the data by the compiling agency."@en ;
        rdfs:isDefinedBy  <http://sdmx.org/wp-content/uploads/2009/01/01_sdmx_cog_annex_1_cdc_2009.pdf> ;
        rdfs:label        "Timeliness - source data"@en ;
        qb:concept        sdmx-concept:timeSource .

sdmx-subject:2.4.2  a    skos:Concept , sdmx:Concept , sdmx-subject:SubjectMatterDomain ;
        skos:broader     sdmx-subject:2.4 ;
        skos:definition  "Energy - energy supply, energy use, energy balances, security of supply, energy markets, trade in energy, energy efficiency, renewable energy sources, government expenditure on energy.\nExcludes\n- energy prices (2.7)"@en ;
        skos:notation    "2.4.2" ;
        skos:prefLabel   "Energy"@en .

sdmx-concept:iMResRel
        a                 sdmx:Concept , skos:Concept ;
        rdfs:comment      "Measures to encourage statistical reporting and/or to sanction non-reporting."@en ;
        rdfs:isDefinedBy  <http://sdmx.org/wp-content/uploads/2009/01/01_sdmx_cog_annex_1_cdc_2009.pdf> ;
        rdfs:label        "Institutional Mandate - respondent relations."@en ;
        skos:broader      sdmx-concept:instMandate ;
        skos:inScheme     sdmx-concept:cog ;
        skos:notation     "urn:sdmx:org.sdmx.infomodel.conceptscheme.Concept=SDMX:CROSS_DOMAIN_CONCEPTS[1.0].I_M_RES_REL" .

sdmx-metadata:indType
        a                 sdmx:MetadataProperty , rdf:Property ;
        rdfs:comment      "The type of index number used in the statistical production process."@en ;
        rdfs:isDefinedBy  <http://sdmx.org/wp-content/uploads/2009/01/01_sdmx_cog_annex_1_cdc_2009.pdf> ;
        rdfs:label        "Index Type"@en ;
        qb:concept        sdmx-concept:indType .

sdmx-concept:instManLaOa
        a                 sdmx:Concept , skos:Concept ;
        rdfs:comment      "Legal acts or other formal or informal agreements that assign responsibility as well as the authority to an agency for the collection, processing, and dissemination of statistics."@en ;
        rdfs:isDefinedBy  <http://sdmx.org/wp-content/uploads/2009/01/01_sdmx_cog_annex_1_cdc_2009.pdf> ;
        rdfs:label        "Institutional Mandate - legal acts and other agreements."@en ;
        skos:broader      sdmx-concept:instMandate ;
        skos:inScheme     sdmx-concept:cog ;
        skos:notation     "urn:sdmx:org.sdmx.infomodel.conceptscheme.Concept=SDMX:CROSS_DOMAIN_CONCEPTS[1.0].INST_MAN_LA_OA" .

sdmx-concept:accuracy
        a                 sdmx:Concept , skos:Concept ;
        rdfs:comment      "Closeness of computations or estimates to the exact or true values that the statistics were intended to measure."@en ;
        rdfs:isDefinedBy  <http://sdmx.org/wp-content/uploads/2009/01/01_sdmx_cog_annex_1_cdc_2009.pdf> ;
        rdfs:label        "Accuracy"@en ;
        skos:inScheme     sdmx-concept:cog ;
        skos:notation     "urn:sdmx:org.sdmx.infomodel.conceptscheme.Concept=SDMX:CROSS_DOMAIN_CONCEPTS[1.0].ACCURACY" .

sdmx-concept:dissOther
        a                 sdmx:Concept , skos:Concept ;
        rdfs:comment      "References to the most important other data dissemination done."@en ;
        rdfs:isDefinedBy  <http://sdmx.org/wp-content/uploads/2009/01/01_sdmx_cog_annex_1_cdc_2009.pdf> ;
        rdfs:label        "Dissemination Format - other"@en ;
        skos:broader      sdmx-concept:dissFormat ;
        skos:inScheme     sdmx-concept:cog ;
        skos:notation     "urn:sdmx:org.sdmx.infomodel.conceptscheme.Concept=SDMX:CROSS_DOMAIN_CONCEPTS[1.0].DISS_OTHER" .

sdmx-subject:1.3  a      skos:Concept , sdmx:Concept , sdmx-subject:SubjectMatterDomain ;
        skos:broader     sdmx-subject:1 ;
        skos:definition  "Education - includes educational participation, illiteracy, educational institutions and systems, human and financial resources invested in education, lifelong learning, vocational training and adult learning, impact of education, assessments of student performance, etc."@en ;
        skos:notation    "1.3" ;
        skos:prefLabel   "Education"@en .

sdmx-metadata:iMResRel
        a                 sdmx:MetadataProperty , rdf:Property ;
        rdfs:comment      "Measures to encourage statistical reporting and/or to sanction non-reporting."@en ;
        rdfs:isDefinedBy  <http://sdmx.org/wp-content/uploads/2009/01/01_sdmx_cog_annex_1_cdc_2009.pdf> ;
        rdfs:label        "Institutional Mandate - respondent relations."@en ;
        qb:concept        sdmx-concept:iMResRel .

sdmx-concept:civilStatus
        a                 sdmx:Concept , skos:Concept ;
        rdfs:comment      "Legal, conjugal status of each individual in relation to the marriage laws or customs of the country."@en ;
        rdfs:isDefinedBy  <http://sdmx.org/wp-content/uploads/2009/01/01_sdmx_cog_annex_1_cdc_2009.pdf> ;
        rdfs:label        "Civil Status"@en ;
        skos:inScheme     sdmx-concept:cog ;
        skos:notation     "urn:sdmx:org.sdmx.infomodel.conceptscheme.Concept=SDMX:CROSS_DOMAIN_CONCEPTS[1.0].CIVIL_STATUS" .

sdmx-metadata:accuracy
        a                 sdmx:MetadataProperty , rdf:Property ;
        rdfs:comment      "Closeness of computations or estimates to the exact or true values that the statistics were intended to measure."@en ;
        rdfs:isDefinedBy  <http://sdmx.org/wp-content/uploads/2009/01/01_sdmx_cog_annex_1_cdc_2009.pdf> ;
        rdfs:label        "Accuracy"@en ;
        qb:concept        sdmx-concept:accuracy .

sdmx-concept:basePer  a   sdmx:Concept , skos:Concept ;
        rdfs:comment      "The period of time used as the base of an index number, or to which a constant price series refers."@en ;
        rdfs:isDefinedBy  <http://sdmx.org/wp-content/uploads/2009/01/01_sdmx_cog_annex_1_cdc_2009.pdf> ;
        rdfs:label        "Base Period"@en ;
        skos:inScheme     sdmx-concept:cog ;
        skos:notation     "urn:sdmx:org.sdmx.infomodel.conceptscheme.Concept=SDMX:CROSS_DOMAIN_CONCEPTS[1.0].BASE_PER" .

sdmx-attribute:relPolLegActs
        a                 qb:AttributeProperty , rdf:Property ;
        rdfs:comment      "Legal acts and other agreements pertaining to data access."@en ;
        rdfs:isDefinedBy  <http://sdmx.org/wp-content/uploads/2009/01/01_sdmx_cog_annex_1_cdc_2009.pdf> ;
        rdfs:label        "Release Policy - legal acts and other agreements"@en ;
        qb:concept        sdmx-concept:relPolLegActs .

sdmx-metadata:relPolTra
        a                 sdmx:MetadataProperty , rdf:Property ;
        rdfs:comment      "Dissemination of the release policy to the public."@en ;
        rdfs:isDefinedBy  <http://sdmx.org/wp-content/uploads/2009/01/01_sdmx_cog_annex_1_cdc_2009.pdf> ;
        rdfs:label        "Release Policy - transparency"@en ;
        qb:concept        sdmx-concept:relPolTra .

sdmx-attribute:relPolicy
        a                 qb:AttributeProperty , rdf:Property ;
        rdfs:comment      "Rules for disseminating statistical data to interested parties."@en ;
        rdfs:isDefinedBy  <http://sdmx.org/wp-content/uploads/2009/01/01_sdmx_cog_annex_1_cdc_2009.pdf> ;
        rdfs:label        "Release Policy"@en ;
        qb:concept        sdmx-concept:relPolicy .

sdmx:CountProperty  a     rdfs:Class , owl:Class ;
        rdfs:label        "Count property"@en ;
        rdfs:subClassOf   sdmx:ConceptRoleProperty ;
        owl:disjointWith  sdmx:MeasureProperty .

sdmx-metadata:origDataId
        a                 sdmx:MetadataProperty , rdf:Property ;
        rdfs:comment      "The data identifier as found in the originating database."@en ;
        rdfs:isDefinedBy  <http://sdmx.org/wp-content/uploads/2009/01/01_sdmx_cog_annex_1_cdc_2009.pdf> ;
        rdfs:label        "Original Data Identifier"@en ;
        qb:concept        sdmx-concept:origDataId .

sdmx-subject:2.4  a      skos:Concept , sdmx:Concept , sdmx-subject:SubjectMatterDomain ;
        skos:broader     sdmx-subject:2 ;
        skos:definition  "Sectoral statistics - statistical activities dealing with one of the specific branches of industry or services mentioned at the three digit level of the classification.\nExcludes: \n- education (1.3) \n- health (1.4)\n- social security (1.6)\n- culture (1.9)\n- statistics covering the whole industrial sector (2.3)\n- statistics covering the whole service or market service sector (2.3)\n- distributive trade (2.3)\n- government and public sector statistics (2.5)\n- research and development (2.9) \n- telecommunication statistics (3.3.3)"@en ;
        skos:notation    "2.4" ;
        skos:prefLabel   "Sectoral statistics"@en .

sdmx-subject:subjectMatterDomain
        a                   skos:ConceptScheme ;
        rdfs:label          "SDMX Statistical Subject-Matter Domains"@en ;
        rdfs:seeAlso        sdmx-subject:SubjectMatterDomain ;
        skos:definition     <http://sdmx.org/wp-content/uploads/2009/01/03_sdmx_cog_annex_3_smd_2009.pdf> ;
        skos:hasTopConcept  sdmx-subject:1 , sdmx-subject:2 , sdmx-subject:3 ;
        skos:note           "The SDMX Content Guidelines for Statistical Subject-Matter Domains."@en ;
        skos:prefLabel      "SDMX Statistical Subject-Matter Domains - concept scheme"@en .

sdmx-concept:visArea  a   sdmx:Concept , skos:Concept ;
        rdfs:comment      "The secondary area, as opposed to reference area, to which the measured data is in relation."@en ;
        rdfs:isDefinedBy  <http://sdmx.org/wp-content/uploads/2009/01/01_sdmx_cog_annex_1_cdc_2009.pdf> ;
        rdfs:label        "Counterpart Reference Area"@en ;
        skos:inScheme     sdmx-concept:cog ;
        skos:notation     "urn:sdmx:org.sdmx.infomodel.conceptscheme.Concept=SDMX:CROSS_DOMAIN_CONCEPTS[1.0].VIS_AREA" .

sdmx-attribute:docMethod
        a                 qb:AttributeProperty , rdf:Property ;
        rdfs:comment      "Descriptive text and references to methodological documents available."@en ;
        rdfs:isDefinedBy  <http://sdmx.org/wp-content/uploads/2009/01/01_sdmx_cog_annex_1_cdc_2009.pdf> ;
        rdfs:label        "Documentation on methodology"@en ;
        qb:concept        sdmx-concept:docMethod .

sdmx:ProvisionAgreement
        a             rdfs:Class , owl:Class ;
        rdfs:comment  "A commitment by a data provider to publish data into a certain DataFlow"@en ;
        rdfs:label    "Provision agreement"@en .

sdmx-attribute:refPerWgts
        a                 qb:AttributeProperty , rdf:Property ;
        rdfs:comment      "Dates or periods to which the observations used to compile the weights refer."@en ;
        rdfs:isDefinedBy  <http://sdmx.org/wp-content/uploads/2009/01/01_sdmx_cog_annex_1_cdc_2009.pdf> ;
        rdfs:label        "Reference Period - weights"@en ;
        qb:concept        sdmx-concept:refPerWgts .

sdmx-concept:metaCertified
        a                 sdmx:Concept , skos:Concept ;
        rdfs:comment      "Date of the latest certification provided by the domain manager to confirm that the metadata posted are still up-to-date, even if the content has not been amended."@en ;
        rdfs:isDefinedBy  <http://sdmx.org/wp-content/uploads/2009/01/01_sdmx_cog_annex_1_cdc_2009.pdf> ;
        rdfs:label        "Metadata Update - last certified"@en ;
        skos:broader      sdmx-concept:metaUpdate ;
        skos:inScheme     sdmx-concept:cog ;
        skos:notation     "urn:sdmx:org.sdmx.infomodel.conceptscheme.Concept=SDMX:CROSS_DOMAIN_CONCEPTS[1.0].META_CERTIFIED" .

sdmx-metadata:dissOther
        a                 sdmx:MetadataProperty , rdf:Property ;
        rdfs:comment      "References to the most important other data dissemination done."@en ;
        rdfs:isDefinedBy  <http://sdmx.org/wp-content/uploads/2009/01/01_sdmx_cog_annex_1_cdc_2009.pdf> ;
        rdfs:label        "Dissemination Format - other"@en ;
        qb:concept        sdmx-concept:dissOther .

sdmx-metadata:relPolLegActs
        a                 sdmx:MetadataProperty , rdf:Property ;
        rdfs:comment      "Legal acts and other agreements pertaining to data access."@en ;
        rdfs:isDefinedBy  <http://sdmx.org/wp-content/uploads/2009/01/01_sdmx_cog_annex_1_cdc_2009.pdf> ;
        rdfs:label        "Release Policy - legal acts and other agreements"@en ;
        qb:concept        sdmx-concept:relPolLegActs .

sdmx-attribute:dataPres
        a                 qb:AttributeProperty , rdf:Property ;
        rdfs:comment      "Description of the disseminated data."@en ;
        rdfs:isDefinedBy  <http://sdmx.org/wp-content/uploads/2009/01/01_sdmx_cog_annex_1_cdc_2009.pdf> ;
        rdfs:label        "Data Presentation"@en ;
        qb:concept        sdmx-concept:dataPres .

sdmx-attribute:contactFax
        a                 qb:AttributeProperty , rdf:Property ;
        rdfs:comment      "Fax number of the contact points for the data or metadata."@en ;
        rdfs:isDefinedBy  <http://sdmx.org/wp-content/uploads/2009/01/01_sdmx_cog_annex_1_cdc_2009.pdf> ;
        rdfs:label        "Contact fax number"@en ;
        qb:concept        sdmx-concept:contactFax .

sdmx-code:obsStatus-E
        a                  skos:Concept , sdmx:Concept , sdmx-code:ObsStatus ;
        skos:definition    "Observation obtained through an estimation methodology (e.g. to produce back-casts) or based on the use of a limited amount of data or ad hoc sampling and through additional calculations (e.g. to produce a value at an early stage of the production stage while not all data are available). It may also be used in case of experimental data (e.g. in the context of a pilot ahead of a full scale production process) or in case of data of (anticipated/assessed) low quality. If needed, additional (uncoded) information can be provided through (free text) \"comments\" at the observation level or at a higher level."@en ;
        skos:inScheme      sdmx-code:obsStatus ;
        skos:notation      "E" ;
        skos:prefLabel     "Estimated value"@en ;
        skos:topConceptOf  sdmx-code:obsStatus .

sdmx-concept:contactEmail
        a                 sdmx:Concept , skos:Concept ;
        rdfs:comment      "E-mail address of the contact points for the data or metadata."@en ;
        rdfs:isDefinedBy  <http://sdmx.org/wp-content/uploads/2009/01/01_sdmx_cog_annex_1_cdc_2009.pdf> ;
        rdfs:label        "Contact email address"@en ;
        skos:broader      sdmx-concept:contact ;
        skos:inScheme     sdmx-concept:cog ;
        skos:notation     "urn:sdmx:org.sdmx.infomodel.conceptscheme.Concept=SDMX:CROSS_DOMAIN_CONCEPTS[1.0].CONTACT_EMAIL" .

sdmx-concept:dataRev  a   sdmx:Concept , skos:Concept ;
        rdfs:comment      "Any change in a value of a statistic released to the public."@en ;
        rdfs:isDefinedBy  <http://sdmx.org/wp-content/uploads/2009/01/01_sdmx_cog_annex_1_cdc_2009.pdf> ;
        rdfs:label        "Data Revision"@en ;
        skos:inScheme     sdmx-concept:cog ;
        skos:notation     "urn:sdmx:org.sdmx.infomodel.conceptscheme.Concept=SDMX:CROSS_DOMAIN_CONCEPTS[1.0].DATA_REV" .

sdmx-subject:3.3.1  a    skos:Concept , sdmx:Concept , sdmx-subject:SubjectMatterDomain ;
        skos:broader     sdmx-subject:3.3 ;
        skos:definition  "Living conditions, poverty and cross-cutting social issues - includes work on multidimensional methods to measure poverty, living conditions in the broad sense, social inclusion/exclusion, social indicators, and social situation.\nExcludes:\n- purely monetary approach to poverty (1.5)\n\nExcludes: \n- multi-domain statistics based on a regional approach (3.2)\n- yearbook type of compendia or similar products by international organisations not following a specific thematic approach (3.4)"@en ;
        skos:notation    "3.3.1" ;
        skos:prefLabel   "Living conditions, poverty, and cross-cutting social issues"@en .
